@prefix : <http://informationexchangestandard.org/ont/building/1.0.0-rc1#> .
@prefix building: <http://ies.data.gov.uk/ontology/ies-building1#> .
@prefix dct: <http://purl.org/dc/terms/> .
@prefix dcterms: <http://purl.org/dc/terms/> .
@prefix ex: <http://example.com/> .
@prefix ies: <http://informationexchangestandard.org/ont/ies#> .
@prefix iso8601: <http://iso8601.iso.org/> .
@prefix my: <http://www.mobile.com/model/> .
@prefix owl: <http://www.w3.org/2002/07/owl#> .
@prefix quantitykind: <http://qudt.org/vocab/quantitykind/> .
@prefix qudt: <http://qudt.org/schema/qudt/> .
@prefix rdf: <http://www.w3.org/1999/02/22-rdf-syntax-ns#> .
@prefix rdfs: <http://www.w3.org/2000/01/rdf-schema#> .
@prefix skos: <http://www.w3.org/2004/02/skos/core#> .
@prefix unit: <http://qudt.org/vocab/unit/> .
@prefix vann: <http://purl.org/vocab/vann/> .
@prefix xsd: <http://www.w3.org/2001/XMLSchema#> .

building: a owl:Ontology ;
   owl:versionInfo "1.0.0-rc1" ;
   owl:versionIRI <http://informationexchangestandard.org/ont/building/1.0.0-rc1> ;
   dcterms:title "IES Domain Ontology - Built Environment"@en-gb ;
   dcterms:modified "2025-07-18"^^xsd:date ;
   vann:preferredNamespacePrefix "building" ;
   vann:preferredNamespaceUri "http://informationexchangestandard.org/ont/ies-building#" ;
   dcterms:license <https://spdx.org/licenses/MIT.html> .

building:hasQuantity a owl:ObjectProperty ;
    rdfs:domain ies:Measure ;
    rdfs:range qudt:Quantity ;
    rdfs:label "has Quantity"@en-gb ;
    rdfs:comment "A relationship between an `ies:Measure` and a `qudt:Quantity` that acts as a bridge to the `qudt` ontology." ;
    skos:note "This bridge was intended for IES 4.3.x but was postponed" .

building:AccreditedEnergyAssessor a rdfs:Class ;
    rdfs:label "Accredited Energy Assessor"@en-gb ;
    rdfs:comment "An `ies:ResponsibleActorState` of a professional who has been trained and certified to evaluate the energy performance of  buildings and to produce an authorised result setting out the findings. In the UK, they must be a member of a government-approved accreditation scheme, which ensures that they meet specific competency standards and adhere to a code of conduct. Accreditation schemes also provide quality assurance for the work undertaken by their members, and they ensure that energy assessors maintain their skills and knowledge up to date through continuing professional development." ;
    rdfs:label "Accredited Energy Assessor" ;
    rdfs:comment "An `ies:ResponsibleActorState` of a professional who has been trained and certified to evaluate the energy performance of  buildings and to produce an authorised result setting out the findings. In the UK, they must be a member of a government-approved accreditation scheme, which ensures that they meet competency standards and adhere to a code of conduct. Accreditation schemes also provide quality assurance for the work undertaken by their members, and they ensure that energy assessors maintain their skills and knowledge up to date through continuing professional development." ;
    rdfs:subClassOf ies:PersonState .

building:AddressableLocation a rdfs:Class ;
    rdfs:label "Addressable Location"@en-gb ;
    ies:powertype building:ClassOfAddressableLocation ;
    rdfs:comment "An `ies:Location` that may be any kind of building, or it may be an object that might not have a 'normal' address -- such as a bus station or an electricity substation." ;
    rdfs:subClassOf building:AddressableLocationState,
        ies:Location .

building:AddressableLocationState a rdfs:Class ;
    rdfs:label "Addressable Location State"@en-gb ;
    ies:powertype building:ClassOfAddressableLocationState ;
    rdfs:comment "A temporal state of a AddressableLocation." ;
    rdfs:subClassOf ies:LocationState .

building:AllStoreysOfAStructure a rdfs:Class, building:ClassOfClassOfStorey ;
    rdfs:label "All Storeys Of A Structure"@en ;
    rdfs:comment """An instance of `building:ClassOfClassOfStorey` representing the collection of all `building:Storey` instances contained within a `building:Structure`. Enables reasoning and querying over the set of storeys in a structure.""" ;
    rdfs:subClassOf ies:FiniteClassOfElement, building:ClassOfStorey .

building:AllFloorsOfAStructureUnit a rdfs:Class, building:ClassOfClassOfFloor ;
    rdfs:label "All Floors Of A Structure Unit"@en-gb ;
    rdfs:comment "An instance of `building:ClassOfClassOfFloorState` that is the collection of all the floors of `building:StructureUnit`" ;
    rdfs:subClassOf ies:FiniteClassOfElement, building:ClassOfFloor .

building:AllOpenFireplacesInAStructureUnit a rdfs:Class, building:ClassOfClassOfFireplace ;
    rdfs:label "All Open Fireplaces In A Structure Unit"@en-gb ;
    rdfs:comment """An instance of `building:ClassOfClassOfFireplace` representing the collection of all `building:OpenFireplace` instances located within a `building:StructureUnit`. Useful for reasoning over or querying aggregate sets of technical systems in a built environment.""" ;
    rdfs:subClassOf ies:FiniteClassOfElement, building:ClassOfFireplace .

building:AllWallsOfAStructureUnit a rdfs:Class, building:ClassOfClassOfWall ;
    rdfs:label "All Walls Of A Structure Unit"@en-gb ;
    rdfs:comment """An instance of `building:ClassOfClassOfWall` representing the collection of all `building:Wall` instances located within a `building:StructureUnit`. This allows reasoning over or querying the set of walls within a building unit.""" ;
    rdfs:subClassOf ies:FiniteClassOfElement, building:ClassOfWall .

building:Building a rdfs:Class ;
    rdfs:label "Building"@en-gb ;
    ies:powertype building:ClassOfBuilding ;
    rdfs:comment "A `building:Structure` that is created to serve specific functions, typically for human occupation or use, such as residential, commercial, industrial, or public purposes. Buildings are usually constructed in-place and are intended not to be regularly moved.  Like other structures, a building can exist in various states over time and is characterized by aspects like architectural design, construction methods, and materials used." ;
    rdfs:seeAlso <https://identifier.buildingsmart.org/uri/buildingsmart/ifc/4.3/class/IfcBuilding> ;
    rdfs:subClassOf building:BuildingState,
        building:Structure .

building:BuildingState a rdfs:Class ;
    rdfs:label "Building State"@en-gb ;
    ies:powertype building:ClassOfBuildingState ;
    rdfs:comment "A temporal state of a Building." ;
    rdfs:subClassOf building:StructureState .

building:BuiltEntity a rdfs:Class ;
    rdfs:label "Built Entity" ;
    rdfs:comment "An `ies:Entity` that is primarily intended to be incorporated into a `building:Structure`, but may have all or part of its existence separate from any `building:Structure`.  A BuiltEntity can exist in various states over time." ;
    skos:example "Floor", "Wall", "Roof", "Gate" ;
    rdfs:seeAlso <https://search.bsdd.buildingsmart.org/uri/buildingsmart/ifc/4.3/class/IfcBuiltElement> ;
    rdfs:subClassOf building:BuiltEntityState,
        ies:Entity .

building:BuiltEntityState a rdfs:Class ;
    rdfs:label "Built Entity State"@en-gb ;
    rdfs:comment "An`ies:State` that is the temporal state of a `building:BuiltEntity`" ;
    rdfs:subClassOf ies:State .

building:AsBuilt a rdfs:Class ;
    rdfs:label "As Built" ;
    rdfs:comment "A `building:BuiltEntityState` that matches the actual condition of the `building:BuiltEntity` at the time it was completed." ;
    rdfs:subClassOf building:BuiltEntityState .

building:BuiltForm a rdfs:Class ;
    rdfs:label "Built Form"@en-gb ;
    rdfs:comment "A `building:ClassOfStructureUnit` that is a classifier of `building:StructureUnit` that defines the built form of a Structure.  Instances of this class are `rdfs:subClass(es)Of` `building:StructureUnitState`." ;
    rdfs:label "Built Form" ;
    rdfs:comment "A `building:ClassOfStructureUnit` that is a classifier of `building:StructureUnit` that defines the built form of a Structure.  Instances of this class are `rdfs:subClass(es)Of` `building:StructureUnitState`." ;
    skos:example "Detached", "Semi-Detached", "End of Terrace" ;
    rdfs:subClassOf building:ClassOfStructureUnitState .

building:CO2Emission a rdfs:Class ;
    rdfs:label "CO2 Emission"@en-gb ;
    rdfs:comment "A `building:ChemicalCompoundRelease` that is the release of carbon dioxide into the atmosphere from various sources, primarily from the burning of fossil fuels like coal, oil, and gas for energy production. " ;
    rdfs:subClassOf building:ChemicalCompoundRelease .

building:CO2EmissionEstimate a rdfs:Class ;
    rdfs:label "CO2 Emission Estimate"@en-gb ;
    rdfs:comment "An `ies:Assessment` that estimates the release of carbon dioxide (CO2)." ;
    rdfs:subClassOf building:EnergyPerformanceAssessment .

building:CO2Released a rdfs:Class ;
    rdfs:label "A release of CO2 event"@en-gb ;
    rdfs:comment "A `building:ChemicalCompoundReleased` that is the release of `building:CO2`." ;
    rdfs:subClassOf building:ChemicalCompoundReleased .

building:StuffPortion a rdfs:Class ;
    rdfs:label "A Portion Of Stuff"@en-gb ;
    rdfs:comment "An `ies:Element` that is part of some stuff (`ies:Stuff`) and has the composition or origin that is characteristic of that stuff" ;
    ies:eachMemberIsPartOfSomeMemberOf ies:Stuff;
    rdfs:subClassOf ies:Element .

building:ChemicalCompound a rdfs:Class ;
    rdfs:label "Chemical Compound"@en-gb ;
    rdfs:comment "An `ies:Stuff` that consists of atoms of two or more chemical elements." ;
    rdfs:subClassOf ies:Stuff .

building:ChemicalCompoundPortion a rdfs:Class ;
    rdfs:label "A Portion Of Chemical Compound" ;
    rdfs:comment "A `building:StuffPortion` that is part of some `building:ChemicalCompound`" ;
    rdfs:subClassOf building:StuffPortion .

building:ChemicalCompoundRelease a rdfs:Class ;
    rdfs:label "Chemical Compound Release"@en-gb ;
    rdfs:comment "An `ies:Event` that is the release of some `building:ChemicalCompoundPortion`" ;
    rdfs:subClassOf ies:Event .

building:ChemicalCompoundReleased a rdfs:Class ;
    rdfs:label "Chemical Compound Released"@en-gb ;
    rdfs:comment "An `ies:BoundingState` that marks the end of the `building:ChemicalCompound` released event." ;
    rdfs:subClassOf ies:BoundingState .

building:ClassOfAddressableLocation a rdfs:Class ;
    rdfs:label "Class Of Addressable Location"@en-gb ;
    rdfs:comment "An `building:ClassOfLocation` that classifies `building:AddressableLocation`.  Instances of this class are subClasses of `building:AddressableLocation`." ;
    rdfs:subClassOf building:ClassOfLocation .

building:ClassOfLocation a rdfs:Class ;
    rdfs:label "Class Of Location"@en-gb ;
    rdfs:comment "An `ies:ClassOfEntity` that is a classifier of `ies:Location`.  Instances of this class are `rdfs:subClass(es)Of` `ies:Location`." ;
    skos:note "To be migrated in future IES releases" ;
    rdfs:subClassOf ies:ClassOfEntity .

building:ClassOfAddressableLocationState a rdfs:Class ;
    rdfs:label "Class Of Addressable Location State"@en-gb ;
    rdfs:comment """An `building:ClassOfLocationState` that classifies `building:AddressableLocationState`. Instances of this class are subClasses of `building:AddressableLocationState`.
""" ;
    rdfs:subClassOf building:ClassOfLocationState .

building:ClassOfLocationState a rdfs:Class ;
    rdfs:label "Class Of Location State"@en-gb ;
    rdfs:comment "An `ies:ClassOfState` that is a classifier of `ies:LocationState`. Instances of this class are `rdfs:subClass(es)Of` `ies:LocationState`. " ;
    skos:note "To be migrated in future IES releases" ;
    rdfs:subClassOf ies:ClassOfState .

building:ClassOfAssetState a rdfs:Class ;
    rdfs:label "Class Of Asset State"@en-gb ;
#    ies:powertype ies:ClassOfAssetState ;
    rdfs:comment "An`ies:ClassOfState` that classifies `ies:AssetState`.  Instances of this class are `rdfs:subClass(es)Of` `ies:AssetState`." ;
    rdfs:subClassOf ies:ClassOfState .

building:ClassOfBuilding a rdfs:Class ;
    rdfs:label "Class Of Building"@en-gb ;
    rdfs:comment "A `building:ClassOfStructure` that classifies `building:Building`.  Instances of this class are `rdfs:subClass(es)Of` of `building:Building`. " ;
    rdfs:subClassOf building:ClassOfStructure .

building:ClassOfBuildingState a rdfs:Class ;
    rdfs:label "Class Of Building State"@en-gb ;
    rdfs:comment "A `building:ClassOfStructureState` that classifies `building:BuildingState`.  Instances of this class are `rdfs:subClass(es)Of` of `building:BuildingState`." ;
    rdfs:subClassOf building:ClassOfStructureState .

building:ClassOfBuiltEntity a rdfs:Class ;
    rdfs:label "Class Of Built Entity"@en-gb ;
    rdfs:comment "A `building:ClassOfEntity` that is a classifier of `building:BuiltEntity`.  Instances of this class are `rdfs:subClass(es)Of` `building:BuiltEntity`." ;
    rdfs:subClassOf ies:ClassOfEntity .

building:ClassOfBuiltEntityState a rdfs:Class ;
    rdfs:label "Class Of Built Entity State"@en-gb ;
    rdfs:comment "A `building:ClassOfEntityState` that is a classifier of `building:BuiltEntityState`. Instances of this class are `rdfs:subClass(es)Of` `building:BuiltEntityState`. " ;
    rdfs:subClassOf building:ClassOfEntityState .


building:ClassOfClassOfBuiltEntity a rdfs:Class ;
    rdfs:label "Class Of Class Of Built Entity"@en-gb ;
    rdfs:comment "An `ies:ClassOfClassOfEntity` that classifies `building:ClassOfBuiltEntity`. Instances of this class are `rdfs:subClass(es)Of` `building:ClassOfBuiltEntity`." ;
    rdfs:subClassOf ies:ClassOfClassOfEntity .

building:ClassOfClassOfBuiltEntityState a rdfs:Class ;
    rdfs:label "Class Of Class Of Built Entity State"@en-gb ;
    rdfs:comment "A `ies:ClassOfClassOfElement` that classifies `building:ClassOfBuiltEntityState`. Instances of this class are `rdfs:subClass(es)Of` `building:ClassOfBuiltEntityState`." ;
    skos:note "It will eventually be made a subclass of `ies:ClassOfClassOfState`." ;
    rdfs:subClassOf ies:ClassOfClassOfElement .

building:ClassOfEntityState a rdfs:Class ;
    rdfs:subClassOf ies:ClassOfState ;
    skos:note "Missing for ies 4.3.3 " .

# building:ClassOfEnergyPerformanceAssessmentResultState a rdfs:Class ;
#     rdfs:label "Class Of Energy Performance Assessment Result State"@en-gb ;
#     rdfs:comment "A `building:ClassOfIndividualDocumentState` that is a classifier on `building:EnergyPerformanceAssessmentResultState`.  Instances of this class are `rdfs:subClass(es)Of` `building:EnergyPerformanceAssessmentResultState`." ;
#     rdfs:subClassOf building:ClassOfIndividualDocumentState .

building:ClassOfEnergyPerformanceCertificate a rdfs:Class ;
    rdfs:label "Class Of Energy Performance Certificate"@en-gb ;
    rdfs:comment "A `building:ClassOfWorkOfDocumentation` that classifies `building:EnergyPerformanceCertificate`.  Instances of this class are `rdfs:subClass(es)Of `building:EnergyPerformanceCertificate`." ;
    rdfs:subClassOf building:ClassOfWorkOfDocumentation .

building:ClassOfWorkOfDocumentation a rdfs:Class ;
    rdfs:label "Class Of Work Of Documentation"@en-gb ;
    rdfs:comment "An `ies:ClassOfClassOfEntity` that classifies `ies:WorkOfDocumentation`.  Instances of this class are `rdfs:subClass(es)Of` `ies:WorkOfDocumentation`." ;
    skos:note "To be migrated in future IES releases" ;
    rdfs:subClassOf ies:ClassOfClassOfEntity .

building:ClassOfFireplace a rdfs:Class ;
    rdfs:label "Class Of Fireplace"@en-gb ;
    rdfs:comment """A `building:ClassOfTechnicalSystem` that classifies instances of `building:Fireplace`. Acts as a superclass for classifications of specific fireplace types.""" ;
    rdfs:subClassOf building:ClassOfTechnicalSystem .

building:ClassOfOpenFireplace a rdfs:Class ;
    rdfs:label "Class Of Open Fireplace"@en-gb ;
    rdfs:comment """A `building:ClassOfFirePlace` that classifies instances of `building:OpenFireplace`. This is a subclass of `building:ClassOfFireplace`.""" ;
    rdfs:subClassOf building:ClassOfFireplace .

building:ClassOfEnclosedFireplace a rdfs:Class ;
    rdfs:label "Class Of Enclosed Fireplace"@en-gb ;
    rdfs:comment """A `building:ClassOfFirePlace` that classifies instances of `building:EnclosedFireplace`. This is a subclass of `building:ClassOfFireplace`.""" ;
    skos:note "Parallel structure to ClassOfOpenFireplace to support ontology consistency." ;
    rdfs:subClassOf building:ClassOfFireplace .

building:ClassOfFloor a rdfs:Class ;
    rdfs:label "Class Of Floor"@en-gb ;
    rdfs:comment """A `building: ClassOfBuiltEntity` that is a classifier of `building:Floor`.  Instances of this class are `rdfs:subClass(es)Of` `building:Floor`.
      """ ;
    rdfs:subClassOf building:ClassOfBuiltEntity .

building:ClassOfClassOfFireplace a rdfs:Class ;
    rdfs:label "Class Of Class Of Fireplace"@en-gb ;
    rdfs:comment """A meta-class that classifies `building:ClassOfFireplace` and its subclasses, such as `building:ClassOfOpenFireplace` and `building:ClassOfEnclosedFireplace`. Part of the meta-modelling layer that organizes classes of classifiers.""" ;
    rdfs:subClassOf building:ClassOfClassOfTechnicalSystem .

building:ClassOfClassOfTechnicalSystem a rdfs:Class ;
    rdfs:label "Class Of Class Of Technical System"@en-gb ;
    rdfs:comment "A meta-class that classifies `building:ClassOfTechnicalSystem` and its subclasses. This is part of the meta-modelling layer that organizes classifiers of technical systems." ;
    rdfs:subClassOf ies:ClassOfClassOfEntity .

building:ClassOfFloorState a rdfs:Class ;
    rdfs:label "Class Of Floor State"@en ;
    rdfs:comment "A `building:ClassOfBuiltEntityState` that is a classifier of `building:FloorState`.  Instances of this class are `rdfs:subClass(es)Of` `building:FloorState`." ;
    rdfs:subClassOf building:ClassOfBuiltEntityState .

building:ClassOfClassOfFloor a rdfs:Class ;
    rdfs:label "Class Of Class Of Floor"@en-gb ;
    rdfs:comment "A `building:ClassOfClassOfBuiltEntity` that classifies `building:ClassOfFloor`. Instances of this class are `rdfs:subClass(es)Of` `building:ClassOfFloor`." ;
    rdfs:subClassOf building:ClassOfClassOfBuiltEntity .

building:ClassOfClassOfFloorState a rdfs:Class ;
    rdfs:label "Class Of Class Of Floor State"@en-gb ;
    rdfs:comment "A `building:ClassOfClassOfBuiltEntityState` that classifies `building:ClassOfFloorState`. Instances of this class are `rdfs:subClass(es)Of` `building:ClassOfFloorState`." ;
    rdfs:subClassOf building:ClassOfClassOfBuiltEntityState .

building:ClassOfIndividualDocumentState a rdfs:Class ;
    rdfs:label "Class Of Individual Document State"@en-gb ;
    rdfs:comment "A `building:ClassOfAssetState` that is a classifier of `building:IndividualDocumentState`.  Instances of this class are `rdfs:subClass(es)Of` `building:IndividualDocumentState`. " ;
    rdfs:subClassOf building:ClassOfAssetState .

building:ClassOfRoof a rdfs:Class ;
    rdfs:label "Class Of Roof"@en-gb ;
    rdfs:comment """A `building:ClassOfBuiltEntity` that is a classifier of `building:Roof`.  Instances of this class are `rdfs:subClass(es)Of` `building:Roof`.
      """ ;
    rdfs:subClassOf building:ClassOfBuiltEntity .

building:ClassOfClassOfRoof a rdfs:Class ;
    rdfs:label "Class Of Class Of Roof"@en ;
    rdfs:comment """A meta-class that classifies `building:ClassOfRoof` and its subclasses. This is part of the meta-modelling layer that organizes classifiers of roofs.""" ;
    rdfs:subClassOf building:ClassOfClassOfBuiltEntity .

building:AllRoofsOfAStructureUnit a rdfs:Class, building:ClassOfClassOfRoof ;
    rdfs:label "All Roofs Of A Structure Unit"@en ;
    rdfs:comment """An instance of `building:ClassOfClassOfRoof` representing the collection of all `building:Roof` instances located within a `building:StructureUnit`. Enables reasoning and querying over the set of roofs in a building unit.""" ;
    rdfs:subClassOf ies:FiniteClassOfElement, building:ClassOfRoof .

building:ClassOfRoofState a rdfs:Class ;
    rdfs:label "Class Of Roof State"@en-gb ;
    rdfs:comment "A `building:ClassOfBuiltEntityState` tha is a classifier of `building:RoofState`.  Instance of this class are `rdfs:subClass(es)Of` `building:RoofState`." ;
    rdfs:subClassOf building:ClassOfBuiltEntityState .

building:ClassOfSpace a rdfs:Class ;
    rdfs:label "Class Of Space"@en-gb ;
    rdfs:comment "An `ies:ClassOfEntity` that is a classifier of `building:Space`.  Instances of this Class are `rdfs:subClass(es)Of` `building:Space`." ;
    rdfs:subClassOf ies:ClassOfEntity .

building:ClassOfSpaceState a rdfs:Class ;
    rdfs:label "Class Of Space State"@en-gb ;
    rdfs:comment "An `ies:ClassOfState` that is a classifier of `building:SpaceState`. Instances of this class are `rdfs:subClass(es)Of` `building:SpaceState`. " ;
    rdfs:subClassOf ies:ClassOfState .

building:ClassOfStorey a rdfs:Class ;
    rdfs:label "Class Of Storey"@en ;
    rdfs:comment """ A `ies:ClassOfEntity` that is a classifier of `Building:Storey`.  Instances of this class are `rdfs:subClass(es)Of` `building:Storey`.
      """ ;
    rdfs:subClassOf ies:ClassOfEntity .

building:ClassOfClassOfStorey a rdfs:Class ;
    rdfs:label "Class Of Class Of Storey"@en ;
    rdfs:comment """A meta-class that classifies `building:ClassOfStorey` and its subclasses. Part of the meta-modelling layer that organizes classifiers of storeys.""" ;
    rdfs:subClassOf ies:ClassOfClassOfEntity .

building:ClassOfStoreyState a rdfs:Class ;
    rdfs:label "Class Of Storey State"@en ;
    rdfs:comment """A `ies:ClassOfState` that is a classifier of `building:StoreyState`.  Instances of this class are `rdfs:subClass(es)Of` `building:StoreyState`.
      """ ;
    rdfs:subClassOf ies:ClassOfState .

building:ClassOfStructure a rdfs:Class ;
    rdfs:label "Class Of Structure"@en-gb ;
    rdfs:comment "An `ies:ClassOfEntity` that is a classifier of `building:Structure`. Instances of this class are `rdfs:subClass(es)Of` `building:Structure`." ;
    rdfs:subClassOf ies:ClassOfEntity .

building:ClassOfStructureState a rdfs:Class ;
    rdfs:label "Class Of Structure State"@en-gb ;
    rdfs:comment "An `ies:ClassOfState` that is a classifier of `building:StructureState`. Instances of this class are `rdfs:subClass(es)Of` `building:StructureState`." ;
    rdfs:subClassOf ies:ClassOfState .

building:ClassOfStructureUnit a rdfs:Class ;
    rdfs:label "Class Of Structure Unit"@en-gb ;
    rdfs:comment "An `ies:ClassOfEntity` that is a classifier of `building:StructureUnit`. Instances of this class are `rdfs:subClass(es)Of` `building:StructureUnit`." ;
    rdfs:subClassOf ies:ClassOfEntity .

building:ClassOfStructureUnitState a rdfs:Class ;
    rdfs:label "Class Of Structure Unit State"@en-gb ;
    rdfs:comment "An `ies:ClassOfState` that is a classifier of `building:StructureUnitState`. Instances of this class are `rdfs:subClass(es)Of` `building:StructureUnitState`." ;
    rdfs:subClassOf ies:ClassOfState .

building:ClassOfStuff a rdfs:Class ;
    rdfs:label "Class Of Stuff"@en-gb ;
    rdfs:comment """An `ies:ClassOfElement` that is a classifier of `ies:Stuff`. Instances of this class are `rdfs:subClass(es)Of` `ies:Stuff`.
      """ ;
    rdfs:subClassOf ies:ClassOfElement .

building:ClassOfWall a rdfs:Class ;
    rdfs:label "Class Of Wall"@en-gb ;
    rdfs:comment """A `building:ClassOfBuiltEntity` the is a classifier of `building:Wall`.  Instances of this class are `rdfs:subClass(es)Of` `building:Wall`.
      """ ;
    rdfs:subClassOf building:ClassOfBuiltEntity .

building:ClassOfClassOfWall a rdfs:Class ;
    rdfs:label "Class Of Class Of Wall"@en-gb ;
    rdfs:comment """A meta-class that classifies `building:ClassOfWall` and its subclasses. This class is part of the meta-modelling layer that organizes classifiers of wall elements.""" ;
    rdfs:subClassOf building:ClassOfClassOfBuiltEntity .

building:ClassOfWallState a rdfs:Class ;
    rdfs:label "Class Of Wall State"@en-gb ;
    rdfs:comment "A `building:ClassOfBuiltEntityState` the is a classifier of `building:WallState`. Instances of this class are `rdfs:subClass(es)Of` `building:WallState`." ;
    rdfs:subClassOf building:ClassOfBuiltEntityState .

building:ClassOfWindow a rdfs:Class ;
    rdfs:label "Class Of Window"@en-gb ;
    rdfs:comment "A `building:ClassOfBuiltEntity` the is a classifier of `building:Window`. Instances of this class are `rdfs:subClass(es)Of` `building:Window`." ;
    rdfs:subClassOf building:ClassOfBuiltEntity .

building:ClassOfClassOfWindow a rdfs:Class ;
    rdfs:label "Class Of Class Of Window"@en ;
    rdfs:comment """A meta-class that classifies `building:ClassOfWindow` and its subclasses. This is part of the meta-modelling layer that organizes classifiers of windows.""" ;
    rdfs:subClassOf building:ClassOfClassOfBuiltEntity .

building:AllWindowsOfAStructureUnit a rdfs:Class, building:ClassOfClassOfWindow ;
    rdfs:label "All Windows Of A Structure Unit"@en ;
    rdfs:comment """An instance of `building:ClassOfClassOfWindow` representing the collection of all `building:Window` instances located within a `building:StructureUnit`. Enables reasoning and querying over the set of windows within a building unit.""" ;
    rdfs:subClassOf ies:FiniteClassOfElement, building:ClassOfWindow .

building:ClassOfWindowState a rdfs:Class ;
    rdfs:label "Class Of Window State"@en-gb ;
    rdfs:comment "A `building:ClassOfBuiltEntityState` the is a classifier of `building:WindowState`. Instances of this class are `rdfs:subClass(es)Of` `building:WindowState`." ;
    rdfs:subClassOf building:ClassOfBuiltEntityState .

building:ConstructedInPeriod a rdfs:Class ;
    rdfs:label "Constructed In Period"@en-gb ;
    rdfs:comment "An `ies:ArbitraryPeriod` during which a structure can be regarded as completed." ;
    rdfs:subClassOf ies:ArbitraryPeriod .

building:ConstructedState a rdfs:Class ;
    rdfs:label "Constructed State"@en-gb ;
    rdfs:comment "An `ies:Created` that is a state indicating that the `ies:Entity` was constructed." ;
    rdfs:subClassOf ies:BoundingState ;
    skos:editorialNote "Could be a subClassOf ies:Created" .

building:CostEstimate a rdfs:Class ;
    rdfs:label "Cost Estimate"@en-gb ;
    rdfs:comment "An `building:EnergyPerformanceAssessment` that estimates a cost." ;
    rdfs:subClassOf building:EnergyPerformanceAssessment .

building:AssessPerformanceOfInsulation a rdfs:Class ;
    rdfs:label "Assess Performance Of Insulation"@en-gb ;
    rdfs:comment "A `building:EnergyPerformanceAssessment` that assesses the relative performance of the insulation of a `building:StructureUnit`" ;
    rdfs:subClassOf building:EnergyPerformanceAssessment .

building:AssessWallInsulation a rdfs:Class ;
    rdfs:subClassOf building:AssessPerformanceOfInsulation ;
    rdfs:label "Assess Wall Insulation"@en-gb ;
    rdfs:comment "A `building:AssessPerformanceOfInsulation` that assesses the nature of wall insulation of a `building:StructureUnit" .
building:AssessFloorInsulation a rdfs:Class ;
    rdfs:subClassOf building:AssessPerformanceOfInsulation ;
    rdfs:label "Assess Floor Insulation"@en-gb ;
    rdfs:comment "A `building:AssessPerformanceOfInsulation` that assesses the nature of floor insulation of a `building:StructureUnit" .

building:AssessRoofInsulationThickness a rdfs:Class ;
    rdfs:subClassOf building:AssessPerformanceOfInsulation ;
    rdfs:label "Assess Roof Insulation Thickness"@en-gb ;
    rdfs:comment "A `building:AssessPerformanceOfInsulation` that assesses the the thickness of roof insulation of a `building:StructureOrStructureUnit" .

building:DescribeHeatingSystem a rdfs:Class ;
    rdfs:subClassOf building:EnergyPerformanceAssessment ;
    rdfs:label "Describe Heating System"@en-gb ;
    rdfs:comment "A `building:EnergyPerformanceAssessment` that describes the installed heating system." .

building:DetermineRoofInsulationLocation a rdfs:Class ;
    rdfs:subClassOf building:AssessPerformanceOfInsulation ;
    rdfs:label "Determine Roof Insulation Location"@en-gb ;
    rdfs:comment "A `building:AssessPerformanceOfInsulation` that assesses the the location of roof insulation of a `building:StructureOrStructureUnit" .

building:AssessWindowInsulation a rdfs:Class ;
    rdfs:subClassOf building:AssessPerformanceOfInsulation ;
    rdfs:label "Assess Window Insulation"@en-gb ;
    rdfs:comment "A `building:AssessPerformanceOfInsulation` that assesses the glazing of a `building:StructureUnit" .

building:AssessConstructionMethod a rdfs:Class ;
    rdfs:label "AssessConstructionMethod"@en-gb ;
    rdfs:comment "A `building:EnergyPerformanceAssessment` that assesses the method of construction of the `built:Entities` that are part of a `building:StructureUnit`" ;
    rdfs:subClassOf building:EnergyPerformanceAssessment .

building:AssessWallConstruction a rdfs:Class ;
    rdfs:label "Assess Wall Construction"@en-gb ;
    rdfs:comment "A `building:AssessConstructionMethod` that assesses the method of construction of the `building:Wall` of a `building:StructureUnit`" ;
    rdfs:subClassOf building:AssessConstructionMethod .

building:AssessFloorConstruction a rdfs:Class ;
    rdfs:label "Assess Floor Construction"@en-gb ;
    rdfs:comment "A `building:AssessConstructionMethod` that assesses the method of construction of the `building:Floor` of a `building:StructureUnit`" ;
    rdfs:subClassOf building:AssessConstructionMethod .

building:AssessRoofConstruction a rdfs:Class ;
    rdfs:label "Assess Roof Construction"@en-gb ;
    rdfs:comment "A `building:AssessConstructionMethod` that assesses the method of construction of the `building:Roof` of a `building:StructureOrStructureUnit`" ;
    rdfs:subClassOf building:AssessConstructionMethod .

building:EPCAssessment a rdfs:Class ;
    rdfs:label "UK Energy Performance Certificate (EPC) Assessment"@en-gb ;
    rdfs:comment "An `ies:Assessment` that assesses the various states of a building in the UK at the time of the assessment. " ;
    rdfs:subClassOf building:EnergyPerformanceAssessment .

building:EnergyPerformanceAssessment a rdfs:Class ;
    rdfs:label "Energy Performance Assessment"@en-gb ;
    rdfs:comment "An `ies:Assessment` that is the assessment of the energy performance of a `building:StructureState` or `building:StructureUnitState`" ;
    rdfs:subClassOf ies:Assessment .

building:DetermineTotalFloorArea a rdfs:Class ;
    rdfs:subClassOf building:EnergyPerformanceAssessment ;
    rdfs:label "Determine Total Floor Area"@en-gb ;
    rdfs:comment "A `building:EnergyPerformanceAssessment` which measures or estimates the area of flooring of a `building:StructureUnit`" .

building:AssessHeatingSystem a rdfs:Class ;
    rdfs:subClassOf building:EnergyPerformanceAssessment ;
    rdfs:label "AssessHeatingSystems"@en-gb ;
    rdfs:comment "A `building:EnergyPerformanceAssessment` which assesses the energy performance of the heating system." .

building:CountNumberOfOpenFireplaces a rdfs:Class ;
    rdfs:subClassOf building:AssessHeatingSystem ;
    rdfs:label "Count Number Of Open Fireplaces"@en-gb ;
    rdfs:comment "A `building:AssessHeatingSystem` that counts the number of open fireplaces." .

building:DetermineMainPurposeOfUse a rdfs:Class ;
    rdfs:subClassOf building:EnergyPerformanceAssessment ;
    rdfs:label "Determine Main Purpose Of Use"@en-gb ;
    rdfs:comment "A `building:EnergyPerformanceAssessment` in which the primary purpose of use of the `building:StructureUnit`." .

building:DetermineStructureUnitType a rdfs:Class ;
    rdfs:subClassOf building:EnergyPerformanceAssessment ;
    rdfs:label "Determine Structure Unit Type"@en-gb ;
    rdfs:comment "A `building:EnergyPerformanceAssessment` to establish the type of the `building:StructureUnit`." .

building:DetermineBuiltForm a rdfs:Class ;
    rdfs:subClassOf building:EnergyPerformanceAssessment ;
    rdfs:label "Determine Built Form"@en-gb ;
    rdfs:comment "A `building:EnergyPerformanceAssessment` to establish the built form of the `building:StructureUnit`." .

building:DetermineConstructionAgeBand a rdfs:Class ;
    rdfs:subClassOf building:EnergyPerformanceAssessment ;
    rdfs:label "Determine Construction Age Band"@en-gb ;
    rdfs:comment "A `building:EnergyPerformanceAssessment` to establish the approximate age of the `building:StructureOrStructureUnit`" .

building:DetermineTypeOfVentilation a rdfs:Class ;
    rdfs:subClassOf building:EnergyPerformanceAssessment ;
    rdfs:label "Determine Type Of Ventilation"@en-gb ;
    rdfs:comment "A `building:EnergyPerformanceAssessment` to establish the type of ventilation of the `building:StructureUnit`." .

building:assessedStateForEnergyPerformance a owl:ObjectProperty ;
    rdfs:label "assessed state for EPC"@en-gb ;
    rdfs:domain building:EnergyPerformanceAssessment ;
    rdfs:range ies:State ;
    rdfs:comment "A relation that holds between a `building:EnergyPerformanceAssessment` and a `ies:State` that is the target of the assessment." ;
    rdfs:subPropertyOf ies:assessed .

building:assumedStateForEnergyPerformance a owl:ObjectProperty ;
    rdfs:label "assumed state for EPC" ;
    rdfs:domain building:EnergyPerformanceAssessment ;
    rdfs:range ies:State ;
    rdfs:comment "A relation that holds between a `building:EnergyPerformanceAssessment` and a `ies:State` that is the target of the assessment where the assessor has made a claim without any particular evidence." ;
    rdfs:subPropertyOf ies:assessed .

building:EnergyPerformanceAssessmentResult a rdfs:Class ;
    rdfs:label "Energy Performance Assessment Result"@en-gb ;
    rdfs:comment "An `ies:EventParticipant` that is the result of an `building:EnergyPerformanceAssessment`.";
    rdfs:subClassOf ies:EventParticipant .

# building:EnergyPerformanceAssessmentResultState a rdfs:Class ;
#     rdfs:label "Energy Performance Assessment Result State"@en-gb ;
#     ies:powertype building:ClassOfEnergyPerformanceCertificateState ;
#     rdfs:comment "A temporal state of a `building:EnergyPerformanceAssessmentResult`." ;
#     rdfs:subClassOf building:IndividualDocumentState .

building:EnergyPerformanceCertificate a rdfs:Class ;
    rdfs:label "Energy Performance Certificate"@en-gb ;
    rdfs:comment "A `ies:IndividualDocument` that is a certificate issued in the UK to provide evidence of a `building:EPCAssessment`." ;
    rdfs:subClassOf ies:ClassOfIndividualDocument .

building:isValidityPeriodOf a owl:ObjectProperty ;
    rdfs:label "is the valid period of (EPC)" ;
    rdfs:subPropertyOf ies:isStateOf ;
    rdfs:domain ies:BoundingState ;
    rdfs:range ies:IndividualDocument ;
    rdfs:comment "An `ies:isStateOf` relationship that asserts the start and end `ies:ParticularPeriod`s during which the document can be considered to be valid." ;
    skos:note "This differs from the treatment in IES 4.3 RC in that it establishes a `ies:State` for the `EPCAssessment`." .

building:EPCValidity a rdfs:Class ;
    rdfs:label "Energy Performance Certificate Validity"@en-gb ;
    rdfs:comment "An `ies:BoundingState` that asserts that an `building:EnergyPerformanceCertificate` is valid." ;
    rdfs:subClassOf ies:BoundingState .

building:EnvironmentalImpactRatingValue a rdfs:Class ;
    rdfs:label "Environmental Impact Rating"@en-gb ;
    rdfs:comment "A `building:MeasureOfTheEnvironment` that is the rating of the environmental impact assessed by the UK EPC assessment process." ;
    rdfs:subClassOf building:MeasureOfTheEnvironment .

building:EnvironmentalImpactRatingCalculation a rdfs:Class ;
    rdfs:label "Environmental Impact Rating Calculation"@en-gb ;
    rdfs:comment "An `ies:Assessment` that is the calculation of the environmental impact based on information provided during a `building:EPCAssessment`." ;
    rdfs:subClassOf building:EnergyPerformanceAssessment .

building:Fireplace a rdfs:Class ;
    rdfs:label "Fireplace"@en ;
    rdfs:comment """A `building:HeatProductionSystem` designed to contain a fire for heating, ambiance, or cooking. Can be either open or enclosed in design.""" ;
    rdfs:subClassOf building:HeatProductionSystem ;
    ies:powertype building:ClassOfFireplace.

building:OpenFireplace a rdfs:Class ;
    rdfs:label "Open Fireplace"@en ;
    rdfs:comment """A `building:Fireplace` where the fire is exposed to the room, typically built into the wall with a firebox, chimney, and hearth.""" ;
    rdfs:subClassOf building:Fireplace ;
    ies:powertype building:ClassOfOpenFireplace .

building:EnclosedFireplace a rdfs:Class ;
    rdfs:label "Enclosed Fireplace"@en ;
    rdfs:comment """A `building:Fireplace` where the fire is enclosed behind glass or metal, providing improved efficiency and safety over open fireplaces.""" ;
    rdfs:subClassOf building:Fireplace ;
    ies:powertype building:ClassOfEnclosedFireplace .

building:Floor a rdfs:Class ;
    rdfs:label "Floor"@en ;
    ies:powertype building:ClassOfFloor ;
    rdfs:comment """A `building:BuiltEntity` that is a horizontal structural component of a building that provides a surface for occupants to walk on and supports the load of furniture, fixtures, and other elements within a `building:Space`. Floors serve as physical boundaries between vertical levels in a multistorey building and may also act as thermal, acoustic, or fire-resistant barriers.
    A floor is considered distinct when it:
	  •	Separates different vertical levels in the building;
	  •	Is constructed as an independent structural element;
	  •	Serves a distinct function (e.g., parking deck, mezzanine);
	  •	Uses a different material or construction method; or
	  •	Is divided by a significant opening or void that results in independent sections.""" ;
    rdfs:seeAlso <https://search.bsdd.buildingsmart.org/uri/buildingsmart/ifc/4.3/class/IfcCoveringFLOORING>,
        <https://search.bsdd.buildingsmart.org/uri/buildingsmart/ifc/4.3/class/IfcSlabFLOOR> ;
    rdfs:subClassOf building:BuiltEntity,
        building:FloorState .

building:FloorArea a rdfs:Class ;
    rdfs:label "Floor Area"@en-gb ;
    rdfs:comment "An `ies:Measure` that is the area of the `building:Floor` of a  `building:Structure`." ;
    rdfs:subClassOf ies:Measure .

building:SurfaceArea a rdfs:Class ;
    rdfs:label "Surface Area" ;
    rdfs:comment "An `ies:Measure` of the extent of an exposed building surface (e.g. roof, roof section, wall, façade, floor, or similar structural element), expressed in two dimensions." ;
    rdfs:subClassOf ies:Measure .

building:OperableWithOneEnergySource a rdfs:Class, ies:Characteristic ;
        rdfs:label "Operable With One Energy Source"@en-gb ;
        rdfs:comment "The characteristic that belongs to those technical systems that can operate on only one energy source - for example, a conventional petrol car, or a furnace heating system that operates on gas only" ;
        rdfs:subClassOf building:TechnicalSystem .

building:OperableWithMultipleEnergySources a rdfs:Class, ies:Characteristic ;
        rdfs:label "Operable With Multiple Energy Sources"@en-gb ;
        rdfs:comment "The characteristic that belongs to those technical systems that can operate on two or more energy sources - for example, a hybrid car, or a heating system that can operate on both electricity and gas" ;
        rdfs:subClassOf building:TechnicalSystem .

building:estimateOfEnergyCost a owl:ObjectProperty ;
    rdfs:label "Estimated Energy Cost"@en-gb ;
    rdfs:comment "An `ies:transferValue` that is the estimated cost associated with energy provision, such as the projected domestic heating cost." ;
    rdfs:domain building:StructureUnitState ;
    rdfs:range ies:AmountOfMoney ;
    rdfs:subPropertyOf ies:transferValue .

building:emitsChemical a owl:ObjectProperty ;
    rdfs:label "emits the chemical"@en-gb ;
    rdfs:comment "A relationship that asserts the end of the emission event of a chemical compound" ;
    rdfs:domain ies:BoundingState ;
    rdfs:range building:ChemicalCompoundPortion .

building:FloorConstruction a rdfs:Class ;
    rdfs:label "Floor By Construction"@en ;
    rdfs:comment "A `building:ClassOfFloor` that is a classifier of `building:Floor` by the method of construction. Instances of this class are `rdfs:subClass(es)`Of `building:Floor`." ;
    rdfs:subClassOf building:ClassOfFloor .

building:FloorInsulation a rdfs:Class ;
    rdfs:label "Floor By Insulation"@en ;
    rdfs:comment "A `building:ClassOfFloor` that is classifier of `building:Floor` by the type of insulation.  Instances of this class are `rdfs:subClass(es)Of` `building:Floor`." ;
    rdfs:subClassOf building:ClassOfFloor .

# building:FloorOfAStructureUnit a rdfs:Class ;
#     rdfs:label "The floor of a structure unit"@en-gb ;
#     building:eachIsPartOf building:StructureUnitState ;
#     rdfs:comment "A `building:ClassOfFloor` whose elements are the parts of the `building:Floor`s which bound all the `building:PhysicallyBoundedSpaces`s of a `building:StructureUnit`." ;
#     rdfs:subClassOf building:ClassOfFloor .

building:FloorState a rdfs:Class ;
    rdfs:label "Floor State"@en ;
    rdfs:comment "The temporal State of a `building:Floor`." ;
    ies:powertype building:ClassOfFloorState ;
    rdfs:subClassOf building:BuiltEntityState .

building:GlazingType a rdfs:Class ;
    rdfs:label "Window By Glazing Type"@en-gb ;
    rdfs:comment "A `building:ClassOfWindow` that classifies of `building:Window` by glazing type.  instances of this class are `rdfs:subClass(es)Of` `building:Window`." ;
    rdfs:subClassOf building:ClassOfWindow .

building:IndividualDocumentState a rdfs:Class ;
    rdfs:label "Individual Document State"@en-gb ;
    ies:powertype building:ClassOfIndividualDocumentState ;
    rdfs:comment "An `ies:AssetState` that is a temporal state of a `ies:IndividualDocument`." ;
    rdfs:subClassOf ies:AssetState .

building:LevelInStructure a rdfs:Class ;
    rdfs:label "Level In Structure"@en-gb ;
    rdfs:comment "An `ies:GeoIdentity` used to identify the level of a `building:Storey` in a `building:Structure`." ;
    rdfs:subClassOf ies:GeoIdentity .

building:FunctionalClassOfStructureUnitState a rdfs:Class ;
    rdfs:label "Main Purpose Of Use"@en-gb ;
    rdfs:comment "A `building:ClassOfStructureUnitState` that is a classifier of `building:StructureUnitState` that defines the main purpose for which a `building:StructureUnit` is being used.  Instance of this class are `building:StructureUnitState`s." ;
    rdfs:subClassOf building:ClassOfStructureUnitState .

building:MeasureOfTheEnvironment a rdfs:Class ;
    rdfs:label "Measure Of The Environment"@en-gb ;
    rdfs:comment "An `ies:Measure` that is the state of the environment or the impact of human activity on the environment." ;
    rdfs:subClassOf ies:Measure .

building:NormalCalendarYear a rdfs:Class ;
    rdfs:label "Normal Calendar Year"@en-gb ;
    rdfs:comment "An `ies:Duration` that is 365 days long" ;
    rdfs:subClassOf ies:Duration .

building:PhysicallyBoundedSpace a rdfs:Class ;
    rdfs:label "Physically Bounded Space"@en-gb ;
    rdfs:comment "A `building:Space` that has physical boundaries.  Usually, in the form of Walls, Roof, and Floor." ;
    rdfs:subClassOf building:Space .

building:InteriorOfAStructureUnit a rdfs:Class ;
    rdfs:label "Interior Of A Structure Unit"@en-gb ;
    rdfs:comment "A `building:PhysicallyBoundedSpace` that is the complete interior space of some `building:StructureUnit`." ;
    ies:eachMemberIsPartOfSomeMemberOf building:StructureUnit;
    rdfs:subClassOf building:PhysicallyBoundedSpace .

building:Roof a rdfs:Class ;
    rdfs:label "Roof"@en ;
    ies:powertype building:ClassOfRoof ;
    rdfs:comment """A `building:BuiltEntity` that is the uppermost part of a `building:StructureOrStructureUnit` that provides protection against weather elements such as rain, snow, sunlight, and wind. It serves as a barrier between the interior of the `building:Structure` and the external environment, contributing to the structural integrity, thermal insulation, and aesthetic appearance.  In the case of a `building:StructureUnit`, it may only separate from the `building:StructureUnit` above.""" ;
    rdfs:seeAlso <https://search.bsdd.buildingsmart.org/uri/buildingsmart/ifc/4.3/class/IfcCoveringROOFING>,
        <https://search.bsdd.buildingsmart.org/uri/buildingsmart/ifc/4.3/class/IfcSlabROOF> ;
    rdfs:subClassOf building:BuiltEntity,
        building:RoofState .

building:RoofConstruction a rdfs:Class ;
    rdfs:label "Roof By Construction"@en ;
    rdfs:comment "A `building:ClassOfRoof` that is a classifier of `building:Roof` by the construction methods used.  Instances of this class are `rdfs:subClass(es)Of` `building:Roof`." ;
    rdfs:subClassOf building:ClassOfRoof .

building:RoofInsulationLocation a rdfs:Class ;
    rdfs:label "Roof By Insulation Location"@en-gb ;
    rdfs:comment "A `building:ClassOfRoof` that is a classifier of `building:Roof` by the location of the insulation. Instances of this class are `rdfs:subClass(es)Of` `building:Roof`." ;
    rdfs:subClassOf building:ClassOfRoof .

building:RoofInsulationThickness a rdfs:Class ;
    rdfs:label "Roof By Insulation Thickness"@en-gb ;
    rdfs:comment "A `building:ClassOfRoof` that is a classifier of `building:Roof` by the thickness of the insulation used. Instances of this class are `rdfs:subClass(es)Of` `building:Roof`." ;
    rdfs:subClassOf building:ClassOfRoof .

building:RoofState a rdfs:Class ;
    rdfs:label "Roof State"@en ;
    ies:powertype building:ClassOfRoofState ;
    rdfs:comment "A `building:BuiltEntityState` that is the temporal state of the `building:BuiltEntity`." ;
    rdfs:subClassOf building:BuiltEntityState .

building:EnvironmentalImpactRating a rdfs:Class ;
    rdfs:label "Environmental Impact Rating"@en-gb ;
    rdfs:comment "A `building:ClassOfStructureUnitState` that is a classifier `building:StructureUnitState` by the 'building:EnvironmentalImpactValue'" ;
    rdfs:subClassOf building:ClassOfStructureUnitState .

building:SAPRating a rdfs:Class ;
    rdfs:label "SAPRating"@en-gb ;
    rdfs:comment "A `building:ClassOfStructureUnitState`.  The Standard Assessment Procedure (SAP) rating is a numerical measure used in the United Kingdom to assess and communicate the energy efficiency and environmental performance of residential buildings. It takes into account factors like insulation, heating systems, ventilation, and renewable energy sources to determine a building's energy efficiency. The higher the SAP rating, the more energy-efficient the building is, with the aim of reducing carbon emissions and promoting sustainable construction practices." ;
    rdfs:subClassOf  building:ClassOfStructureUnitState . # building:MeasureOfTheEnvironment .

building:SAPRatingValue a rdfs:Class ;
    rdfs:label "SAP Rating Value"@en-gb ;
    rdfs:comment "A `building:MeasureOfTheEnvironment` that is the result SAP Rating Calculation" ;
    skos:altLabel "Current SAP Score"@en-gb ;
    rdfs:subClassOf building:MeasureOfTheEnvironment .

building:SAPRatingCalculation a rdfs:Class ;
    rdfs:label "SAP Rating Calculation"@en-gb ;
    rdfs:comment "An `ies:Assessment` that is the calculation of the SAP Rating based on details provide during the `building:EPCAssessment`." ;
    rdfs:subClassOf building:EnergyPerformanceAssessment .

building:isBoundedBy a owl:ObjectProperty ;
    rdfs:label "is bounded by"@en-gb ;
    rdfs:comment "A relationship that obtains between an instance of `building:PhysicallyBoundedSpace` and `building:BuiltEntitySection` in which they enclose the `building:PhysicallyBoundedSpace`." ;
    rdfs:domain building:PhysicallyBoundedSpace ;
    rdfs:range building:BuiltEntitySection .

building:Space a rdfs:Class ;
    rdfs:label "Space"@en-gb ;
    ies:powertype building:ClassOfSpace ;
    rdfs:comment "An `ies:Entity` that is a volume or area bounded some `building:WallSection`, `building:FloorSection`, or `building:RoofSection`. 'Space' is a common term in architecture." ;
    rdfs:seeAlso <https://search.bsdd.buildingsmart.org/uri/buildingsmart/ifc/4.3/class/IfcSpace> ;
    rdfs:subClassOf building:SpaceState,
        ies:Entity ,
        building:StructureUnitOrSpace .

building:Room a rdfs:Class ;
    rdfs:label "Room" ;
    rdfs:comment "A `building:Space` that is an enclosed area within a building, typically bounded by walls, floor, and ceiling, and designated for a specific function such as sleeping, cooking, or working." ;
    rdfs:subClassOf building:Space, building:RoomState .

building:RoomState a rdfs:Class ;
    rdfs:label "Room State" ;
    rdfs:comment "An `building:SpaceState` that is the temporal state of a building:Room." ;
    rdfs:subClassOf building:SpaceState .

building:SpaceState a rdfs:Class ;
    rdfs:label "Space State"@en-gb ;
    ies:powertype building:ClassOfSpaceState ;
    rdfs:comment "An `ies:State` that is the temporal state of `building:Space`." ;
    rdfs:subClassOf ies:State .

building:StructureUnitOrSpace a rdfs:Class ;
    rdfs:label "Structure Unit Or Space"@en-gb ;
    ies:powertype building:ClassOfStructureUnitOrSpace ;
    rdfs:comment "An `ies:Entity` that is either a `building:Space` or a `building:StructureUnit`." ;
    rdfs:seeAlso <https://search.bsdd.buildingsmart.org/uri/buildingsmart/ifc/4.3/class/IfcSpace> ;
    rdfs:subClassOf ies:Entity,
        building:StructureUnitOrSpaceState .

building:StructureUnitOrSpaceState a rdfs:Class ;
    rdfs:label "Structure Unit Or Space State"@en-gb ;
    ies:powertype building:ClassOfSpaceState ;
    rdfs:comment "An `ies:State` that is the temporal state of `building:StructureUnitOrSpace`." ;
    rdfs:subClassOf ies:State .

building:Storey a rdfs:Class ;
    rdfs:label "Storey"@en ;
    ies:eachMemberHasPartSomeMemberOf building:Space;
    ies:eachMemberIsPartOfSomeMemberOf building:StructureState;
    ies:powertype building:ClassOfStorey ;
    rdfs:comment "An `ies:Entity` that is a (primarily) horizontal aggregation of `building:Space`s, vertically delimited by structural boundaries such as floors and ceilings."@en ;
    rdfs:seeAlso <https://identifier.buildingsmart.org/uri/buildingsmart/ifc/4.3/class/IfcBuildingStorey> ;
    rdfs:subClassOf building:StoreyState,
        ies:Entity .

building:Basement a rdfs:Class ;
    rdfs:label "Basement" ;
    rdfs:comment "A `building:Storey` that is part of a `building:Structure` and below ground level." ;
    rdfs:subClassOf building:Storey, building:BasementState .

building:BasementState a rdfs:Class ;
    rdfs:comment "A `building:StoreyState` that is the temporal state of a `building:Basement`" ;
    rdfs:label "Basement State" ;
    rdfs:subClassOf building:StoreyState .

building:StoreyState a rdfs:Class ;
    rdfs:label "Storey State"@en ;
    ies:powertype building:ClassOfStoreyState ;
    rdfs:comment "An `ies:State` that is the temporal State of a Storey." ;
    rdfs:subClassOf ies:State .

building:Structure a rdfs:Class ;
    rdfs:label "Structure"@en-gb ;
    ies:powertype building:ClassOfStructure ;
    rdfs:comment "An `ies:Entity` that is human-made, has a defined shape and stability and is meant to protect a region of space from atmospheric agents; a structure can exist in different states over time.  The `building:Space` that is enclosed by a structure is often divided into smaller `building:Space`s by various arrangement of `building:BuiltElements`." ;
    rdfs:subClassOf building:StructureState,
        ies:Entity .

building:StructureState a rdfs:Class ;
    rdfs:label "Structure State"@en-gb ;
    ies:powertype building:ClassOfStructureState ;
    rdfs:comment "An `ies:State` that is the temporal state of a `building:Structure`." ;
    rdfs:subClassOf ies:State .

building:StructureUnitType a rdfs:Class ;
    rdfs:label "Structure Unit Type"@en-gb ;
    rdfs:comment "A `building:ClassOfStructureUnit` that is a classifier of `building:StructureUnitState` that defines the type of the `building:StructureUnit`." ;
    rdfs:subClassOf building:ClassOfStructureUnitState .

building:StructureUnit a rdfs:Class ;
    rdfs:label "Structure Unit (Collection of building:Space)"@en-gb ;
    ies:eachMemberHasPartSomeMemberOf building:Space;
    ies:eachMemberIsPartOfSomeMemberOf building:StructureState;
    ies:powertype building:ClassOfStructureUnit ;
    rdfs:comment "An `ies:Asset` that is the mereological sum of `building:Space`(s) meaning, a `building:StructureUnit` consists of `building:Space`s and the parts of those `building:Spaces`.  A unit typically may have shared or auxiliary spaces that support the primary function of the unit." ;
    rdfs:subClassOf building:StructureUnitState,
        ies:Asset, building:StructureUnitOrSpace .

building:StructureUnitState a rdfs:Class ;
    rdfs:label "Structure Unit State"@en-gb ;
    rdfs:comment "An ies:State` that is the temporal state of `building:StructureUnit`" ;
   ies:powertype building:ClassOfStructureUnitState ;
    rdfs:subClassOf ies:State, building:StructureUnitOrSpaceState .

building:UDPRN a rdfs:Class ;
    rdfs:label "UDPRN"@en-gb ;
    rdfs:comment "An `ies:GeoIdentity` that is the UK Royal Mail’s Unique Delivery Point Reference Number (UDPRN)." ;
    rdfs:subClassOf ies:GeoIdentity .

building:UKDomesticEPC a rdfs:Class ;
    rdfs:label "UK Domestic EPC"@en-gb ;
    rdfs:comment "A `building:UK_EPC` that is for residential properties. If someone is selling or renting out a home, they'll need a Domestic EPC for potential buyers or tenants to view." ;
    rdfs:subClassOf building:UK_EPC .

building:UKNonDomesticEPC a rdfs:Class ;
    rdfs:label "UK Non-Domestic EPC"@en-gb ;
    rdfs:comment "A `building:UK_EPC` that is for commercial properties, such as offices, shops, or industrial buildings. If a commercial property is being sold, rented, or built, a Non-Domestic EPC is usually required." ;
    rdfs:subClassOf building:UK_EPC .

building:UK_DOM_EPC_G a building:UKDomesticEPC ;
    ies:representationValue "G" ;
    rdfs:label "UK Domestic EPC G" ;
    rdfs:comment "A `building:UKDomesticEPC` that is the result of a `building:EPCAssessment` assessed as grade G, corresponding to a `building:SAPRating` of between 1 and 20.  " ;
    rdfs:subClassOf ies:IndividualDocument .

building:UK_DOM_EPC_F a building:UKDomesticEPC ;
    rdfs:label "UK Domestic EPC F" ;
    ies:representationValue "F" ;
    rdfs:comment "A `building:UKDomesticEPC` that is the result of a `building:EPCAssessment` assessed as grade F, corresponding to a `building:SAPRating` of between 21 and 38.  " ;
    rdfs:subClassOf ies:IndividualDocument .

building:UK_DOM_EPC_E a building:UKDomesticEPC ;
    rdfs:label "UK Domestic EPC E" ;
    ies:representationValue "E" ;
    rdfs:comment "A `building:UKDomesticEPC` that is the result of a `building:EPCAssessment` assessed as grade E, corresponding to a `building:SAPRating` of between 39 and 54." ;
    rdfs:subClassOf ies:IndividualDocument .

building:UK_DOM_EPC_A a building:UKDomesticEPC ;
    rdfs:label "UK Domestic EPC A" ;
    ies:representationValue "A" ;
    rdfs:comment "A `building:UKDomesticEPC` that is the result of a `building:EPCAssessment` assessed as grade A, corresponding to a `building:SAPRating` of between 92 and 100.  " ;
    rdfs:subClassOf ies:IndividualDocument .

building:UK_DOM_EPC_B a building:UKDomesticEPC ;
    rdfs:label "UK Domestic EPC B" ;
    ies:representationValue "B" ;
    rdfs:comment "A `building:UKDomesticEPC` that is the result of a `building:EPCAssessment` assessed as grade B, corresponding to a `building:SAPRating` of between 81 and 91.  " ;
    rdfs:subClassOf ies:IndividualDocument .

building:UK_DOM_EPC_C a building:UKDomesticEPC ;
    rdfs:label "UK Domestic EPC C" ;
    ies:representationValue "C" ;
    rdfs:comment "A `building:UKDomesticEPC` that is the result of a `building:EPCAssessment` assessed as grade C, corresponding to a `building:SAPRating` of between 69 and 80.  " ;
    rdfs:subClassOf ies:IndividualDocument .

building:UK_DOM_EPC_D a building:UKDomesticEPC ;
    rdfs:label "UK Domestic EPC D" ;
    ies:representationValue "D" ;
    rdfs:comment "A `building:UKDomesticEPC` that is the result of a `building:EPCAssessment` assessed as grade D, corresponding to a `building:SAPRating` of between 55 and 68.  " ;
    rdfs:subClassOf ies:IndividualDocument .

building:UK_EPC a rdfs:Class ;
    rdfs:label "UK Energy Performance Certificate"@en-gb ;
    rdfs:comment "A `building:EnergyPerformanceCertificate` that is a document in the UK that provides information about a property's energy use and typical energy costs. It also offers recommendations on how to reduce energy and save money. Properties are rated on a scale from A (most efficient) to G (least efficient), and the certificate is required when selling or renting a property.  Since the same methodologies (SAP and RdSAP) are used, the EPC ratings and values assigned are comparable across all home nations. This means an EPC rating of 'A' in England represents the same level of energy efficiency as an 'A' rating in Scotland, Wales, or Northern Ireland." ;
    rdfs:subClassOf building:EnergyPerformanceCertificate ;
    skos:note "The same methodologies (SAP and RdSAP) are used across the UK, the EPC ratings and values assigned are comparable." .

building:UK_EPC_Identifier a rdfs:Class ;
    rdfs:label "UK EPC Identifier"@en-gb ;
    rdfs:comment "A `ies:Identifier` that is used to identify a `building:UK_EPC`" ;
    rdfs:subClassOf ies:Identifier .

building:UPRN a rdfs:Class ;
    rdfs:label "UPRN"@en-gb ;
    rdfs:comment "An `ies: GeoIdentity` that is a unique numeric identifier for every addressable location in Great Britain. The UPRN is the persistent identifier providing consistency across the AddressBase product range. Each address record has a UPRN, assigned by Local Authorities in England, Wales and Scotland or Ordnance Survey depending on the type of address. This is the primary key of the AddressBase product. Throughout its lifecycle, information on the address of a property can change. This may be due to a change of name, change of use, or the eventual demolition of the property. Independent of any changes being made the UPRN associated to an address is never changed, meaning the unique identifier remains persistent and reliable" ;
    rdfs:subClassOf ies:GeoIdentity ;
    skos:note """UPRN can regarded an identifier of a whole-life Entity.
    'UPRNs provide every property or object with a unique identifier
    throughout its lifecycle, from planning through to demolition.'""" ;
    skos:seeAlso <https://www.geoplace.co.uk/blog/2020/so-what-are-these-uprns-and-usrns-that-everyone-is-talking-about> .

building:OSID a rdfs:Class ;
    rdfs:label "OSID" ;
    rdfs:comment "An `ies:GeoIdentity` that is the persistent unique identifier assigned by Ordnance Survey UK to a real-world geographic feature within its authoritative datasets, such as the OS MasterMap Topography Layer. An OSID enables the consistent referencing of a feature over time, even if its geometry or attributes change. It is assigned when the feature is first captured in the dataset and remains in place until the feature is removed." ;
    rdfs:subClassOf ies:GeoIdentity ;
    skos:note """OSIDs are used internally within Ordnance Survey products and APIs to ensure consistency across dataset updates.
    While some OSIDs appear in open datasets (such as certain linked data resources), many originate from licensed datasets like OS MasterMap and are not directly searchable in public web maps.""" ;
    skos:seeAlso <https://www.ordnancesurvey.co.uk/products/mastermap-topography> .

building:Wall a rdfs:Class ;
    rdfs:label "Wall"@en ;
    ies:powertype building:ClassOfWall ;
    rdfs:comment """A `building:BuiltEntity` that is a vertically orient element that defines and encloses spaces within a building, providing support, shelter, and separation. Walls can be load-bearing, contributing to the structural integrity of the building, or non-load-bearing, primarily serving to divide interior spaces.  While openings (e.g., doors, windows) modify the geometry of a wall, they do not inherently divide it into separate entities unless the sections on either side of the opening are structurally, functionally, or materially distinct.""" ;
    skos:example """
    A Long Facade Wall With Windows:

    A 20m-long external wall contains 5 windows, is still one wall because:
	  •	The material, structure, and function are consistent throughout.
	  •	The windows are just modifications (openings) in the wall’s geometry.
    """ ;
    skos:example """
    A Wall with a Large Sliding Door:

    An internal partition wall contains a large sliding door opening (e.g., 4m wide), is still one wall unless:
	  •	The sections on either side of the opening are made of different materials (e.g., drywall on one side, glass on the other).
	  •	The wall is structurally independent on either side of the opening.
    """ ;
    skos:example """
    """ ;
    skos:note "Treat walls as divided only when there’s a clear structural, functional, or material reason." ;
    rdfs:seeAlso <https://search.bsdd.buildingsmart.org/uri/buildingsmart/ifc/4.3/class/IfcWall> ;
    rdfs:subClassOf building:BuiltEntity,
        building:WallState .

building:BuiltEntitySection a rdfs:Class ;
    rdfs:comment "A `building:BuiltEntity that is a section of `building:Wall` contained within a boundary, according to some coordinate reference system. A `building:BuiltEntitySection` is part of the `building:BuiltEntity` and may be distinguished based on geometry, material, or function, but remains part of the overall `building:BuiltEntity`." ;
    rdfs:label "Built Entity Section"@en-gb ;
    ies:eachMemberIsPartOfSomeMemberOf building:BuiltEntity;
    rdfs:subClassOf building:BuiltEntity, building:BuiltEntitySectionState .

building:BuiltEntitySectionState a rdfs:Class ;
    rdfs:label "Wall Section State"@en-gb ;
    rdfs:comment "A `building:BuiltEntityState` that is the state of the `building:BuiltEntitySection` from time to time." ;
    rdfs:subClassOf building:BuiltEntityState .

building:WallSection a rdfs:Class ;
    rdfs:comment "A `building:BuiltEntity that is a section of `building:Wall` contained within a boundary, according to some coordinate reference system. A `building:WallSection` is part of the `building:Wall` and may be distinguished based on geometry, material, or function, but remains part of the overall `building:Wall`." ;
    rdfs:label "Wall Section"@en-gb ;
    ies:powertype building:ClassOfWallSection ;
    rdfs:subClassOf building:BuiltEntitySection, building:WallSectionState .

building:ClassOfWallSection a rdfs:Class ;
    rdfs:comment "A `building:ClassOfBuiltEntity` that classifies `building:WallSection`.  Instances of this class are `rdfs:subClassOf` `building:WallSection` " ;
    rdfs:label "Class Of Wall Section"@en-gb ;
    rdfs:subClassOf building:ClassOfBuiltEntity .

building:WallSectionState a rdfs:Class ;
    rdfs:label "Wall Section State"@en-gb ;
    rdfs:comment "A `building:BuiltEntityState` that is the state of the `building:WallSection` from time to time." ;
    ies:powertype building:ClassOfWallSectionState ;
    rdfs:subClassOf building:BuiltEntitySectionState .

building:ClassOfWallSectionState a rdfs:Class ;
    rdfs:comment "A `building:ClassOfBuiltEntity` that classifies `building:WallSectionState`.  Instances of this class are `rdfs:subClassOf` `building:WallSectionState` " ;
    rdfs:label "Class Of Wall Section State"@en-gb ;
    rdfs:subClassOf building:ClassOfBuiltEntity .

building:FloorSection a rdfs:Class ;
    rdfs:comment "A `building:BuiltEntity that is a section of `building:Floor` contained within a boundary, according to some coordinate reference system. A `building:FloorSection` is part of the `building:Floor` and may be distinguished based on geometry, material, or function, but remains part of the overall `building:Floor`." ;
    rdfs:label "Floor Section"@en-gb ;
    ies:powertype building:ClassOfFloorSection ;
    rdfs:subClassOf building:BuiltEntitySection, building:FloorSectionState .

building:FloorSectionState a rdfs:Class ;
    rdfs:label "Floor Section State"@en-gb ;
    rdfs:comment "A `building:BuiltEntityState` that is the state of the `building:FloorSection` from time to time." ;
    rdfs:subClassOf building:BuiltEntityState .

building:RoofSection a rdfs:Class ;
    rdfs:comment "A `building:BuiltEntity that is a section of `building:Roof` contained within a boundary, according to some coordinate reference system. A `building:RoofSection` is part of the `building:Roof` and may be distinguished based on geometry, material, or function, but remains part of the overall `building:Roof`." ;
    rdfs:label "Roof Section"@en-gb ;
    ies:powertype building:ClassOfRoofSection ;
    rdfs:subClassOf building:BuiltEntitySection, building:RoofSectionState .

building:ClassOfRoofSection a rdfs:Class ;
    rdfs:comment "A `building:ClassOfBuiltEntity` that classifies `building:RoofSection`.  Instances of this class are `rdfs:subClassOf` `building:RoofSection` " ;
    rdfs:label "Class Of Roof Section"@en-gb ;
    rdfs:subClassOf building:ClassOfBuiltEntity .

building:RoofSectionState a rdfs:Class ;
    rdfs:label "Roof Section State"@en-gb ;
    rdfs:comment "A `building:BuiltEntityState` that is the state of the `building:RoofSection` from time to time." ;
    rdfs:subClassOf building:BuiltEntitySectionState .

building:ClassOfRoofSectionState a rdfs:Class ;
    rdfs:comment "A `building:ClassOfBuiltEntityState` that classifies `building:RoofSectionState`.  Instances of this class are `rdfs:subClassOf` `building:RoofSectionState` " ;
    rdfs:label "Class Of Roof Section"@en-gb ;
    rdfs:subClassOf building:ClassOfBuiltEntityState .

building:ClassOfClassOfRoofSectionState a rdfs:Class ;
    rdfs:comment "A `building:ClassOfClassOfBuiltEntityState` that classifies `building:ClassOfRoofSectionState`.  Instances of this class are `rdfs:subClassOf` `building:ClassOfRoofSectionState` " ;
    rdfs:label "Class Of Class Of Roof Section" ;
    rdfs:subClassOf building:ClassOfClassOfBuiltEntityState .

building:WallConstruction a rdfs:Class ;
    rdfs:label "Wall By Construction"@en ;
    rdfs:comment "A `building:ClassOfWall` that is a classifier of `building:Wall` by construction method.  Instances of this class are `rdfs:subClass(es)Of` `building:Wall`." ;
    rdfs:subClassOf building:ClassOfWall .

building:WallInsulation a rdfs:Class ;
    rdfs:label "Wall By Insulation"@en ;
    rdfs:comment "A `building:ClassOfWall` that is a classifier of `building:Wall` by insulation.  Instances of this class are `rdfs:subClass(es)Of` `building:Wall`." ;
    rdfs:subClassOf building:ClassOfWall .

building:WallState a rdfs:Class ;
    rdfs:label "Wall State"@en ;
    ies:powertype building:ClassOfWallState ;
    rdfs:comment "A `building:BuiltEntityState` that is the temporal State of a `building:Wall`." ;
    rdfs:subClassOf building:BuiltEntityState .

building:Window a rdfs:Class ;
    rdfs:label "Window"@en ;
    ies:powertype building:ClassOfWindow ;
    rdfs:comment "A `building:BuiltEntity` that allows the passage of light, air, and sound into a space while providing a view to the outside, often framed and made from transparent or translucent materials such as glass, and designed to be opened or closed to control ventilation and maintain environmental comfort." ;
    rdfs:seeAlso <https://search.bsdd.buildingsmart.org/uri/buildingsmart/ifc/4.3/class/IfcWindow> ;
    rdfs:subClassOf building:BuiltEntity,
        building:WindowState .

building:WindowState a rdfs:Class ;
    rdfs:label "Window State"@en ;
    ies:powertype building:ClassOfWindowState ;
    rdfs:comment "A `building:BuiltEntityState` that is the temporal State of a `building:Window`." ;
    rdfs:subClassOf building:BuiltEntityState .

building:0mm_Insulation a building:RoofInsulationThickness ;
    rdfs:label "0mm Insulation"@en-gb ;
    rdfs:comment "An instance of `building:RoofInsulationThickness` that meets a specification of 0mm thickness" .

building:100mm_Insulation a building:RoofInsulationThickness ;
    rdfs:label "100mm Insulation"@en-gb ;
    rdfs:comment "An instance of `building:RoofInsulationThickness` that meets a specification of 100mm" .

building:12mm_Insulation a building:RoofInsulationThickness ;
    rdfs:label "12mm Insulation"@en-gb ;
    rdfs:comment "An instance of `building:RoofInsulationThickness` that meets a specification of 12mm" .

building:150mm_Insulation a building:RoofInsulationThickness ;
    rdfs:label "150mm Insulation"@en-gb ;
    rdfs:comment "An instance of `building:RoofInsulationThickness` that meets a specification of 150mm" .

building:200mm_Insulation a building:RoofInsulationThickness ;
    rdfs:label "200mm Insulation"@en-gb ;
    rdfs:comment "An instance of `building:RoofInsulationThickness` that meets a specification of 200mm" .

building:250mm_Insulation a building:RoofInsulationThickness ;
    rdfs:label "250mm Insulation"@en-gb ;
    rdfs:comment "An instance of `building:RoofInsulationThickness` that meets a specification of 250mm" .

building:25mm_Insulation a building:RoofInsulationThickness ;
    rdfs:label "25mm Insulation"@en-gb ;
    rdfs:comment "An instance of `building:RoofInsulationThickness` that meets a specification of 25mm" .

building:270mm_Insulation a building:RoofInsulationThickness ;
    rdfs:label "270mm Insulation"@en-gb ;
    rdfs:comment "An instance of `building:RoofInsulationThickness` that meets a specification of 270mm" .

building:300mm_Insulation a building:RoofInsulationThickness ;
    rdfs:label "300mm Insulation"@en-gb ;
    rdfs:comment "An instance of `building:RoofInsulationThickness` that meets a specification of 300mm" .

building:350mm_Insulation a building:RoofInsulationThickness ;
    rdfs:label "350mm Insulation"@en-gb ;
    rdfs:comment "An instance of `building:RoofInsulationThickness` that meets a specification of 350mm" .

building:400mm_Insulation a building:RoofInsulationThickness ;
    rdfs:label "400mm Insulation"@en-gb ;
    rdfs:comment "An instance of `building:RoofInsulationThickness` that meets a specification of 400mm" .

building:50mm_Insulation a building:RoofInsulationThickness ;
    rdfs:label "50mm Insulation"@en-gb ;
    rdfs:comment "An instance of `building:RoofInsulationThickness` that meets a specification of 50mm" .

building:75mm_Insulation a building:RoofInsulationThickness ;
    rdfs:label "75mm Insulation"@en-gb ;
    rdfs:comment "An instance of `building:RoofInsulationThickness` that meets a specification of 75mm" .

building:AnotherDwellingAbove a building:RoofConstruction ;
    rdfs:label "Another Dwelling Above"@en-gb ;
    rdfs:comment "An instance of `building:RoofConstruction` indicating that the roof is in fact another dwelling on the level above." .

building:AnotherDwellingBelow a building:FloorConstruction ;
    rdfs:label "Another Dwelling Below"@en-gb ;
    rdfs:comment "An instance of `building:FloorConstruction` indicating that the floor is in fact another dwelling on the level below." .

building:ToExternalAir a building:FloorConstruction ;
    rdfs:label "To External Air" ;
    rdfs:comment "An instance of `building:FloorConstruction` where the floor is directly exposed to the external environment." .

building:ToUnheatedSpace a building:FloorConstruction ;
    rdfs:label "To Unheated Space" ;
    rdfs:comment "An instance of `building:FloorConstruction` where the floor is above an unheated space, such as a garage or cellar." .

building:Bungalow a building:StructureUnitType ;
    rdfs:label "Bungalow"@en-gb ;
    rdfs:comment "An instance of `building:StructureUnitType` that is a type of low-rise residential building, typically consisting of a single story or a partial second story built into a sloped roof. Bungalows are characterised by their compact layout, often featuring a broad, covered porch, wide eaves, and a low-pitched roof." ;
    rdfs:subClassOf building:House .

building:CavityWall a building:WallConstruction ;
    rdfs:label "Cavity Wall"@en-gb ;
    rdfs:comment "An instance of `building:WallConstruction` that consists of two parallel walls, or \"leaves,\" separated by a cavity or gap. This gap, or cavity, is usually filled with insulating material and serves to reduce heat transfer through the wall, improve thermal insulation, and prevent moisture penetration." .

building:CeilingInsulated a building:RoofInsulationLocation ;
    rdfs:label "Ceiling Insulated"@en-gb ;
    rdfs:comment "An instance of `building:RoofInsulationLocation` where the `building:Roof` has insulation in the ceiling." .

building:AdditionalRoofInsulation a building:RoofInsulation ;
    rdfs:label "Additional Roof Insulation" ;
    rdfs:comment "An instance of `building:RoofInsulation` representing additional insulation applied to the roof." .

building:Cob a building:WallConstruction ;
    rdfs:label "Cob"@en-gb ;
    rdfs:comment "An instance of `building:WallConstruction` that is a type of wall construction made from a natural building material composed of subsoil, water, fibrous organic material (typically straw), and sometimes lime. Cob is a traditional building method, particularly common in regions with suitable soil, and is known for its durability, thermal mass, and ability to regulate humidity." .

building:StoneOrLimestone a building:WallConstruction ;
    rdfs:label "Stone or Limestone" ;
    rdfs:comment "An instance of `building:WallConstruction` that is a type of wall construction made from natural stone, such as limestone, arranged and bonded together with mortar or other binding materials. This method is valued for its durability, thermal mass, and aesthetic qualities, and is commonly found in traditional and historic buildings." .

building:Commercial a building:FunctionalClassOfStructureUnitState ;
    rdfs:label "Commercial"@en-gb ;
    rdfs:comment "An instance of `building:FunctionalClassOfStructureUnitState` that states that the `building:StructureUnit` is used for business or commercial activities." ;
    rdfs:subClassOf building:StructureUnitState .

building:Detached a building:BuiltForm ;
    rdfs:label "Detached"@en-gb ;
    rdfs:comment "An instance of `building:BuiltForm` that is a standalone residential building that is not attached to any other building or structure. It is typically designed for a single family, offering privacy and exclusive use of the surrounding land, which may include a garden, driveway, or garage. " ;
    rdfs:subClassOf building:StructureUnitState .

building:DomesticEnergyRelatedCosts a rdfs:Class ;
    rdfs:label "Domestic Energy Related Costs"@en-gb ;
    rdfs:comment "A `building:CostEstimate` that is an estimate of the energy-related costs for a domestic `building:StructureUnit`." ;
    rdfs:subClassOf building:CostEstimate .

building:DomesticHeatingCostEstimate a building:DomesticEnergyRelatedCosts ;
    rdfs:label "Domestic Heating Cost Estimate"@en-gb ;
    rdfs:comment "A `building:CostEstimate` that is an estimate of the cost of heating a domestic `building:StructureUnit`." ;
    rdfs:subClassOf building:CostEstimate .

building:DomesticLightingCostEstimate a building:DomesticEnergyRelatedCosts ;
    rdfs:label "Domestic Lighting Cost Estimate"@en-gb ;
    rdfs:comment "A `building:CostEstimate` that is an estimate of the cost of lighting a domestic `building:StructureUnit`." ;
    rdfs:subClassOf building:CostEstimate .

building:DomesticWaterHeatingCostEstimate a building:DomesticEnergyRelatedCosts ;
    rdfs:label "Domestic Water Heating Cost Estimate"@en-gb ;
    rdfs:comment "A `building:CostEstimate` that is an estimate of the cost of heating the water supply of a domestic `building:StructureUnit`." ;
    rdfs:subClassOf building:CostEstimate .

building:DoubleGlazing a building:GlazingType ;
    rdfs:label "Double Glazing" ;
    rdfs:comment "An instance of `building:GlazingType` that uses two panes of glass separated by a gap, usually filled with air or inert gas, to improve thermal insulation, reduce noise, and enhance energy efficiency.  " ;
    rdfs:subClassOf building:MultipleGlazing .

building:MultipleGlazing a building:GlazingType ;
    rdfs:label "Multiple Glazing";
    rdfs:comment "An instance of `building:GlazingType` that that consists of more than one pane of glass, such as double or triple glazing, to improve thermal insulation." ;
    rdfs:subClassOf building:Window .

building:DoubleGlazingAfter2002 a building:GlazingType ;
    rdfs:label "Double Glazing After2002" ;
    rdfs:comment "An instance of `building:GlazingType` that was manufactured after 2002.  In 2002 the UK, the government introduced changes to the Building Regulations, specifically Part L, which focused on energy conservation. These changes required that new or replacement windows (including double glazing) meet higher standards for thermal insulation." ;
    rdfs:subClassOf building:MultipleGlazing .

building:DoubleGlazingBefore2002 a building:GlazingType ;
    rdfs:label "Double Glazing Before2002" ;
    rdfs:comment "An instance of `building:GlazingType` that was manufactured before 2002. In 2002 the UK, the government introduced changes to the Building Regulations, specifically Part L, which focused on energy conservation. These changes required that new or replacement windows (including double glazing) meet higher standards for thermal insulation." ;
    rdfs:subClassOf building:MultipleGlazing .

building:TerraceHouse a building:BuiltForm ;
    rdfs:label "Terrace House"@en-gb ;
    rdfs:comment "An instance of `building:BuiltForm` that is a `building:StructureUnit` that is part of a continuous row of identical or similar houses, sharing side walls with neighbouring properties. These houses are typically built in a uniform architectural style and are common in densely populated urban areas." ;
    rdfs:subClassOf building:StructureUnitState .

building:EnclosedEndOfTerrace a building:BuiltForm ;
    rdfs:label "Enclosed End Of Terrace"@en-gb ;
    rdfs:comment "An instance of `building:BuiltForm` that is a `building:TerraceHouse` that is at the end of a row, but has two rather than three external walls.  This could be through some addition like a conservatory." ;
    rdfs:subClassOf building:TerraceHouse .

building:EnclosedMidTerrace a building:BuiltForm ;
    rdfs:label "Enclosed Mid Terrace"@en-gb ;
    rdfs:comment "An instance of `building:BuiltForm` that is a `building:TerraceHouse` that is not at the end of a row, but has one rather than two external walls.  This could be through some addition like a conservatory." ;
    rdfs:subClassOf building:TerraceHouse .

building:EndOfTerrace a building:BuiltForm ;
    rdfs:label "End Of Terrace"@en-gb ;
    rdfs:comment "An instance of `building:BuiltForm` that is a `building:TerraceHouse` that is at the end of a row with three external walls." ;
    rdfs:subClassOf building:TerraceHouse .

building:ExternalInsulation a building:WallInsulation ;
    rdfs:label "External Insulation"@en-gb ;
    rdfs:comment "An instance of `building:WallInsulation` that is a layer of insulating material applied to the exterior surface of a building's walls, typically covered with a protective and decorative finish. " .

building:FilledWallCavityInsulation a building:WallInsulation ;
    rdfs:label "Filled Wall Cavity Insulation" ;
    rdfs:comment "An instance of `building:WallInsulation` where the cavity between inner and outer walls is completely filled with insulating material to improve thermal performance." .

building:AdditionalWallInsulation a building:WallInsulation ;
    rdfs:label "Additional Wall Insulation" ;
    rdfs:comment "An instance of `building:WallInsulation` where extra insulating material is added to an existing wall to increase its thermal resistance and energy efficiency." .

building:Flat a building:StructureUnitType ;
    rdfs:label "Flat"@en-gb ;
    rdfs:comment "An instance `building:StructureType` that is a class of self-contained residential `building:StructureUnit` within a larger building, typically consisting of multiple rooms such as a living area, kitchen, bathroom, and one or more bedrooms. " ;
    rdfs:subClassOf building:StructureUnitState .

building:FlatRoof a building:RoofConstruction ;
    rdfs:label "Flat Roof"@en-gb ;
    rdfs:comment "An instance of `building:RoofConstruction` that is a type of roof with a nearly level surface, typically having a slight pitch to allow for water drainage. " .

building:GraniteOrWhinstone a building:WallConstruction ;
    rdfs:label "Granite Or Whinstone"@en-gb ;
    rdfs:comment "An instance of `building:WallConstruction` that is a type of masonry wall constructed using granite blocks or stones. Granite is a hard, durable, and aesthetically appealing igneous rock known for its strength and resistance to weathering. " .

building:House a building:StructureUnitType ;
    rdfs:label "House"@en-gb ;
    rdfs:comment "An instance `building:StructureType` that is a class of self-contained residential `building:StructureUnit` which is a residential building designed primarily for living purposes, typically intended to accommodate a single household or family." ;
    rdfs:subClassOf building:StructureUnitState .

building:Insulated a building:RoofInsulationLocation ;
    rdfs:label "Insulated (Roof)"@en-gb ;
    rdfs:comment "An instance of `building:RoofInsulationLocation` that simply asserts that the `building:Roof` is insulated." .

building:InsulatedAtRafters a building:RoofInsulationLocation ;
    rdfs:label "Insulated At Rafters"@en-gb ;
    rdfs:comment "An instance of `building:RoofInsulationLocation` that asserts that the insulation of the `building:Roof` is in the rafters.  Rafters are structural components of a roof, typically a sloped beam, that extends from the ridge or peak of the roof down to the eaves." .

building:InsulatedFloor a building:FloorInsulation ;
    rdfs:label "Insulated Floor"@en-gb ;
    rdfs:comment "An instance of `building:FloorInsulation` that is the class of `building:Floor` that are insulated." .

building:InsulatedWall a building:WallInsulation ;
    rdfs:label "Insulated Wall"@en-gb ;
    rdfs:comment "An instance of `building:WallInsulation` that is the class of `building:Wall` that are insulated." .
    # rdfs:subClassOf building:Wall .

building:InsulatedWithThatched a building:RoofInsulationLocation ;
    rdfs:label "Insulated With Thatched"@en-gb ;
    rdfs:comment "An instance of `building:RoofInsulationLocation` that is the class of `building:Roof` with a thatch cover.  A thatched roof is a traditional roofing system made from natural materials such as straw, reed, or heather, layered to create a weatherproof covering." .

building:InternalInsulation a building:WallInsulation ;
    rdfs:label "Internal Insulation"@en-gb ;
    rdfs:comment "An instance of `building:WallInsulation` that is the class of `building:Wall` that has internal insulation.  An internally insulated wall is a type of wall construction where insulation is added to the interior side of the wall, typically between the wall's structural elements and the interior finish (such as drywall or plaster). " .

building:LimitedFloorInsulation a building:FloorInsulation ;
    rdfs:label "Limited Floor Insulation"@en-gb ;
    rdfs:comment "An instance of `building:FloorInsulation` that is the class of `building:Floor` with limited insulation." .

building:LimitedInsulation a building:RoofInsulationLocation ;
    rdfs:label "Limited Insulation"@en-gb ;
    rdfs:comment "An instance of `building:RoofInsulationLocation` that is the class of `building:Roof` with limited insulation." .

building:LoftInsulation a building:RoofInsulationLocation ;
    rdfs:label "Loft Insulation" ;
    rdfs:comment "An instance of `building:RoofInsulationLocation` that is the class of `building:Roof` with a loft that is insulated. A loft is a space located directly under the roof of a building, often referred to as an attic or garret." .

building:Maisonette a building:StructureUnitType ;
    rdfs:label "Maisonette"@en-gb ;
    rdfs:comment "An instance of `building:StructureType` that is the class of `StructureUnit`. A maisonette is a self-contained residential `building:StructureUnit` that occupies part of a larger `building:Building` and typically spans two or more floors. Maisonettes often have their own private entrance from the outside, rather than a shared hallway or lobby. It combines elements of both a house and an apartment, often featuring internal stairs and sometimes a small outdoor space like a balcony or garden." ;
    rdfs:subClassOf building:Flat .

building:VentilationSystem a rdfs:Class ;
    rdfs:label "Ventilation System" ;
    rdfs:comment "A `building:TechnicalSystem` that exchanges stale air for fresh air in a `building:Structure` or `building:StructureUnit`." ;
    rdfs:subClassOf building:TechnicalSystem .

building:MechanicalExtractOnly a rdfs:Class ;
    rdfs:label "Mechanical Extract Only"@en-gb ;
    skos:altLabel "MEV"@en-gb ;
    rdfs:comment "A `building:VentilationSystem` that uses mechanical systems to extract air." ;
    rdfs:subClassOf building:VentilationSystem .

building:MechanicalSupplyAndExtract a rdfs:Class ;
    rdfs:label "Mechanical Supply And Extract"@en-gb ;
    rdfs:comment "A `building:VentilationSystem` that both supplies and extracts air through mechanical systems" ;
    rdfs:subClassOf building:VentilationSystem .

building:MidTerrace a building:BuiltForm ;
    rdfs:label "Mid Terrace"@en-gb ;
    rdfs:comment "An instance of `building:BuiltForm` that is a `building:TerraceHouse` that is not at the end of a row, and has two external walls." ;
    rdfs:subClassOf building:TerraceHouse .

building:MoreThan300mm_Insulation a building:RoofInsulationThickness ;
    rdfs:label "More Than300mm_ Insulation"@en-gb ;
    rdfs:comment "An instance of `building:RoofInsulationThickness` that is the class of `building:Roof` with insulation that meets the specification of being thicker than 300mm." .

building:MoreThan400mm_Insulation a building:RoofInsulationThickness ;
    rdfs:label "More Than 400mm Insulation"@en-gb ;
    rdfs:comment "An instance of `building:RoofInsulationThickness` that is the class of `building:Roof` with insulation that meets the specification of being thicker than 300mm." .

building:NaturalVentilation a rdfs:Class ;
    rdfs:label "Natural Ventilation"@en-gb ;
    rdfs:comment "A `building:VentilationSystem` that allows for the natural movement of air." ;
    rdfs:subClassOf building:VentilationSystem .

building:NoInsulationInFloor a building:FloorInsulation ;
    rdfs:label "No Insulation In Floor"@en-gb ;
    rdfs:comment "An instance of `building:FloorInsulation` that is the class of `building:Floor` of `building:StructureUnits` that are not insulated." .

building:NoInsulationInRoof a building:RoofInsulationLocation ;
    rdfs:label "No Insulation In Roof"@en-gb ;
    rdfs:comment "An instance of `building:RoofInsulation` that is the class of `building:Roof` of `building:StructureUnits` that are not insulated." .

building:NoInsulationInWall a building:WallInsulation ;
    rdfs:label "No Insulation In Wall"@en-gb ;
    rdfs:comment "An instance of `building:WallInsulation` that is the class of `building:Wall` of `building:StructureUnits` that are not insulated." .

building:OtherPremisesAbove a building:RoofConstruction ;
    rdfs:label "Other Premises Above"@en-gb ;
    rdfs:comment "An instance of `building:RoofConstruction` that is the class of `building:Roof` consisting of another `building:StructureUnit` above forming the `building:Roof`." .

building:OtherPremisesBelow a building:FloorConstruction ;
    rdfs:label "Other Premises Below"@en-gb ;
    rdfs:comment "An instance of `building:FloorConstruction` that is the class of `building:Floor` consisting of another `building:StructureUnit` below forming the `building:Floor`." .

building:ParkHomeWall a building:WallConstruction ;
    rdfs:label "Park Home Wall"@en-gb ;
    rdfs:comment "An instance of `building:WallConstruction` that is the external wall structure of a park home, which is a type of prefabricated." .

building:PartialInsulation a building:WallInsulation ;
    rdfs:label "Partial Insulation"@en-gb ;
    rdfs:comment "An instance of `building:WallInsulation` that is a class of `building:Wall` that is not insulated in places." .

building:PitchedRoof a building:RoofConstruction ;
    rdfs:label "Pitched Roof"@en-gb ;
    rdfs:comment "An instance of `building:RoofConstruction` that is is a `building:Roof` with sloping surfaces, typically inclined at an angle greater than 10 degrees, which allows for efficient water run-off and can provide additional space under the roof, such as an attic or loft. " .

building:ResidentialDwelling a building:FunctionalClassOfStructureUnitState ;
    rdfs:label "Residential Dwelling"@en-gb ;
    skos:note "An instance of `building:FunctionalClassOfStructureUnitState` that is a class of `building:StructureUnitState` that is used primarily as a place for people to live. " ;
    rdfs:comment "A structure unit state that is used primarily as a place for people to live" ;
    rdfs:subClassOf building:StructureUnitState .

building:RoofInsulation rdfs:label "Roof Insulation"@en-gb ;
    rdfs:comment "A `building:ClassOfRoof` that is a classifier of `building:Roof` by the construction methods used. Instances of this class are `rdfs:subClass(es)Of` `building:Roof`." ;
    rdfs:subClassOf building:ClassOfRoof .

building:RoofRooms a building:RoofConstruction ;
    rdfs:label "Roof Rooms"@en-gb ;
    rdfs:comment "An instance of `building:RoofConstruction` that includes an `building:PhysicallyBoundedSpace`" .

building:Sandstone a building:WallConstruction ;
    rdfs:label "Sandstone"@en-gb ;
    rdfs:comment "An instance of `building:WallConstruction` that is is a type of masonry wall constructed using sandstone blocks or stones. Sandstone is a sedimentary rock composed mainly of sand-sized mineral particles or rock fragments. " .

building:SecondaryGlazing a building:GlazingType ;
    rdfs:label "Secondary Glazing" ;
    rdfs:comment "An instance of `building:GlazingType` that is  an additional window pane or glazing unit installed on the interior side of an existing window. It is typically used to enhance thermal insulation, reduce noise, and improve energy efficiency in `building:StructureUnit` without replacing the original `building:window`s." ;
    rdfs:subClassOf building:MultipleGlazing .

building:SemiDetached a building:BuiltForm ;
    rdfs:label "Semi Detached"@en-gb ;
    rdfs:comment "An instance of `building:BuiltForm` that is a `building:StructureUnit` that shares one common wall with an adjacent `building:StructureUnit`. This configuration means that the two `building:StructureUnit`s are mirror images of each other or designed similarly, each having its own separate entrance and private living space." ;
    rdfs:subClassOf building:StructureUnitState .

building:SingleGlazing a building:GlazingType ;
    rdfs:label "Single Glazing"@en-gb ;
    rdfs:comment "An instance of `building:GlazingType` that is  a single pane of glass within the `building:Window`. " .

building:Solid a building:FloorConstruction ;
    rdfs:label "Solid"@en-gb ;
    rdfs:comment "An instance of `building:FloorConstruction` that is a type of floor construction made from a continuous, rigid material, typically concrete, laid directly onto the ground or on a solid base." .

building:SolidBrick a building:WallConstruction ;
    rdfs:label "Solid Brick"@en-gb ;
    rdfs:comment "An instance of `building:WallConstruction` that is a type of wall construction where the wall is built entirely from bricks without any internal cavity or gap." .

building:Suspended a building:FloorConstruction ;
    rdfs:label "Suspended"@en-gb ;
    rdfs:comment "An instance of `building:FloorConstruction` that is  a type of floor construction where the floor surface is raised above the ground level, supported by a framework of joists, beams, or other structural elements. Unlike solid floors, which are laid directly on the ground, suspended floors have an air space (void) between the ground and the floor surface." .

building:SystemBuilt a building:WallConstruction ;
    rdfs:label "System Built"@en-gb ;
    rdfs:comment "An instance of `building:WallConstruction` that is a type of wall construction that utilises prefabricated components or modules, which are manufactured off-site and then assembled on-site to create the wall " .

building:ThatchedRoof a building:RoofConstruction ;
    rdfs:label "Thatched Roof"@en-gb ;
    rdfs:comment "An instance of `building:RoofConstruction` that is a type of roof constructed from natural materials such as straw, reed, heather, or palm leaves, which are layered and bound together to create a weather-resistant covering." .

building:ThatchedWithAdditionalInsulation a building:RoofInsulationLocation ;
    rdfs:label "Thatched With Additional Insulation"@en-gb ;
    rdfs:comment "An instance of `building:RoofInsulationLocation` that has insulation materials in the roof in addition to the `building:Thatched` roof." .

building:TimberFrame a building:WallConstruction ;
    rdfs:label "Timber Frame"@en-gb ;
    rdfs:comment "An instance of `building:WallConstruction` that is a type of wall construction that uses a framework of timber (wood) as the primary structural element." .

building:TripleGlazing a building:GlazingType ;
    rdfs:label "Triple Glazing" ;
    rdfs:comment "An instance of `building:GlazingType` that is a type of window that incorporates three panes of glass separated by air or gas-filled spaces, providing enhanced thermal insulation, soundproofing, and energy efficiency compared to single or double glazed windows. " ;
    rdfs:subClassOf building:MultipleGlazing .

building:lodgementDate a owl:ObjectProperty ;
    rdfs:label "Lodgement Date"@en-gb ;
    rdfs:comment "An `ies: ParticularPeriod ` that is the date on which the `building:EnergyPerformanceResult` was lodged into the Register." ;
    rdfs:domain building:EnergyPerformanceAssessmentResult ;
    rdfs:range ies:ParticularPeriod ;
    rdfs:subPropertyOf ies:relationship .

building:assessedEachMemberOf a owl:ObjectProperty ;
    rdfs:label "Assessed Each Member Of"@en-gb ;
    rdfs:comment "The relation that obtains between an assessment a and a class of elements E if and only a has as target the members of E" ;
    rdfs:domain ies:Assessment ;
    rdfs:range ies:ClassOfElement .

building:assumedEachMemberOf a owl:ObjectProperty ;
    rdfs:comment "The relation that obtains between an assessment a and a class of elements E if and only a has assumed as target the members of E" ;
    rdfs:domain ies:Assessment ;
    rdfs:range ies:ClassOfElement .

# building:assessedAs

building:hasQuantity a owl:ObjectProperty ;
    rdfs:label "hasQuantity"@en ;
    rdfs:comment """
      A relationship linking a Measure to a qudt:Quantity;
      QUDT, <http://qudt.org/schema/qudt/>, or Quantities, Units, Dimensions,
      and Types, is an ontology for describing 'semantic specifications for
      units of measure, quantity kind, dimensions and data types.'
      """@en ;
    rdfs:domain ies:Measure ;
    rdfs:range <http://qudt.org/schema/qudt/Quantity> ;
    skos:note "Expected in IES 4.4" .

building:hasParentUPRN a owl:ObjectProperty ;
    rdfs:label "has Parent UPRN"@en-gb ;
    rdfs:comment "An `ies:isPartOf` relationship that allows for UPRNs to group into a hierarchy" ;
    rdfs:domain building:UPRN ;
    rdfs:range building:UPRN ;
    rdfs:subPropertyOf ies:isPartOf .

building:isBoundedByPartOf a owl:ObjectProperty ;
    rdfs:label "is bounded by part Of"@en-gb ;
    rdfs:comment "The relation that obtains between a `building:PhysicallyBoundedSpace` A and `building:BuiltEntity` B if and only if A has part of B as a boundary." ;
    rdfs:domain building:PhysicallyBoundedSpace ;
    rdfs:range building:Floor,
        building:Roof,
        building:Wall .

building:CO2 a building:ChemicalCompound ;
    rdfs:label "CO2"@en-gb ;
    rdfs:comment "An instance `building:ChemicalCompound` otherwise known as carbon dioxide. CO2 is a colourless, odourless gas that is naturally present in Earth's atmosphere. It is composed of one carbon atom and two oxygen atoms. CO2 is produced by the burning of fossil fuels, respiration in living organisms, and the decay of organic matter. It is utilised by plants during photosynthesis and is a significant greenhouse gas, contributing to the greenhouse effect and climate change when present in elevated levels." .

building:pluriverse a ies:Element ;
    rdfs:label "Pluriverse"@en ;
    rdfs:comment """
      A singleton individual at the ontology level, meaning everything
      contained in all the possible worlds.
      """@en ;
    skos:note "Expected in IES 4.3" .

building:TechnicalSystem a rdfs:Class ;
    rdfs:label "Technical System"@en-gb ;
    rdfs:comment "An `ies:Entity` that is a human-made system (consisting of parts interacting with each other according to some rule or pattern) that is intended to serve a certain function.  A TechnicalSystem can exist in various states over time." ;
    ies:powertype building:ClassOfTechnicalSystem ;
    rdfs:subClassOf building:TechnicalSystemState,
        ies:Entity .

building:TechnicalSystemState a rdfs:Class ;
    rdfs:label "Technical System State"@en-gb ;
    rdfs:comment "An `ies:State` that is a temporal state of `building:TechnicalSystem`." ;
    rdfs:subClassOf ies:State .

building:ElectricityGenerationSystem a rdfs:Class ;
    rdfs:label "Electricity Generation System" ;
    rdfs:comment "A technical system that is designed to generate electricity." ;
    rdfs:subClassOf building:TechnicalSystem .

building:SolarPhotovoltaicSystem a rdfs:Class ;
    rdfs:label "Solar Photovoltaic System" ;
    rdfs:comment "An electricity generation system that converts sunlight into electricity using photovoltaic panels." ;
    rdfs:subClassOf building:ElectricityGenerationSystem .

building:WindTurbine a rdfs:Class ;
    rdfs:label "Wind Turbine" ;
    rdfs:comment "An electricity generation system that converts wind energy into electricity." ;
    rdfs:subClassOf building:ElectricityGenerationSystem .

##################### from prior work on heating systems (edited) ##############################

building:AirSourceHeatPump a rdfs:Class ;
    rdfs:label "Air Source Heat Pump"@en-gb ;
    rdfs:comment "A heat pump that operates by absorbing heat from external air" ;
    rdfs:subClassOf building:HeatPump .

building:BoilerHeatProductionSystem a rdfs:Class ;
    rdfs:label "Boiler Heat Production System"@en-gb ;
    rdfs:comment "A heat production system that operates by boiling an amount of water" ;
    rdfs:subClassOf building:HeatProductionSystem .

building:B30K_Boiler a rdfs:Class ;
    rdfs:label "B30K Boiler" ;
    rdfs:comment "A `building:BoilerHeatProductionSystem` that is compatible with B30K fuel, a blend of kerosene and FAME biofuel." ;
    rdfs:subClassOf building:BoilerHeatProductionSystem .

building:CentralHeatingSystem a rdfs:Class ;
    rdfs:label "Central Heating System"@en-gb ;
    rdfs:comment "A heating system that is designed for producing heat and distributing it across a structure unit or a group of structure units in order to heat them up; it has as sub-systems a heat production system and a heat distribution system" ;
    rdfs:subClassOf building:HeatingSystem .

building:CommunityCentralHeatingSystem a rdfs:Class ;
    rdfs:label "Community Central Heating System"@en-gb ;
    rdfs:comment "A central heating system that is designed for heating a group of structure units" ;
    rdfs:subClassOf building:CentralHeatingSystem .

building:ElectricHeatProductionSystem a rdfs:Class ;
    rdfs:label "Electric Heat Production System"@en-gb ;
    rdfs:comment "A heat production system that operates by turning electricity into heat" ;
    rdfs:subClassOf building:HeatProductionSystem .

building:ElectricRadiantHeatingSystem a rdfs:Class ;
    rdfs:label "Electric Radiant Heating System"@en-gb ;
    rdfs:comment "A radiant system that produces heat by means of electric heating coils or wires" ;
    rdfs:subClassOf building:RadiantHeatingSystem .

building:EnergySource a rdfs:Class ;
    rdfs:label "Energy Source"@en-gb ;
    rdfs:comment "A stuff - ies:Stuff - that can be used for releasing energy for various usages" ;
    rdfs:subClassOf ies:Stuff .

# building:Fuel a rdfs:Class ;
#     rdfs:label "Fuel" ;
#     rdfs:comment "An energy source that can be used for releasing thermal energy by making it undergo certain chemical reactions" ;
#     rdfs:subClassOf building:EnergySource .

# building:FossilFuel a rdfs:Class ;
#     rdfs:label "Fossil Fuel" ;
#     rdfs:comment "A `building:Fuel` that is formed from the remains of ancient organisms, typically consisting of hydrocarbons." ;
#     rdfs:subClassOf building:Fuel .

# building:SolidFossilFuel a rdfs:Class ;
#     rdfs:label "Solid Fossil Fuel" ;
#     rdfs:comment "A `building:FossilFuel` that is a solid fuel formed from the remains of ancient organisms." ;
#     rdfs:subClassOf building:FossilFuel .

# building:LiquidFossilFuel a rdfs:Class ;
#     rdfs:label "Liquid Fossil Fuel" ;
#     rdfs:comment "A `building:FossilFuel` that is liquid fuel formed from the remains of ancient organisms." ;
#     rdfs:subClassOf building:FossilFuel .

# building:GaseousFossilFuel a rdfs:Class ;
#     rdfs:label "Gaseous Fossil Fuel" ;
#     rdfs:comment "A `building:FossilFuel` that is a gaseous fuel formed from the remains of ancient organisms." ;
#     rdfs:subClassOf building:FossilFuel .

# building:Biofuel a building:Fuel, building:RenewableEnergySource ;
#         rdfs:comment "The fuel that consists of materials coming from animal waste or from the tissues of plants or algae" ;
#         rdfs:label "Biofuel" ;
#         rdfs:subClassOf building:Fuel .

# building:SolidBiofuel a rdfs:Class ;
#     rdfs:label "Solid Biofuel" ;
#     rdfs:comment "A solid fuel derived from organic matter." ;
#     rdfs:subClassOf building:Biofuel .

# building:LiquidBiofuel a rdfs:Class ;
#     rdfs:label "Liquid Biofuel" ;
#     rdfs:comment "A liquid fuel derived from organic matter." ;
#     rdfs:subClassOf building:Biofuel .

# building:GaseousBiofuel a rdfs:Class ;
#     rdfs:label "Gaseous Biofuel" ;
#     rdfs:comment "A gaseous fuel derived from organic matter." ;
#     rdfs:subClassOf building:Biofuel .

# building:Biogas a building:GaseousBiofuel, building:RenewableEnergySource ;
#         rdfs:comment "The part of building:Biofuel that under normal temperature and pressure occurs in gas state - as such, it is also a part of building:FuelGas; the heating value of biogas derives from its methane content; portions of biogas typically result from the decomposition of portions of biomass" ;
#         rdfs:label "Biogas" ;
#         ies:isPartOf building:Biofuel, building:FuelGas .

# building:RawBiogas a building:GaseousBiofuel, building:RenewableEnergySource ;
#     rdfs:label "Raw Biogas" ;
#         rdfs:comment "The part of building:Biogas that has a percentage of methane between 50 percent and 75 percent; it results from waste management processes, and has not been further refined to increase its methane content" ;
#         ies:isPartOf building:Biogas .

# building:Biomethane a building:GaseousBiofuel, building:RenewableEnergySource ;
#     rdfs:label "Biomethane" ;
#         rdfs:comment "The part of building:Biogas that has a percentage of methane above 75 percent; it is first produced by means of waste management processes and is then refined to increase its methane content" ;
#         ies:isPartOf building:Biogas .

# building:LiquidBiofuel a building:Fuel, building:RenewableEnergySource ;
#     rdfs:label "Liquid BioFuel" ;
#         rdfs:comment "The part of building:Biofuel that under normal temperature and pressure occurs in liquid state" ;
#         ies:isPartOf building:Biofuel .

# building:Biodiesel a building:LiquidBiofuel, building:RenewableEnergySource ;
#     rdfs:label "Biodiesel" ;
#         rdfs:comment "The part of building:LiquidBiofuel that (i) consists mostly of FAME (fatty acid methyl esters) and glycerin, and (ii) is produced through a process (transesterification) in which vegetables oils and/or animal fats are reacted with ethanol or methanol" ;
#         ies:isPartOf building:Biofuel .

# building:BioOil a building:LiquidBiofuel, building:RenewableEnergySource ;
#     rdfs:label "BioOil" ;
#         rdfs:comment "The part of building:LiquidBiofuel that is produced from biomasses through their thermal degradation in an inert atmosphere free from oxygen (pyrolysis)" ;
#         ies:isPartOf building:Biofuel .

# building:Kerosene a building:LiquidFossilFuel, building:EnergySource ;
#     rdfs:label "Kerosene" ;
#         rdfs:comment "The fuel that consists of a mixture of hydrocarbons of which the main constituents are saturated straight-chain and branched-chain paraffins; under normal pressure and temperature it occurs in liquid state; it is typically produced from petroleum through a process of fractional distillation" .

building:FurnaceHeatProductionSystem a rdfs:Class ;
    rdfs:label "Furnace Heat Production System"@en-gb ;
    rdfs:comment "A heat production system that operates by boiling an amount of water" ;
    rdfs:subClassOf building:HeatProductionSystem .

building:GasPortableHeater a rdfs:Class ;
    rdfs:label "Gas portable Heater" ;
    rdfs:comment "A portable heater that operates by burning gas" ;
    rdfs:subClassOf building:PortableHeater .

building:GroundSourceHeatPump a rdfs:Class ;
    rdfs:label "Ground Source Heat Pump"@en-gb ;
    rdfs:comment "A heat pump that operates by absorbing heat from the ground" ;
    rdfs:subClassOf building:HeatPump .

building:HeatDistributionSystem a rdfs:Class ;
    rdfs:label "Heat Distribution System"@en-gb ;
    rdfs:comment "A technical system that is designed to be the sub-system of a central heating system that distributes the produced heat across a structure unit or a group of structure units in order to heat them up; it operates by circulating a warm fluid as a medium for delivering heat" ;
    rdfs:subClassOf building:TechnicalSystem .

building:HeatProductionSystem a rdfs:Class ;
    rdfs:label "Heat Production System"@en-gb ;
    rdfs:comment "A technical system that is designed to be the sub-system of a central heating system that produces the heat to heat up a structure unit or a group of structure units" ;
    rdfs:subClassOf building:TechnicalSystem .

building:ClassOfTechnicalSystem a rdfs:Class ;
    rdfs:label "Class Of Technical System"@en-gb ;
    rdfs:comment "An `ies:ClassOfEntity` that is the various classes of building:TechnicalSystem`." ;
    rdfs:subClassOf ies:ClassOfEntity .

building:ClassOfTechnicalSystemState a rdfs:Class ;
    rdfs:label "Class Of Technical System"@en-gb ;
    rdfs:comment "An `ies:ClassOfEntityState` that is the various classes of building:TechnicalSystemState`." ;
    rdfs:subClassOf building:ClassOfEntityState .

building:HeatPump a rdfs:Class ;
    rdfs:label "Heat Pump"@en-gb ;
    rdfs:comment "A heat production system that operates by absorbing heat from the external environment" ;
    rdfs:subClassOf building:HeatProductionSystem .

building:HeatingControlSystem a rdfs:Class ;
    rdfs:label "Heating Control System"@en-gb ;
    skos:altLabel "Building Services Heating Controls"@en-gb, "Heating Control Services"@en-gb ;
    rdfs:comment "A technical system that is designed to be the sub-system of a heating system that regulates the operations of the whole heating system in order to maintain a desired temperature in the serviced area" ;
    ies:powertype building:ClassOfHeatingControlSystem ;
    rdfs:subClassOf building:TechnicalSystem .

building:ClassOfHeatingControlSystem a rdfs:Class ;
    rdfs:subClassOf building:ClassOfTechnicalSystem ;
    rdfs:label "Class Of Heating Control System"@en-gb ;
    rdfs:comment "A `building:ClassOfTechnicalSystem` that classifies `building:HeatingControlSystems" .

building:heatingControlDescription a owl:DatatypeProperty ;
    rdfs:label "Heating Control Description" ;
    rdfs:comment "A description of the heating control system, typically a string of text" ;
    rdfs:domain building:ClassOfHeatingControlSystem ;
    rdfs:range xsd:string ;
    rdfs:subPropertyOf ies:attribute .

building:UKCtrl_2204 a building:ClassOfHeatingControlSystem ;
    rdfs:label "UK Heating Control Code 2204" ;
    rdfs:comment "Control code 2204 for `building:StructureUnits` with programmer and room thermostat" ;
    building:heatingControlDescription "Programmer and room thermostat" ;
    rdfs:seeAlso <https://files.bregroup.com/SAP/SAP-2012_9-92.pdf> ;
    skos:note "There are a large number of codes as in the link above page 212 table 4e" ;
    ies:isIdentifiedBy [
        a ies:Representation ;
        ies:representationValue "2204"
    ] .

building:UKCtrl_2106 a building:ClassOfHeatingControlSystem ;
    rdfs:label "UK Heating Control Code 2106"@en-gb ;
    rdfs:comment "Control code 2106 for `building:StructureUnits` with programmer, room thermostat and TRVs" ;
    building:heatingControlDescription "Programmer, room thermostat and TRVs" ;
    rdfs:seeAlso <https://files.bregroup.com/SAP/SAP-2012_9-92.pdf> ;
    skos:note "There are a large number of codes as in the link above page 212 table 4e" ;
    ies:isIdentifiedBy [
        a ies:Representation ;
        ies:representationValue "2106"
    ] .

building:HeatingSystem a rdfs:Class ;
    rdfs:label "Heating System"@en-gb ;
    skos:altLabel "Building Services Heating"@en-gb, "Heating Services"@en-gb ;
    rdfs:comment "A technical system that is designed for heating one structure unit, a group of structure units, or a space" ;
    rdfs:subClassOf building:TechnicalSystem .

building:HeatStorageSystem a rdfs:Class ;
    rdfs:label "Heat Storage System" ;
    rdfs:comment "A heating system that stores thermal energy for later use." ;
    rdfs:subClassOf building:HeatingSystem .

building:HydronicHeatDistributionSystem a rdfs:Class ;
    rdfs:label "Hydronic Heat Distribution System"@en-gb ;
    rdfs:comment "A heat distribution system that operates by circulating hot liquid water through a network of pipes" ;
    rdfs:subClassOf building:HeatDistributionSystem .

building:NonServicedWithHeating a rdfs:Class ;
    rdfs:label "Non Serviced With Heating"@en-gb ;
    rdfs:comment "The characteristic of states of structure units or spaces that consists in having no heating system in place for heating it" ;
    rdfs:subClassOf building:StructureUnitOrSpaceState .

building:RadiantHeatingSystem a rdfs:Class ;
    rdfs:label "Radiant Heating System"@en-gb ;
    rdfs:comment "A heating system that radiates heat directly into one or more spaces of a structure unit to heat them up, without employing a dedicated heat distribution sub-system for circulating a warm fluid" ;
    rdfs:subClassOf building:HeatingSystem .

building:RadiatorHydronicHeatDistributionSystem a rdfs:Class ;
    rdfs:label "Radiator Hydronic Heat Distribution System"@en-gb ;
    rdfs:comment "A hydronic heat distribution system that operates by circulating hot liquid water through a network of pipes and radiators" ;
    rdfs:subClassOf building:HydronicHeatDistributionSystem .

building:RadiatorSteamHeatDistributionSystem a rdfs:Class ;
    rdfs:label "Radiator Steam Heat Distribution System"@en-gb ;
    rdfs:comment "A steam heat distribution system that operates by circulating hot water steam through a network of pipes and radiators" ;
    rdfs:subClassOf building:SteamHeatDistributionSystem .

# building:RenewableEnergySource a rdfs:Class ;
#     rdfs:label "Renewable Energy Source" ;
#     rdfs:comment "An energy source that can be replenished at a higher rate than it is consumed" ;
#     rdfs:subClassOf building:EnergySource .

# building:Sunlight a building:RenewableEnergySource ;
#     rdfs:label "Sunlight" ;
#     rdfs:comment "The energy source that consists of electromagnetic radiation given off by the Sun." .

# building:Wind a building:RenewableEnergySource ;
#     rdfs:label "Wind" ;
#     rdfs:comment "The energy source that consists of the bulk movement of air." .

building:ServicedWithHeating a rdfs:Class ;
    rdfs:label "Serviced With Heating"@en-gb ;
    rdfs:comment "The characteristic of states of structure units or spaces that consists in having some heating system in place for heating it" ;
    rdfs:subClassOf building:StructureUnitOrSpaceState .

building:SingleUnitCentralHeatingSystem a rdfs:Class ;
    rdfs:label "Single Unit Central Heating System"@en-gb ;
    rdfs:comment "A central heating system that is designed for heating one structure unit" ;
    rdfs:subClassOf building:CentralHeatingSystem .

building:PortableHeater a rdfs:Class ;
    rdfs:label "Portable Heater" ;
    rdfs:comment "A heating system that is designed to be easily moved and is typically used for heating a space of a structure unit" ;
    rdfs:subClassOf building:HeatingSystem .

building:ElectricCeilingHeater a rdfs:Class ;
    rdfs:label "Electric Ceiling Heater" ;
    rdfs:comment:"A `building:HeatingSystem` that is mounted on the ceiling and uses electricity to generate heat, typically through resistance coils or infrared radiation." ;
    rdfs:subClassOf building:HeatingSystem .

building:FanCoilUnit a rdfs:Class ;
rdfs:label "Fan Coil Unit" ;
rdfs:comment "A `building:HeatDistributionSystem` that uses a coil and a fan to heat or cool air and distribute it within a space. Fan coil units are typically part of HVAC systems and can be used for both heating and cooling by circulating air over a coil containing hot or cold water." ;
rdfs:subClassOf building:HeatDistributionSystem .

building:SteamHeatDistributionSystem a rdfs:Class ;
    rdfs:label "Steam Heat Distribution System"@en-gb ;
    rdfs:comment "A heat distribution system that operates by circulating hot water steam through a network of pipes" ;
    rdfs:subClassOf building:HeatDistributionSystem .

building:UnderfloorElectricRadiantSystem a rdfs:Class ;
    rdfs:label "Underfloor Electric Radiant System"@en-gb ;
    rdfs:comment "An electric radiant heating system that is installed beneath a floor and radiates heat through the floor surface" ;
    rdfs:subClassOf building:ElectricRadiantHeatingSystem .

building:UnderfloorHydronicHeatDistributionSystem a rdfs:Class ;
    rdfs:label "Underfloor Hydronic Heat Distribution System"@en-gb ;
    rdfs:comment "A hydronic heat distribution system that operates by circulating hot liquid water through a network of pipes that are positioned beneath the floor" ;
    rdfs:subClassOf building:HydronicHeatDistributionSystem .

building:UnderfloorSteamHeatDistributionSystem a rdfs:Class ;
    rdfs:label "Underfloor Steam Heat Distribution System"@en-gb ;
    rdfs:comment "A steam heat distribution system that operates by circulating hot water steam through a network of pipes that are positioned beneath the floor" ;
    rdfs:subClassOf building:SteamHeatDistributionSystem .

building:WarmAirHeatDistributionSystem a rdfs:Class ;
    rdfs:label "Warm Air Heat Distribution System"@en-gb ;
    rdfs:comment "A heat distribution system that operates by circulating warm air through a network of ducts" ;
    rdfs:subClassOf building:HeatDistributionSystem .

building:WaterSourceHeatPump a rdfs:Class ;
    rdfs:label "Water Source Heat Pump"@en-gb ;
    rdfs:comment "A heat pump that operates by absorbing heat from an external body of water" ;
    rdfs:subClassOf building:HeatPump .

building:ExhaustAirHeatPump a rdfs:Class ;
    rdfs:label "Exhaust Air Heat Pump" ;
    rdfs:comment "A heat pump that operates by absorbing heat from the exhaust air from a source." ;
    rdfs:subClassOf building:HeatPump .

building:CommunityHeatPump a rdfs:Class ;
    rdfs:label "Community Heat Pump" ;
    rdfs:comment "A heat pump that is designed for heating a group of structure units" ;
    rdfs:subClassOf building:HeatPump .

# building:Anthracite a building:SolidFossilFuel ;
#     rdfs:label "Anthracite" ;
#     ies:isPartOf building:Coal ;
#     rdfs:comment "The part of building:Coal that has 86 percent or more of fixed carbon" .

# building:Biomass a building:Fuel ,
#         building:RenewableEnergySource ;
#     rdfs:label "Biomass" ;
#     rdfs:comment "The fuel that consists of materials coming from animal waste or from the tissues of plants or algae" ;
#     ies:isPartOf building:Biofuel .

# building:Electricity a building:EnergySource ;
#     rdfs:label "Electricity" ;
#     rdfs:comment "The energy source - building:EnergySource - that consists of all the elements that are electrically charged" .

# building:LPG a building:GaseousFossilFuel ;
#     rdfs:label "Liquid Petroleum Gas" ;
#     ies:isPartOf building:FuelGas ;
#     rdfs:comment "The part of building:FuelGas that is mostly composed of a mixture of propene, propane, butene, and butane, with common additions of ethane, ethylene, and mercaptan; it is stored in liquid form by means of pressurisation, and it quickly evaporates under normal temperature and pressure" .

# building:NaturalFuelGas a building:GaseousFossilFuel ;
#     rdfs:label "Natural Fuel Gas" ;
#     ies:isPartOf building:FuelGas ;
#     rdfs:comment "The part of building:FuelGas that has natural origin and is composed of a mixture of gaseous hydrocarbons - mostly methane" .

# building:Oil a building:Fuel ;
#     rdfs:label "Oil" ;
#     rdfs:comment "The fuel that consists of a complex mixture of hydrocarbons that comes from geological formations and occurs in liquid state" .

# building:SmokelessCoal a building:SolidFossilFuel ;
#     rdfs:label "Smokeless Coal" ;
#     ies:isPartOf building:Coal ;
#     rdfs:comment "The part of building:Coal that has the tendency to emit no visible smoke or minimal amounts of smoke during combustion" .

# building:BituminousCoal a building:SolidFossilFuel ;
#     rdfs:label "Bituminous Coal" ;
#     ies:isPartOf building:Coal ;
#     rdfs:comment "The part of `building:Coal` containing a high percentage of volatile matter, which produces smoke when burned." .

# building:WoodChips a building:Fuel,
#         building:RenewableEnergySource ;
#     rdfs:label "Wood Chips" ;
#     ies:isPartOf building:Wood ;
#     rdfs:comment "The part of building:Wood that consists of small bits resulted from the cutting of larger chunks of wood" .

# building:WoodLogs a building:Fuel,
#         building:RenewableEnergySource ;
#     rdfs:label "Wood Logs" ;
#     ies:isPartOf building:Wood ;
#     rdfs:comment "The part of building:Wood that consists of mid-sized portable chunks" .

# building:WoodPellets a building:Fuel,
#         building:RenewableEnergySource ;
#     rdfs:label "Wood Pellets" ;
#     ies:isPartOf building:Wood ;
#     rdfs:comment "The part of building:Wood that consists of small cylindrical units produced by compressing wood fibres" .

building:isEquipmentOf a owl:ObjectProperty ;
    rdfs:label "is Equipment Of"@en-gb ;
    rdfs:comment "The relation that obtains between an element e and a technical system t if and only if (i) e is not part of t, and (ii) e enhances or completes t's capabilities" ;
    rdfs:domain ies:Element ;
    rdfs:range building:TechnicalSystem .

building:isEquipmentOfStructureUnitOrSpace a owl:ObjectProperty ;
    rdfs:label "is Equipment Of Unit Or Space"@en-gb ;
    rdfs:comment "The relation that obtains between an element e and a structure unit or space t if and only if (i) e is not part of t, and (ii) e enhances or completes t's capabilities" ;
    rdfs:domain ies:Element ;
    rdfs:range building:StructureUnitOrSpaceState ;
    rdfs:subPropertyOf building:isEquipmentOf .

building:isHeatedBy a owl:ObjectProperty ;
    rdfs:label "is Heated By"@en-gb ;
    rdfs:comment "The sub-relation of building:isServicedBy that obtains between a state of a structure unit or space and the heating system that is put in place for heating it; a structure unit or space state can be heated even by a heating system that is located far away from it: for example, a flat can be heated by a community heating system whose heat production system is installed in another part of the building; when a heating system heats an entire structure unit, the relation building:isHeatedBy obtains between the entire structure unit state and the heating system, as well as between each individual space and the heating system" ;
    rdfs:domain building:StructureUnitOrSpaceState ;
    rdfs:range building:HeatingSystem ;
    rdfs:subPropertyOf building:isServicedBy .

building:isPrimarilyHeatedBy a owl:ObjectProperty ;
    rdfs:label "is Primarily Heated By" ;
    rdfs:comment "The sub-relation of building:isHeatedBy that obtains between a state of a structure unit or space and the heating system that is considered the primary source of heating." ;
    rdfs:domain building:StructureUnitOrSpaceState ;
    rdfs:range building:HeatingSystem ;
    rdfs:subPropertyOf building:isHeatedBy .

building:isSecondarilyHeatedBy a owl:ObjectProperty ;
    rdfs:label "is Secondarily Heated By" ;
    rdfs:comment "The sub-relation of building:isHeatedBy that obtains between a state of a structure unit or space and a heating system that is considered a secondary source of heating." ;
    rdfs:domain building:StructureUnitOrSpaceState ;
    rdfs:range building:HeatingSystem ;
    rdfs:subPropertyOf building:isHeatedBy .

building:isOperableWithFuel a owl:ObjectProperty ;
    rdfs:label "is Operable With Fuel"@en-gb ;
    rdfs:comment "The sub-relation of building:isOperableWithEnergySource that obtains between a technical system and a fuel on which that technical system can operate" ;
    rdfs:domain building:TechnicalSystem ;
    rdfs:range building:ClassOfFuelPortion ;
    rdfs:subPropertyOf building:isOperableWithEnergySource .

building:isOperableWithEnergySource a owl:ObjectProperty ;
    rdfs:label "is Operable With Energy Source"@en-gb ;
    rdfs:comment "The relation that obtains between a technical system and an energy source on which that technical system can operate" ;
    rdfs:domain building:TechnicalSystem ;
    rdfs:range building:ClassOfEnergySourcePortion .

building:isServicedBy a owl:ObjectProperty ;
    rdfs:label "is Serviced By"@en-gb ;
    rdfs:comment "The relation that obtains between a state of a structure unit or space s and a technical system t if and only if t is put in place for enhancing the capabilities of s or benefiting the occupiers of s; examples of technical systems that service structure units or space include heating systems, power supply systems, and plumbing systems" ;
    rdfs:domain building:StructureUnitOrSpaceState ;
    rdfs:range building:TechnicalSystem .

# building:Coal a building:SolidFossilFuel ;
#     rdfs:label "Coal" ;
#     rdfs:comment "The fuel that consists of a solid carbon-rich material with more than 50 percent by mass - or 70 percent by volume - of carbonaceous matter" .

# building:FuelGas a building:Fuel ;
#     rdfs:label "Fuel Gas" ;
#     rdfs:comment "The fuel that under normal temperature and pressure occurs in gas state" .

# building:Wood a building:Fuel,
#         building:RenewableEnergySource ;
#     rdfs:label "Wood" ;
#     rdfs:comment "The stuff - ies:Stuff - that consists of all the matter that is part of or originates from the nutrient-conducting tissues of trees, shrubs, or lianas; it is a fuel, since it can be used for releasing thermal energy by making it undergo combustion" .


##################### Nature of supply ###############
building:EnergySupply a rdfs:Class ;
    rdfs:label "Energy Supply"@en-gb ;
    rdfs:comment "An instance of `ies:ClassOfEvent` that is the supply of a portion usable energy. " ;
    rdfs:subClassOf ies:Event .

building:MainsGasSupply a rdfs:Class ;
    rdfs:label "Mains Gas Supply"@en-gb ;
    rdfs:comment "A `building:EnergySupply` which is the direct supply of `building:FuelGas` to a `building:StructureUnitOrSpace`." ;
    rdfs:subClassOf building:EnergySupply .

############# Geography #####################

building:locationBoundaryPoint a owl:ObjectProperty ;
    rdfs:label "location boundary point"@en-gb ;
    rdfs:comment "A relationship between an `ies:Location` and an `ies:GeoPoint` that holds when the point is on the boundary of the location." ;
    skos:note "we need a more thorough description of regions and boundaries" ;
    rdfs:domain ies:Location ;
    rdfs:range ies:GeoPoint .

#############   TrustMark   #############
building:TrustMark a ies:Organisation ;
    rdfs:label "TrustMark"@en-gb ;
    rdfs:comment "TrustMark (2005) Limited is a not-for-profit organisation, operating under a Master Licence Agreement, issued by the Government's Department for Business & Trade." .

building:TrustMarkAssessment a rdfs:Class ;
    rdfs:label "TrustMark Assessment"@en-gb ;
    rdfs:comment "A `building:EnergyPerformanceAssessment` that assesses the state of a building in the UK using the TrustMark quality scheme for home improvements." ;
    rdfs:subClassOf building:EnergyPerformanceAssessment .

building:Resident a rdfs:Class ;
    rdfs:label "Resident"@en-gb ;
    rdfs:comment "A temporal state of a Responsible Actor whose legal domicile is a `building:StructureUnitState`." ;
    rdfs:subClassOf ies:InResidence .

building:hasDomicileIn a owl:ObjectProperty ;
    rdfs:label "is Located In"@en-gb ;
    rdfs:domain building:Resident ;
    rdfs:range building:StructureUnitState ;
    rdfs:comment "A sibling property of `ies:visits` connecting a `building:Resident` to a location (`building:StructureUnitState`) in which it has legal domicile." ;
    rdfs:subPropertyOf ies:inLocation .

building:residesIn a owl:ObjectProperty ;
    rdfs:label "Resides In"@en-gb ;
    rdfs:domain ies:PersonState ;
    rdfs:range building:ResidentialDwelling ;
    rdfs:comment "A relation connecting a `ies:PersonState` to a location (`building:ResidentialDwelling`) in which they live." ;
    rdfs:subPropertyOf building:hasDomicileIn .

building:Tenure a rdfs:Class ;
    rdfs:label "Tenure"@en-gb ;
    rdfs:comment "A classifier of the temporal state of `building:StructureUnit` during which a property is occupied for a particular purpose, such as residence or business. It can refer to the ownership or rental status of a property. Tenure is also the legal rights associated with that occupation." ;
    skos:example "Owner Occupied", "Private Rental Sector", "Social Housing", "Other" ;
    rdfs:subClassOf building:ClassOfStructureUnitState .

building:OwnerOccupied a building:Tenure ;
    rdfs:label "Owner Occupied"@en-gb ;
    rdfs:comment "A `building:Tenure` where the occupant owns the property." ;
    rdfs:subClassOf building:StructureUnitState .

building:PrivateRentalSector a building:Tenure ;
    rdfs:label "Private Rental Sector"@en-gb ;
    rdfs:comment "A `building:Tenure` where the occupant rents the property from a private landlord." ;
    rdfs:subClassOf building:StructureUnitState .

building:SocialHousing a building:Tenure ;
    rdfs:label "Social Housing"@en-gb ;
    rdfs:comment "A `building:Tenure` where the occupant rents the property from a social landlord, such as a local authority or housing association." ;
    rdfs:subClassOf building:StructureUnitState .

building:OtherTenure a building:Tenure ;
    rdfs:label "Other Tenure"@en-gb ;
    rdfs:comment "A `building:Tenure` that does not fit into the other categories, such as temporary accommodation or shared ownership." ;
    rdfs:subClassOf building:StructureUnitState .

building:TMLicensee a rdfs:Class ;
    rdfs:label "Trust Mark Licensee" ;
    rdf:comment "An `ies:OrganisationState` that asserts that the organisation has been certified under the Trustmark Quality Scheme" ;
    rdfs:subClassOf ies:OrganisationState .

building:Installer a rdfs:Class ;
    rdfs:label "Installer"@en-gb ;
    rdfs:comment "An `ies:EventParticipant` where a `ies:ResponsibleActor` has a role in a `building:ConstructionProject`." ;
    rdfs:subClassOf ies:EventParticipant .

building:TMInstaller a rdfs:Class ;
    rdfs:label "TrustMark Installer"@en-gb ;
    rdfs:comment "An `building:Installer` that has been certified under the TrustMark quality scheme." ;
    rdfs:subClassOf building:Installer .

building:TMLicence a rdfs:Class ;
    rdfs:label "TrustMark Licence"@en-gb ;
    rdfs:comment "A `ies:IndividualDocument` certifying the competency and quality workmanship of a TrustMark Registered Business." ;
    rdfs:subClassOf ies:IndividualDocument .

building:TMLicenceNumber a rdfs:Class ;
    rdfs:label "TrustMark Licence Number"@en-gb ;
    rdfs:comment "The licence number a business obtains upon completing the TrustMark certification." ;
    rdfs:subClassOf ies:Identifier .

building:TMIdentifier a rdfs:Class ;
    rdfs:label "TrustMark Identifier"@en-gb ;
    rdfs:comment "A `ies:Identifier` that is used to identify a `building:TrustMarkAssessment`." ;
    rdfs:subClassOf ies:Identifier .

building:hasTMLicence a owl:ObjectProperty ;
    rdfs:label "has TrustMark Licence"@en-gb ;
    rdfs:domain building:TMLicensee ;
    rdfs:range building:TMLicence ;
    rdfs:comment "A relation between a `building:TMInstaller` and an asset (TrustMark licence) in their possession." ;
    rdfs:subPropertyOf ies:inPossessionOf .

building:EnergySupplier a rdfs:Class ;
    rdfs:label "Energy Supplier"@en-gb ;
    rdfs:comment "A business supplying energy to a `building:Structure`. " ;
    rdfs:subClassOf ies:Supplier .

building:ECOSupplier a rdfs:Class ;
    rdfs:label "ECO Supplier"@en-gb ;
    rdfs:comment "An `building:EnergySupplier` that has an obligation under the Energy Company Obligation (ECO) scheme." ;
    rdfs:seeAlso building:ECOSupplierReference ;
    rdfs:subClassOf building:EnergySupplier .

building:ECOSupplierReference a rdfs:Class ;
    rdfs:label "ECO Supplier Reference"@en-gb ;
    rdfs:comment "The `ies:Identifier` of a business supplying energy to a `building:Structure` under the Energy Company Obligation (ECO) scheme." ;
    skos:example "Avro Energy", "British Gas", "Bulb", "E", "EDF Energy", "E.ON Energy", "Green Network", "Green Star", "npower", "Octopus Energy", "OVO", "SSE", "ScottishPower", "Shell Energy (formerly First Utility)", "The Co-operative Energy", "The Utility Warehouse", "Utilita" ;
    rdfs:subClassOf ies:Identifier .

building:StandardAssessmentProcedure a rdfs:Class ;
    rdfs:label "Standard Assessment Procedure"@en-gb ;
    rdfs:comment "The Standard Assessment Procedure (SAP) is the UK Government's recommended method for measuring the energy rating of residential properties." ;
    rdfs:subClassOf building:EnergyPerformanceAssessment     .

building:RdSAP a rdfs:Class ;
    rdfs:label "Reduced Data Standard Assessment Procedure"@en-gb ;
    rdfs:comment "The Reduced Data Standard Assessment Procedure (RdSAP) is a simplified version of the SAP used for residential properties." ;
    skos:note "Often abbreviated rdSAP" ;
    rdfs:subClassOf building:EnergyPerformanceAssessment .

building:RdSAPTransaction a rdfs:Class ;
    rdfs:label "RdSAP Transaction"@en-gb ;
    rdfs:comment "A `ies:BusinessEvent` specifying the purpose for which the RdSAP energy performance assessment is conducted." ;
    rdfs:subClassOf ies:BusinessEvent .

building:ClassOfRenovationProject a rdfs:Class ;
    rdfs:label "Class Of Renovation Project"@en-gb ;
    rdfs:comment "An `ies:ClassOfEvent` that is a classifier of `building:RenovationProject`." ;
    rdfs:subClassOf ies:ClassOfEvent .

building:RdSAPWorkType a rdfs:Class ;
    rdfs:label "RdSAP Work Type"@en-gb ;
    rdfs:comment "The type of renovation project classified according to the RdSAP. Instances of this class are `rdfs:subClassOf` `building:RenovationProject`." ;
    rdfs:subClassOf building:ClassOfRenovationProject .

building:GasSupplySystem a rdfs:Class ;
    rdfs:label "Gas Supply System"@en-gb ;
    skos:altLabel "Gas Services"@en-gb ;
    rdfs:comment "A technical system for the supply of gas to a building." ;
    rdfs:subClassOf building:TechnicalSystem .

building:ElectricitySupplySystem a rdfs:Class ;
    rdfs:label "Building Services Electricity"@en-gb ;
    skos:altLabel "Electricity Services"@en-gb ;
    rdfs:comment "A technical system for the supply of electricity to a building." ;
    rdfs:subClassOf building:TechnicalSystem .

building:HotWaterSupplySystem a rdfs:Class ;
    rdfs:label "Building Services Hot Water"@en-gb ;
    skos:altLabel "Hot Water Services"@en-gb ;
    rdfs:comment "A technical system for the supply of hot water to a building." ;
    rdfs:subClassOf building:TechnicalSystem .

# propertyType in the data dictionary, as specified in RdSAP Appendix S1.
building:ParkHome a building:StructureUnitType ;
    rdfs:label "Park Home"@en-gb ;
    rdfs:comment "An instance `building:StructureType` that is a single-storey, detached residential `building:StructureUnit` situated within private or local authority-run parks." ;
    rdfs:subClassOf building:StructureUnitState .

building:hasPropertyType a owl:ObjectProperty ;
    rdfs:label "has Property Type"@en-gb ;
    rdfs:comment "A relation between a `building:StructureUnitState` and a `building:ClassOfStructureUnitState` that specifies the type of the structure unit as in RdSAP Appendix S1, that is using one instance of `building:StructureUnitType` and one of `building:BuiltForm`." ;
    rdfs:domain building:StructureUnit ;
    rdfs:range building:ClassOfStructureUnitState ;
    rdfs:subPropertyOf ies:relationship .

# PropertyConstruction in the data dictionary refers to PAS 2023-19 Table B.1, criterion 5
# For the following 5 entities, I have used the same design pattern of Class Of Structure Unit State.
building:StructureUnitByRiskGrade a rdfs:Class ;
    rdfs:label "Structure Unit by Risk Grade"@en-gb ;
    rdfs:comment "A `building:ClassOfStructureUnit` that is a classifier of `building:StructureUnit` by the risk grade." ;
    rdfs:subClassOf building:ClassOfStructureUnitState .

building:hasBuiltPart a owl:ObjectProperty ;
    rdfs:label "has Built Part"@en-gb ;
    rdfs:comment "A relationship connecting the state of a built entity to a classifier of a built entity." ;
    rdfs:domain ies:ClassOfState ;
    rdfs:range building:ClassOfBuiltEntity ;
    skos:example "A `building:StructureUnitState` comprises (`building:hasBuiltPart`) a built entity such as `building:CavityWall`." ;
    rdfs:subPropertyOf ies:relationship .

building:Conventional a building:StructureUnitByRiskGrade ;
    rdfs:label "Conventional"@en-gb ;
    rdfs:comment "An instance of `building:StructureUnitByRiskGrade` specified in PAS 2035:19 Table B.1, which means masonry cavity wall construction (brick and/or block) with or without render, tile hanging or other external cladding." ;
    building:hasBuiltPart building:CavityWall ;
    skos:example "Conventional, not high-rise, not protected" ;
    rdfs:subClassOf building:StructureUnitState .

building:Traditional a building:StructureUnitByRiskGrade ;
    rdfs:label "Traditional"@en-gb ;
    rdfs:comment "An instance of `building:StructureUnitByRiskGrade` specified in PAS 2035:19 Table B.1, which means constructed with solid brick or stone walls, or timber-framed walls with any infill." ;
    building:hasBuiltPart building:SolidBrick, building:GraniteOrWhinstone, building:TimberFrame ;
    skos:example "Traditional, not protected" ;
    rdfs:subClassOf building:StructureUnitState .

building:System-Built a building:StructureUnitByRiskGrade ;
    rdfs:label "System-Built"@en-gb ;
    rdfs:comment "An instance of `building:StructureUnitByRiskGrade` specified in PAS 2035:19 Table B.1, which means frame (timber, steel or concrete) and pre-fabricated panel (concrete or timber, or a combination) construct ion, or timber-framed construction with brick or stone external cladding." ;
    building:hasBuiltPart building:SystemBuilt ;
    skos:example "System-built, not high-rise, not protected" ;
    rdfs:subClassOf building:StructureUnitState .

building:HighRise a building:StructureUnitByRiskGrade ;
    rdfs:label "High rise"@en-gb ;
    rdfs:comment "An instance of `building:StructureUnitByRiskGrade` specified in PAS 2035:19 Table B.1, which means over 12 metres or over four storeys in height above the ground." ;
    skos:example "High-rise, any construction" ;
    rdfs:subClassOf building:StructureUnitState .

building:Protected a building:StructureUnitByRiskGrade ;
    rdfs:label "Protected"@en-gb ;
    rdfs:comment "An instance of `building:StructureUnitByRiskGrade` specified in PAS 2035:19 Table B.1, which includes Listed Buildings and buildings in Conservation Areas or World Heritage Sites" ;
    skos:example "Protected, any construction or built form" ;
    rdfs:subClassOf building:StructureUnitState .

building:ConstructionProject a rdfs:Class ;
    rdfs:label "Construction Project"@en-gb ;
    rdfs:comment "An `ies:Event`that is the creation, maintenance, or destruction of a `building:Structure` or `building:StructureUnit`." ;
    rdfs:subClassOf ies:Event .

building:NewBuild a rdfs:Class ;
    rdfs:label "New Build"@en-gb ;
    rdfs:comment "A `building:ConstructionProject` that covers the construction of a new `building:structure`s." ;
    rdfs:subClassOf building:ConstructionProject .

building:Demolition a rdfs:Class ;
    rdfs:label "Demolition"@en-gb ;
    rdfs:comment "A `building:ConstructionProject` that covers the destruction of existing `building:structure`s." ;
    rdfs:subClassOf building:ConstructionProject .

building:RenovationProject a rdfs:Class ;
    rdfs:label "Renovation Project"@en-gb ;
    rdfs:comment "A `building:ConstructionProject` covering the modification of existing `building:structure`s." ;
    ies:powertype building:ClassOfRenovationProject ;
    rdfs:subClassOf building:ConstructionProject .

building:EnergyEfficiencyProject a building:RdSAPWorkType ;
    rdfs:label "Energy Efficiency Project"@en-gb ;
    rdfs:comment "A specific type of `building:RenovationProject` aiming to improve the energy efficiency." ;
    rdfs:subClassOf building:RenovationProject .

building:RepairMaintenanceImprovement a building:RdSAPWorkType ;
    rdfs:label "Repair Maintenance and Improvement"@en-gb ;
    rdfs:comment "A generic type of `building:RenovationProject` aiming to repair, maintain, or improve existing `building:structure`s." ;
    rdfs:subClassOf building:RenovationProject .

building:OtherProject a building:RdSAPWorkType ;
    rdfs:label "Other Project"@en-gb ;
    rdfs:comment "A `building:RenovationProject` that does not fit into the other categories." ;
    rdfs:subClassOf building:RenovationProject .

############################################  Event replacement for measures ########################
### Fabric insulation

building:ImproveCavityWallInsulation
    a rdfs:Class ;
    rdfs:subClassOf building:EnergyEfficiencyProject ;
    rdfs:label "Improve cavity wall insulation"@en-gb ;
    skos:note "Coverage: Both. PAS/TM: Cavity Wall Insulation; RdSAP: Cavity wall insulation."@en-gb .

building:ImproveSolidWallInsulationInternal
    a rdfs:Class ;
    rdfs:subClassOf building:EnergyEfficiencyProject ;
    rdfs:label "Improve solid wall insulation – internal (IWI)"@en-gb ;
    skos:note "Coverage: Both. PAS/TM: Solid Wall Insulation (internal); RdSAP: Solid wall insulation (internal)."@en-gb .

building:ImproveSolidWallInsulationExternal
    a rdfs:Class ;
    rdfs:subClassOf building:EnergyEfficiencyProject ;
    rdfs:label "Improve solid wall insulation – external (EWI)"@en-gb ;
    skos:note "Coverage: Both. PAS/TM: Solid Wall Insulation (external); RdSAP: Solid wall insulation (external)."@en-gb .

building:ImproveLoftInsulation
    a rdfs:Class ;
    rdfs:subClassOf building:EnergyEfficiencyProject ;
    rdfs:label "Improve loft insulation"@en-gb ;
    skos:note "Coverage: Both. PAS/TM: Roof/Loft insulation; RdSAP: Loft insulation."@en-gb .

building:ImproveRoomInRoofInsulation
    a rdfs:Class ;
    rdfs:subClassOf building:EnergyEfficiencyProject ;
    rdfs:label "Improve room-in-roof insulation"@en-gb ;
    skos:note "Coverage: Both. PAS/TM: Room-in-roof; RdSAP: Room-in-roof insulation."@en-gb .

building:ImproveFloorInsulation
    a rdfs:Class ;
    rdfs:subClassOf building:EnergyEfficiencyProject ;
    rdfs:label "Improve floor insulation"@en-gb ;
    skos:note "Coverage: Both. PAS/TM: Floor insulation; RdSAP: Floor insulation."@en-gb .

building:ImproveParkHomeInsulation
    a rdfs:Class ;
    rdfs:subClassOf building:EnergyEfficiencyProject ;
    rdfs:label "Improve park home insulation"@en-gb ;
    skos:note "Coverage: TM-primary (RdSAP special). PAS/TM: Park Home Insulation; RdSAP: Modelled per conventions, limited/conditional."@en-gb .

### Glazing & doors

building:UpgradeWindowsDoubleOrTripleGlazing
    a rdfs:Class ;
    rdfs:subClassOf building:EnergyEfficiencyProject ;
    rdfs:label "Upgrade windows (double/triple glazing)"@en-gb ;
    skos:note "Coverage: Both. PAS/TM: Windows; RdSAP: Glazing improvements."@en-gb .

building:UpgradeExternalDoors
    a rdfs:Class ;
    rdfs:subClassOf building:EnergyEfficiencyProject ;
    rdfs:label "Upgrade external doors"@en-gb ;
    skos:note "Coverage: Both (limited in RdSAP). PAS/TM: Doors; RdSAP: Door improvements variably represented via U-values/assumptions."@en-gb .

### Heating

building:ReplaceBoiler
    a rdfs:Class ;
    rdfs:subClassOf building:EnergyEfficiencyProject ;
    rdfs:label "Replace boiler"@en-gb ;
    skos:note "Coverage: Both. PAS/TM: Boiler; RdSAP: Boiler replacement improvement."@en-gb .

building:InstallAirSourceHeatPump
    a rdfs:Class ;
    rdfs:subClassOf building:EnergyEfficiencyProject ;
    rdfs:label "Install air source heat pump (ASHP)"@en-gb ;
    skos:note "Coverage: Both. PAS/TM: Other Heating/Microgeneration; RdSAP 10: Heat pumps supported."@en-gb .

building:InstallGroundSourceHeatPump
    a rdfs:Class ;
    rdfs:subClassOf building:EnergyEfficiencyProject ;
    rdfs:label "Install ground source heat pump (GSHP)"@en-gb ;
    skos:note "Coverage: Both. PAS/TM: Other Heating/Microgeneration; RdSAP 10: Heat pumps supported."@en-gb .

building:UpgradeHeatingControls
    a rdfs:Class ;
    rdfs:subClassOf building:EnergyEfficiencyProject ;
    rdfs:label "Upgrade heating controls (programmer/room stat/TRVs/zoning/compensation)"@en-gb ;
    skos:note "Coverage: Both. PAS/TM: Controls under building services; RdSAP: Heating control improvements."@en-gb .

building:InstallOrUpgradeElectricStorageHeating
    a rdfs:Class ;
    rdfs:subClassOf building:EnergyEfficiencyProject ;
    rdfs:label "Install or upgrade electric storage heating (incl. high heat retention)"@en-gb ;
    skos:note "Coverage: Both. PAS/TM: Electric Storage Heating; RdSAP: Electric storage heating options."@en-gb .

building:ConnectToOrUpgradeDistrictHeatingIncluding
    a rdfs:Class ;
    rdfs:subClassOf building:EnergyEfficiencyProject ;
    rdfs:label "Connect to or upgrade district heating (incl. HIU)"@en-gb ;
    skos:note "Coverage: Both. PAS/TM: District Heating; RdSAP: Community/district heating options."@en-gb .

building:UpgradeSecondaryHeating
    a rdfs:Class ;
    rdfs:subClassOf building:EnergyEfficiencyProject ;
    rdfs:label "Upgrade secondary heating (e.g. room heater, gas/electric fire, wood stove)"@en-gb ;
    skos:note "Coverage: RdSAP-primary (TM other heating). PAS/TM: Other Heating; RdSAP: Secondary heating recognised, limited improvement recommendations."@en-gb .

### Hot water

building:InsulateHotWaterCylinder
    a rdfs:Class ;
    rdfs:subClassOf building:EnergyEfficiencyProject ;
    rdfs:label "Insulate hot water cylinder"@en-gb ;
    skos:note "Coverage: Both. PAS/TM: Hot water; RdSAP: Cylinder insulation improvement."@en-gb .

building:UpgradeHotWaterSystemOrControls
    a rdfs:Class ;
    rdfs:subClassOf building:EnergyEfficiencyProject ;
    rdfs:label "Upgrade hot water system / controls"@en-gb ;
    skos:note "Coverage: Both. PAS/TM: Hot water; RdSAP: Efficient water heating / controls where supported."@en-gb .

### Ventilation & airtightness

building:InstallMechanicalExtractVentilation
    a rdfs:Class ;
    rdfs:subClassOf building:EnergyEfficiencyProject ;
    rdfs:label "Install mechanical extract ventilation (MEV)"@en-gb ;
    skos:note "Coverage: TM-primary (RdSAP partial). PAS/TM: Ventilation systems; RdSAP 10: Expanded inputs; improvement recommendation may be indirect."@en-gb .

building:InstallMechanicalVentilationWithHeatRecovery
    a rdfs:Class ;
    rdfs:subClassOf building:EnergyEfficiencyProject ;
    rdfs:label "Install mechanical ventilation with heat recovery (MVHR)"@en-gb ;
    skos:note "Coverage: TM-primary (RdSAP partial). PAS/TM: Heat recovery/MVHR; RdSAP 10: Partial/indirect handling."@en-gb .

building:EnhanceAirtightness
    a rdfs:Class ;
    rdfs:subClassOf building:EnergyEfficiencyProject ;
    rdfs:label "Enhance airtightness (fabric sealing)"@en-gb ;
    skos:note "Coverage: TM-primary (RdSAP input). PAS/TM: Fabric QA; RdSAP 10: Accepts measured air test, but not typically a standalone recommendation."@en-gb .

### Renewables & storage

building:InstallSolarPhotovoltaics
    a rdfs:Class ;
    rdfs:subClassOf building:EnergyEfficiencyProject ;
    rdfs:label "Install solar photovoltaics (PV)"@en-gb ;
    skos:note "Coverage: Both. PAS/TM: Micro-Generation; RdSAP: Solar PV improvement."@en-gb .

building:InstallSolarThermalHotWater
    a rdfs:Class ;
    rdfs:subClassOf building:EnergyEfficiencyProject ;
    rdfs:label "Install solar thermal hot water"@en-gb ;
    skos:note "Coverage: Both. PAS/TM: Micro-Generation; RdSAP: Solar hot water improvement."@en-gb .

building:InstallBatteryStorage
    a rdfs:Class ;
    rdfs:subClassOf building:EnergyEfficiencyProject ;
    rdfs:label "Install battery storage"@en-gb ;
    skos:note "Coverage: TM-only. PAS/TM: Storage referenced; RdSAP: Generally not directly modelled."@en-gb .

### Lighting

building:UpgradeLightingLowEnergy
    a rdfs:Class ;
    rdfs:subClassOf building:EnergyEfficiencyProject ;
    rdfs:label "Upgrade lighting (low-energy lamps/fixtures)"@en-gb ;
    skos:note "Coverage: Both. PAS/TM: Lighting; RdSAP: Low energy lighting improvement."@en-gb .

### Appliances

building:ReplaceOrServiceAppliancesEfficientModels
    a rdfs:Class ;
    rdfs:subClassOf building:EnergyEfficiencyProject ;
    rdfs:label "Replace or service appliances (efficient models)"@en-gb ;
    skos:note "Coverage: TM-only. PAS/TM: Appliance intervention area; RdSAP: Appliances not modelled."@en-gb .


#################################### end measure replacement #########################

building:RenovationProjectTarget a rdfs:Class ;
    rdfs:label "Renovation Project Intervention Target" ;
    rdfs:comment "An `ies:EventParticipant` that is the expected target `ies:Entity` at which the `building:RenovationTarget` is aimed. " ;
    rdfs:subClassOf ies:EventParticipant .

################################ Describe the area for wind driven rain ###############################
### Genus
building:ExposureZoneLocation
    a rdfs:Class ;
    rdfs:subClassOf ies:Location ;
    rdfs:label "Exposure zone location"@en-gb ;
    rdfs:comment "A location classified by its characteristic exposure to wind-driven rain, used to judge suitability and detailing requirements for fabric interventions (e.g., cavity wall insulation) per UK practice informed by BS 8104."@en-gb .

### Zone 1
building:Zone1Location
    a rdfs:Class ;
    rdfs:subClassOf building:ExposureZoneLocation ;
    rdfs:label "Exposure Zone 1 (sheltered/low)"@en-gb ;
    rdfs:comment "An ExposureZoneLocation that is characterised by LOW wind-driven rain exposure, typically inland, sheltered by surrounding terrain/urban form, and away from prevailing-wind coasts; contrasted with Zone 2–4 by materially lower façade wetting risk. Retrofit implication: fabric measures (including CWI) generally suitable where substrate and detailing comply with specification."@en-gb .

### Zone 2
building:Zone2Location
    a rdfs:Class ;
    rdfs:subClassOf building:ExposureZoneLocation ;
    rdfs:label "Exposure Zone 2 (moderate)"@en-gb ;
    rdfs:comment "An ExposureZoneLocation that is characterised by MODERATE wind-driven rain exposure, commonly in reasonably open inland contexts without pronounced coastal or ridge exposure; contrasted with Zone 1 by greater façade wetting and with Zone 3–4 by absence of persistent severe exposure. Retrofit implication: CWI typically suitable subject to sound walls, verified cavities/ties, and compliant detailing/QA."@en-gb .

### Zone 3
building:Zone3Location
    a rdfs:Class ;
    rdfs:subClassOf building:ExposureZoneLocation ;
    rdfs:label "Exposure Zone 3 (high)"@en-gb ;
    rdfs:comment "An ExposureZoneLocation that is characterised by HIGH wind-driven rain exposure, often near windward coasts, elevated/open sites, or large unobstructed façades; contrasted with Zones 1–2 by sustained higher façade wetting and with Zone 4 by less extreme conditions. Retrofit implication: CWI only with specifically suitable systems and enhanced detailing/QA (e.g., appropriate beads/binders, closers/vents, verified cavity condition) and robust aftercare."@en-gb .

### Zone 4
building:Zone4Location
    a rdfs:Class ;
    rdfs:subClassOf building:ExposureZoneLocation ;
    rdfs:label "Exposure Zone 4 (severe/very high)"@en-gb ;
    rdfs:comment "An ExposureZoneLocation that is characterised by SEVERE wind-driven rain exposure, typically highly exposed coastal frontages, headlands, ridges, or fully open sites to prevailing winds; contrasted with Zones 1-3 by consistently extreme façade wetting. Retrofit implication: CWI may be unsuitable or restricted to specific certified systems with stringent moisture-risk design and maintenance; consider alternatives such as EWI/IWI subject to hygrothermal assessment."@en-gb .

building:CombustionVentilationAcceptable a rdfs:Class ;
    rdfs:label "Combustion Ventilation Acceptable"@en-gb ;
    rdfs:comment "A `building:AssessHeatingSystem` establishing if the ventilation for combustion processes is acceptable or not." ;
    rdfs:subClassOf building:AssessHeatingSystem .


building:DestructiveTestsConducted a rdfs:Class ;
    rdfs:label "Destructive Tests Conducted"@en-gb ;
    rdfs:comment "A `ies:Assessment` using destructive methods to investigate the state of a building." ;
    rdfs:subClassOf ies:Assessment .

building:OccupancyState a rdfs:Class ;
    rdfs:label "Occupancy State"@en-gb ;
    rdfs:comment "A temporal state of a `building:ResidentialDwelling` describing whether or not it is occupied by one or more persons." ;
    rdfs:subClassOf building:StructureUnitOrSpaceState   .

building:NumberOfOccupants a rdfs:Class ;
    rdfs:label "Number of Occupants"@en-gb ;
    rdfs:comment "The number of occupants in a `building:StructureUnit`." ;
    rdfs:subClassOf ies:Measure .

building:hasNumberOfOccupants a owl:ObjectProperty ;
    rdfs:label "has number of Occupants"@en-gb ;
    rdfs:comment "A relation connecting a `building:StructureUnitOrSpaceState` to its `building:NumberOfOccupants`." ;
    rdfs:domain building:StructureUnitOrSpaceState ;
    rdfs:range building:NumberOfOccupants ;
    rdfs:subPropertyOf ies:relationship .

##################### quick test ####################

ex:MyHome a building:StructureUnit, building:House .
ex:MyHomeOnCensusDay a building:OccupancyState ;
    ies:isStateOf ex:MyHome ;
    building:hasNumberOfOccupants [
        a building:NumberOfOccupants ;
        building:hasQuantity [
            a qudt:QuantityValue ;
            qudt:numericValue 3 ;
            qudt:unit unit:UNITLESS
    ]] .

#######################################

building:RRN a rdfs:Class ;
    rdfs:label "RRN"@en-gb ;
    rdfs:comment "The report reference number (RRN) for Energy Performance Certificates & Recommendations reports, Action Plans, Display Energy Certificates & Advisory Reports held on the Scottish Energy Performance Certificate Register." ;
    rdfs:seeAlso <https://www.scottishepcregister.org.uk/> ;
    rdfs:subClassOf ies:Identifier .

# building:ExistingVentilationProvided a rdfs:Class ;
#     rdfs:label "Existing Ventilation Provided"@en-gb ;
#     rdfs:comment "A `building:StructureUnitState` asserting whether the ventilation provided in a building is acceptable or not." ;
#     rdfs:subClassOf building:StructureUnitState .

building:CentralisedMechanicalExtractVentilation a rdfs:Class ;
    rdfs:label "Centralised Mechanical Extract Ventilation"@en-gb ;
    skos:altLabel "Centralised MEV"@en-gb ;
    rdfs:comment "A `building:VentilationSystem` that has centralised the mechanical systems required to extract air." ;
    rdfs:subClassOf building:VentilationSystem .

building:ContinuousMechanicalExtractVentilation a rdfs:Class ;
    rdfs:label "Continuous Mechanical Extract Ventilation"@en-gb ;
    skos:altLabel "CMEV"@en-gb ;
    rdfs:comment "A `building:VentilationSystem` where the mechanical systems that extract air operate continuously." ;
    rdfs:subClassOf building:VentilationSystem .

building:IntermittentExtractVentilation a rdfs:Class ;
    rdfs:label "Intermittent Extract Ventilation"@en-gb ;
    skos:altLabel "IEV"@en-gb ;
    rdfs:comment "A `building:VentilationSystem` where the mechanical systems that extract air operate intermittently." ;
    rdfs:subClassOf building:VentilationSystem .

building:MechanicalVentilationHeatRecovery a rdfs:Class ;
    rdfs:label "Mechanical Ventilation Heat Recovery"@en-gb ;
    skos:altLabel "MVHR"@en-gb ;
    rdfs:comment "A `building:VentilationSystem` that recovers heat from the extracted air." ;
    rdfs:subClassOf building:VentilationSystem .

building:PassiveStackVentilation a rdfs:Class ;
    rdfs:label "Passive Stack Ventilation"@en-gb ;
    skos:altLabel "PSV"@en-gb ;
    rdfs:comment "A `building:VentilationSystem` that ses differences in air temperature and pressure to move stale air out of a building and draw in fresh air—without the need for mechanical fans." ;
    rdfs:subClassOf building:VentilationSystem .

building:PositiveInputVentilation a rdfs:Class ;
    rdfs:label "Positive Input Ventilation"@en-gb ;
    skos:altLabel "PIV"@en-gb ;
    rdfs:comment "A `building:VentilationSystem` that uses a small, low-energy fan to push filtered fresh air into a building." ;
    rdfs:subClassOf building:VentilationSystem .

building:ClassOfTechnicalSystemState a rdfs:Class ;
    rdfs:label "Class of Technical System State"@en-gb ;
    rdfs:comment "An `ies:ClassOfState` that is a classifier and powertype of `building:TechnicalSystemState`, i.e. instances of this class are `rdfs:subClassOf building:StructureUnitState`." ;
    rdfs:subClassOf ies:ClassOfState .

building:PreRetrofitPulseAirTightnessTestRating a rdfs:Class ;
    rdfs:label "Pre-Retrofit Pulse Air Tightness Test Rating"@en-gb ;
    rdfs:comment "A `building:ClassOfTechnicalSystemState` that is a classifier for ventilation systems. It is the rating obtained from tests conducted before a retrofit project to assess the air tightness of a building." ;
    rdfs:subClassOf building:ClassOfTechnicalSystemState .

building:PreRetrofitBlowerDoorAirTightnessTestRating a rdfs:Class ;
    rdfs:label "Pre-Retrofit Blower Door Air Tightness Test Rating"@en-gb ;
    rdfs:comment "A `building:ClassOfTechnicalSystemState` that is a classifier for ventilation systems. It is the rating obtained from blower door tests conducted before a retrofit project to assess the air tightness of a building." ;
    rdfs:subClassOf building:ClassOfTechnicalSystemState .

building:SuitableBackgroundVentilationPresent a rdfs:Class ;
    rdfs:label "Suitable Background Ventilation Present"@en-gb ;
    rdfs:comment "A `building:EnergyPerformanceAssessmentResult` asserting whether the background ventilation in a building is suitable or not. Background ventilators are air inlets, commonly known as trickle ventilators." ;
    rdfs:subClassOf building:EnergyPerformanceAssessmentResult .

building:AppraisalOfHeritage a rdfs:Class ;
    rdfs:label "Appraisal of Heritage"@en-gb ;
    rdfs:comment "A `building:EnergyPerformanceAssessmentResult` asserting the appraisal of the dwelling's heritage, architectural features, structure, construction and condition and the installed building services (ventilation, heating, hot water and lighting) in sufficient detail to establish the suitability of the dwelling for improvement" ;
    rdfs:subClassOf building:EnergyPerformanceAssessmentResult .

building:assessedEachStateOf a owl:ObjectProperty ;
    rdfs:label "assessed Each State Of"@en-gb ;
    rdfs:comment "The relation between an assessment and a class of states if and only if the assessment has as target a class of states." ;
    rdfs:domain ies:Assessment ;
    rdfs:range ies:ClassOfState .

building:Bedroom a rdfs:Class ;
    rdfs:label "Bedroom"@en-gb ;
    rdfs:comment "A `building:Room` that is used primarily for sleeping." ;
    rdfs:subClassOf building:Room .

building:ClassOfBedroom a rdfs:Class ;
    rdfs:label "Class of Bedroom"@en-gb ;
    rdfs:comment "A `building:ClassOfSpace` that is a classifier of `building:Bedroom`. Instances of this class are `rdfs:subClassOf building:Bedroom`." ;
    rdfs:subClassOf building:ClassOfSpace .

building:AllBedroomsInAStructureUnit a rdfs:Class ;
    rdfs:label "All Bedrooms In A Structure Unit"@en-gb ;
    rdfs:comment "An entity representing the collection of all `building:Bedroom` instances located within a `building:StructureUnit`. Useful for reasoning over or querying aggregate sets of structure units in a built environment." ;
    rdfs:subClassOf ies:FiniteClassOfElement, building:ClassOfBedroom .


############ New fuel portions ######################
building:EnergySourcePortion a rdfs:Class ;
    rdfs:label "Portion of Energy Source" ;
    rdfs:comment "A `building:StuffPortion` that can be used for releasing energy for various usages" ;
    ies:powertype building:ClassOfEnergySourcePortion ;
    rdfs:subClassOf building:StuffPortion ;
    ies:eachMemberIsPartOfSomeMemberOf ies:Stuff .

building:ClassOfEnergySourcePortion a rdfs:Class ;
    rdfs:label "Class Of Portion Of Energy Source" ;
    rdfs:comment "An `ies:ClassOfElement that is a classifier of `building:EnergySourcePortion`.  Instances of this class are `rdfs:subClass(es)Of` `building:EnergySourcePortion`." ;
    rdfs:subClassOf ies:ClassOfElement .

building:FuelPortion a rdfs:Class ;
    rdfs:label "Fuel Portion" ;
    rdfs:comment "A portion of energy source that can be used for releasing energy by making it undergo a chemical or nuclear reaction" ;
    rdfs:subClassOf building:EnergySourcePortion ;
    ies:powertype building:ClassOfFuelPortion ;
    ies:eachMemberIsPartOfSomeMemberOf ies:Stuff .

building:ClassOfFuelPortion a rdfs:Class ;
    rdfs:label "Class Of Fuel Portion" ;
    rdfs:comment "An `ies:ClassOfElement that is a classifier of `building:FuelPortion`.  Instances of this class are `rdfs:subClass(es)Of` `building:FuelPortion`." ;
    rdfs:subClassOf building:ClassOfEnergySourcePortion .

building:FossilFuelPortion a rdfs:Class, building:ClassOfFuelPortion ;
    rdfs:label "Fossil Fuel Portion" ;
    rdfs:comment "A portion of fuel formed from the remains of ancient plants and animals, such as coal, oil, or natural gas." ;
    rdfs:subClassOf building:NonRenewableEnergySourcePortion .

building:SolidFossilFuelPortion a rdfs:Class, building:ClassOfFuelPortion ;
    rdfs:label "Solid Fossil Fuel Portion" ;
    rdfs:comment "A portion of fossil fuel that is in a solid state at standard temperature and pressure, such as coal or lignite." ;
    ies:eachMemberIsPartOfSomeMemberOf ies:Stuff ;
    rdfs:subClassOf building:FossilFuelPortion .

building:LiquidFossilFuelPortion a rdfs:Class, building:ClassOfFuelPortion ;
    rdfs:label "Liquid Fossil Fuel Portion" ;
    rdfs:comment "A portion of fossil fuel that is in a liquid state at standard temperature and pressure, such as gasoline or diesel." ;
    ies:eachMemberIsPartOfSomeMemberOf ies:Stuff ;
    rdfs:subClassOf building:FossilFuelPortion .
building:KerosenePortion a rdfs:Class, building:ClassOfFuelPortion ;
    rdfs:label "Kerosene Portion" ;
    rdfs:comment "A portion of `building:LiquidFossilFuel` that is distilled from crude oil, typically used for heating, lighting, and as jet fuel." ;
    rdfs:subClassOf building:LiquidFossilFuelPortion .

building:GaseousFossilFuelPortion a rdfs:Class, building:ClassOfFuelPortion ;
    rdfs:label "Gaseous Fossil Fuel Portion" ;
    rdfs:comment "A portion of fossil fuel that is in a gaseous state at standard temperature and pressure, such as natural gas or propane." ;
    ies:eachMemberIsPartOfSomeMemberOf ies:Stuff ;
    rdfs:subClassOf building:FossilFuelPortion .

building:RenewableEnergySourcePortion a rdfs:Class, building:ClassOfEnergySourcePortion ;
    rdfs:label "Renewable Energy Source" ;
    rdfs:comment "A portion of an energy source where an equivalent portion can be replenished on a human timescale, such as solar, wind, rain, tides, waves, and geothermal heat." ;
    rdfs:subClassOf building:EnergySourcePortion .

building:NonRenewableEnergySourcePortion a rdfs:Class, building:ClassOfEnergySourcePortion ;
    rdfs:label "Non-Renewable Energy Source Portion";
    rdfs:comment "A portion of an energy source that is produced from fuels that are consumed faster than they can be replaced by natural means or whose use and consumption is unsustainable for the foreseeable future." ;
    rdfs:subClassOf building:EnergySourcePortion .

building:PartiallyRenewableEnergySourcePortion a rdfs:Class, building:ClassOfEnergySourcePortion ;
    rdfs:label "Partially Renewable Energy Source" ;
    rdfs:comment "A `building:EnergySourcePortion` derived from a mixture of renewable and non-renewable sources, such as a blend of biodiesel and fossil-derived kerosene." ;
    rdfs:subClassOf building:EnergySourcePortion .

building:B30K_FuelPortion a rdfs:Class, building:ClassOfEnergySourcePortion ;
    rdfs:label "B30K Fuel Portion" ;
    rdfs:comment "A `building:PartiallyRenewableEnergySourcePortion` that is a liquid fuel blend consisting of 30% FAME biodiesel and 70% kerosene by volume, making it partially renewable." ;
    rdfs:subClassOf building:PartiallyRenewableEnergySourcePortion ;
    ies:eachMemberHasPartSomeMemberOf building:FAME, building:Kerosene .

building:BiomassPortion a rdfs:Class, building:ClassOfEnergySourcePortion ;
    rdfs:label "Biomass Portion" ;
    rdfs:comment "A portion of renewable energy source derived from organic matter, such as wood, crops, or waste." ;
    rdfs:subClassOf building:RenewableEnergySourcePortion .

building:BiofuelPortion a rdfs:Class, building:ClassOfFuelPortion ;
    rdfs:label "Biofuel Portion" ;
    rdfs:comment "A portion of fuel derived directly from living matter (biomass)." ;
    rdfs:subClassOf building:BiomassPortion .

building:SolidBiofuelPortion a rdfs:Class, building:ClassOfFuelPortion ;
    rdfs:label "Solid Biofuel Portion" ;
    rdfs:comment "A portion of biofuel that is in a solid state at standard temperature and pressure, such as wood pellets or charcoal." ;
    ies:eachMemberIsPartOfSomeMemberOf ies:Stuff ;
    rdfs:subClassOf building:BiofuelPortion .

building:LiquidBiofuelPortion a rdfs:Class, building:ClassOfFuelPortion ;
    rdfs:label "Liquid Biofuel Portion" ;
    rdfs:comment "A portion of biofuel that is in a liquid state at standard temperature and pressure, such as bioethanol or biodiesel." ;
    ies:eachMemberIsPartOfSomeMemberOf ies:Stuff ;
    rdfs:subClassOf building:BiofuelPortion .

building:FAME a rdfs:Class, building:ClassOfFuelPortion ;
    rdfs:label "FAME" ;
    rdfs:comment "A liquid biofuel consisting of fatty acid methyl esters, produced from vegetable oils or animal fats via transesterification." ;
    ies:eachMemberIsPartOfSomeMemberOf ies:Stuff ;
    rdfs:subClassOf building:LiquidBiofuelPortion .

building:GaseousBiofuelPortion a rdfs:Class, building:ClassOfFuelPortion ;
    rdfs:label "Gaseous Biofuel Portion" ;
    rdfs:comment "A portion of biofuel that is in a gaseous state at standard temperature and pressure, such as biogas or syngas." ;
    ies:eachMemberIsPartOfSomeMemberOf ies:Stuff ;
    rdfs:subClassOf building:BiofuelPortion .

building:ElectricityPortion a rdfs:Class, building:ClassOfEnergySourcePortion ;
    rdfs:label "Electricity Portion" ;
    rdfs:comment "A quantity of energy resulting from the flow of electric charge, which is a secondary energy source." ;
    rdfs:subClassOf building:EnergySourcePortion .

building:SolarEnergyPortion a rdfs:Class, building:ClassOfEnergySourcePortion ;
    rdfs:label "Solar Energy Portion" ;
    rdfs:comment "A portion of renewable energy derived from the sun's radiation." ;
    rdfs:subClassOf building:RenewableEnergySourcePortion .

building:WindEnergyPortion a rdfs:Class, building:ClassOfEnergySourcePortion ;
    rdfs:label "Wind Energy Portion" ;
    rdfs:comment "A portion of renewable energy derived from the movement of air." ;
    rdfs:subClassOf building:RenewableEnergySourcePortion .

building:HydroEnergyPortion a rdfs:Class, building:ClassOfEnergySourcePortion ;
    rdfs:label "Hydro Energy Portion" ;
    rdfs:comment "A portion of renewable energy derived from the movement of water." ;
    rdfs:subClassOf building:RenewableEnergySourcePortion .

building:GeothermalEnergyPortion a rdfs:Class, building:ClassOfEnergySourcePortion ;
    rdfs:label "Geothermal Energy Portion" ;
    rdfs:comment "A portion of renewable energy derived from heat within the Earth." ;
    rdfs:subClassOf building:RenewableEnergySourcePortion .

building:NuclearEnergyPortion a rdfs:Class, building:ClassOfEnergySourcePortion ;
    rdfs:label "Nuclear Energy Portion" ;
    rdfs:comment "A quantity of energy released from atomic nuclei, via fission or fusion." ;
    rdfs:subClassOf building:NonRenewableEnergySourcePortion .

building:WoodPortion a rdfs:Class, building:ClassOfFuelPortion ;
    rdfs:label "Wood Portion" ;
    rdfs:comment "A portion of solid biofuel derived from trees." ;
    ies:eachMemberIsPartOfSomeMemberOf ies:Stuff ;
    rdfs:subClassOf building:SolidBiofuelPortion .

building:WoodChipsPortion a rdfs:Class, building:ClassOfFuelPortion ;
    rdfs:label "Wood Chips Portion" ;
    rdfs:comment "A portion of solid biofuel consisting of small pieces of wood." ;
    ies:eachMemberIsPartOfSomeMemberOf ies:Stuff ;
    rdfs:subClassOf building:SolidBiofuelPortion .

building:WoodPelletsPortion a rdfs:Class, building:ClassOfFuelPortion ;
    rdfs:label "Wood Pellets Portion" ;
    rdfs:comment "A portion of solid biofuel made from compressed sawdust or other wood waste." ;
    ies:eachMemberIsPartOfSomeMemberOf ies:Stuff ;
    rdfs:subClassOf building:SolidBiofuelPortion .

building:CoalPortion a rdfs:Class, building:ClassOfFuelPortion ;
    rdfs:label "Coal Portion" ;
    rdfs:comment "A combustible sedimentary rock containing more than 50% by weight (or 70% by volume) of carbonaceous matter derived from plant material, typically found in underground deposits and widely used as a fuel." ;
    ies:eachMemberIsPartOfSomeMemberOf ies:Stuff ;
    rdfs:subClassOf building:SolidFossilFuelPortion .

building:AnthracitePortion a rdfs:Class, building:ClassOfFuelPortion ;
    rdfs:label "Anthracite Portion" ;
    rdfs:comment "A hard, high-rank coal containing more than 86% fixed carbon on a dry, mineral-matter-free basis, with a high lustre, low volatile matter, and the highest energy content of all coal types." ;
    ies:eachMemberIsPartOfSomeMemberOf ies:Stuff ;
    rdfs:subClassOf building:CoalPortion .

building:SmokelessCoalPortion a rdfs:Class, building:ClassOfFuelPortion ;
    rdfs:label "Smokeless Coal Portion" ;
    rdfs:comment "A coal portion that has been treated to remove the volatile compounds that produce smoke when burned." ;
    ies:eachMemberIsPartOfSomeMemberOf ies:Stuff ;
    rdfs:subClassOf building:CoalPortion .

building:BituminousCoalPortion a rdfs:Class, building:ClassOfFuelPortion ;
    rdfs:label "Bituminous Coal Portion" ;
    rdfs:comment "A relatively soft coal containing a tar-like substance called bitumen or asphalt. It is of lower rank than anthracite and higher than lignite." ;
    ies:eachMemberIsPartOfSomeMemberOf ies:Stuff ;
    rdfs:subClassOf building:CoalPortion .

building:LPGPortion a rdfs:Class, building:ClassOfFuelPortion ;
    rdfs:label "LPG Portion" ;
    rdfs:comment "Liquefied petroleum gas; a flammable mixture of hydrocarbon gases used as fuel in heating appliances, cooking equipment, and vehicles." ;
    ies:eachMemberIsPartOfSomeMemberOf ies:Stuff ;
    rdfs:subClassOf building:GaseousFossilFuelPortion .

building:NaturalGasPortion a rdfs:Class, building:ClassOfFuelPortion ;
    rdfs:label "Natural Gas Portion" ;
    rdfs:comment "A naturally occurring hydrocarbon gas mixture consisting primarily of methane, but commonly including varying amounts of other higher alkanes, and sometimes a small percentage of carbon dioxide, nitrogen, hydrogen sulfide, or helium." ;
    ies:eachMemberIsPartOfSomeMemberOf ies:Stuff ;
    rdfs:subClassOf building:GaseousFossilFuelPortion .

building:MainsGasPortion a rdfs:Class, building:ClassOfFuelPortion, building:ClassOfEnergySourcePortion ;
    rdfs:label "Mains Gas Portion" ;
    rdfs:comment "A portion of gaseous fossil fuel supplied through the UK national gas grid, consisting primarily of natural gas (methane) sourced from fossil reserves, but which may include a small proportion of biomethane or other renewable gaseous fuels." ;
    ies:eachMemberIsPartOfSomeMemberOf ies:Stuff ;
    rdfs:subClassOf building:GaseousFossilFuelPortion .

building:BiodieselPortion a rdfs:Class, building:ClassOfFuelPortion ;
    rdfs:label "Biodiesel Portion" ;
    rdfs:comment "A biodegradable fuel derived from vegetable oils or animal fats." ;
    ies:eachMemberIsPartOfSomeMemberOf ies:Stuff ;
    rdfs:subClassOf building:LiquidBiofuelPortion .

building:BiogasPortion a rdfs:Class, building:ClassOfFuelPortion ;
    rdfs:label "Biogas Portion" ;
    rdfs:comment "A mixture of gases, primarily consisting of methane and carbon dioxide, produced from raw materials such as agricultural waste, manure, municipal waste, plant material, sewage, green waste or food waste." ;
    ies:eachMemberIsPartOfSomeMemberOf ies:Stuff ;
    rdfs:subClassOf building:GaseousBiofuelPortion .

###################### OS Data Extension ########################
building:AccessPoint a rdfs:Class ;
    rdfs:label "Access Point" ;
    ies:powertype building:ClassOfAccessPoint ;
    rdfs:comment "A `building:BuiltEntity` that allows pedestrian or vehicular access to or from a site, consistent with Ordnance Survey's 'Site Access Location' concept." ;
    rdfs:subClassOf building:AccessPointState,
        building:BuiltEntity .

building:AccessPointState a rdfs:Class ;
    rdfs:label "Access Point State" ;
    ies:powertype building:ClassOfAccessPointState ;
    rdfs:comment "A temporal state of a `building:AccessPoint`." ;
    rdfs:subClassOf building:BuiltEntityState .

building:ClassOfAccessPoint a rdfs:Class ;
    rdfs:label "Class of Access Point Location" ;
    rdfs:comment "An `building:ClassOfLocation` that acts as a classifier for types of AccessPoint, e.g., pedestrian-only access, vehicular access, or mixed-use access points." ;
    rdfs:subClassOf building:ClassOfBuiltEntity .

building:ClassOfAccessPointState a rdfs:Class ;
    rdfs:label "Class of Access Point State" ;
    rdfs:comment "An `building:ClassOfLocationState` that acts as a classifier for types of AccessPointState, e.g., open, closed, restricted, or temporarily diverted access points." ;
    rdfs:subClassOf building:ClassOfBuiltEntityState .

# Classifier for access mode (parallel to AccessPointByLevel)
building:AccessPointByAccessMode a rdfs:Class ;
    rdfs:label "Access Point by Access Mode" ;
    rdfs:comment "A `building:ClassOfAccessPoint` that classifies `building:AccessPoint` by the mode(s) permitted at the access point (pedestrian, vehicular, or both), aligned to OS NGD accessmodevalue." ;
    rdfs:subClassOf building:ClassOfAccessPoint .

# Instances of the classifier (and subclasses of AccessPoint) per OS code list

building:AccessPedestrianOnly a building:AccessPointByAccessMode ;
    rdfs:label "Access Pedestrian Only" ;
    rdfs:comment "An instance of `building:AccessPointByAccessMode` corresponding to OS NGD `accessmodevalue` 'Pedestrian' — an entrance/exit location for pedestrians only." ;
    rdfs:subClassOf building:AccessPoint .

building:AccessVehicularOnly a building:AccessPointByAccessMode ;
    rdfs:label "Access Vehicular Only" ;
    rdfs:comment "An instance of `building:AccessPointByAccessMode` corresponding to OS NGD `accessmodevalue` 'Vehicular' — an entrance/exit location for vehicles only." ;
    rdfs:subClassOf building:AccessPoint .

building:AccessPedestrianAndVehicular a building:AccessPointByAccessMode ;
    rdfs:label "Access Pedestrian And Vehicular" ;
    rdfs:comment "An instance of `building:AccessPointByAccessMode` corresponding to OS NGD `accessmodevalue` 'Pedestrian And Vehicular' — an entrance/exit location for both pedestrians and vehicles." ;
    rdfs:subClassOf building:AccessPoint .

# Classifier for access purpose (parallel to AccessPointByLevel)
building:AccessPointByAccessPurpose a rdfs:Class ;
    rdfs:label "Access Point by Access Purpose" ;
    rdfs:comment "A `building:ClassOfAccessPoint` that classifies `building:AccessPoint` by the principal function of the access location (Emergency, Primary Public, Private, or Public), aligned to OS NGD `accesspurposevalue`." ;
    rdfs:subClassOf building:ClassOfAccessPoint .

# Instances of the classifier (and subclasses of AccessPoint) per OS code list

building:EmergencyAccess a building:AccessPointByAccessPurpose ;
    rdfs:label "Emergency Access" ;
    rdfs:comment "An instance of `building:AccessPointByAccessPurpose` corresponding to OS NGD `accesspurposevalue` 'Emergency' — an entrance/exit location that is solely intended for use in emergencies." ;
    rdfs:subClassOf building:AccessPoint .

building:PrimaryPublicAccess a building:AccessPointByAccessPurpose ;
    rdfs:label "Primary Public Access" ;
    rdfs:comment "An instance of `building:AccessPointByAccessPurpose` corresponding to OS NGD `accesspurposevalue` 'Primary Public' — a principal entrance/exit location that is intended for public use, usually referred to as the ‘Main Entrance’. A given Site/Building may have more than one primary public access location, especially for larger features." ;
    rdfs:subClassOf building:AccessPoint .

building:PrivateAccess a building:AccessPointByAccessPurpose ;
    rdfs:label "Private Access" ;
    rdfs:comment "An instance of `building:AccessPointByAccessPurpose` corresponding to OS NGD `accesspurposevalue` 'Private' — an entrance/exit location that is not intended for public use." ;
    rdfs:subClassOf building:AccessPoint .

building:PublicAccess a building:AccessPointByAccessPurpose ;
    rdfs:label "Public Access" ;
    rdfs:comment "An instance of `building:AccessPointByAccessPurpose` corresponding to OS NGD `accesspurposevalue` 'Public' — an entrance/exit location that is intended for public use." ;
    rdfs:subClassOf building:AccessPoint .

# Classifier for accessibility (parallel to AccessPointByAccessPurpose)
building:AccessPointByAccessibility a rdfs:Class ;
    rdfs:label "Access Point by Accessibility" ;
    rdfs:comment "A `building:ClassOfAccessPoint` that classifies `building:AccessPoint` by its accessibility state or impact on mobility (Facilitated, Unconstrained, or Constrained)." ;
    rdfs:subClassOf building:ClassOfAccessPoint .

# Instances of the classifier (and subclasses of AccessPoint)

building:FacilitatedAccessPoint a building:AccessPointByAccessibility ;
    rdfs:label "Facilitated Access" ;
    rdfs:comment "An instance of `building:AccessPointByAccessibility` — an access point whose features facilitate mobility for many users (e.g., ramp with appropriate slope, automatic door)." ;
    rdfs:subClassOf building:AccessPoint .

building:UnconstrainedAccessPoint a building:AccessPointByAccessibility ;
    rdfs:label "Unconstrained Access" ;
    rdfs:comment "An instance of `building:AccessPointByAccessibility` — an access point with no notable features expected to significantly constrain or facilitate mobility for most users." ;
    rdfs:subClassOf building:AccessPoint .

building:ConstrainedAccessPoint a building:AccessPointByAccessibility ;
    rdfs:label "Constrained Access" ;
    rdfs:comment "An instance of `building:AccessPointByAccessibility` — an access point whose features are likely to constrain mobility for some users (e.g., step, narrow doorway, steep gradient)." ;
    rdfs:subClassOf building:AccessPoint .

building:accessibilityImpactedBy a owl:ObjectProperty;
    rdfs:label "accessibility impacted by" ;
    rdfs:comment "A relationship that obtains between an instance of `building:AccessPoint` and `building:BuiltEntity` whose existence influences the accessibility of that `building:AccessPoint` (positively or negatively)." ;
    rdfs:domain building:AccessPointState ;
    rdfs:range building:BuiltEntityState .

########################  add ramp and step classes #####################

### Ramp

building:Ramp a rdfs:Class ;
    rdfs:label "Ramp" ;
    ies:powertype building:ClassOfRamp ;
    rdfs:comment "A `building:BuiltEntity` that provides an inclined surface for pedestrian or vehicular movement between different elevations, facilitating accessibility or transport." ;
    rdfs:seeAlso <https://search.bsdd.buildingsmart.org/uri/buildingsmart/ifc/4.3/class/IfcRamp> ;
    rdfs:subClassOf building:RampState,
        building:BuiltEntity .

building:RampState a rdfs:Class ;
    rdfs:label "Ramp State" ;
    rdfs:comment "A temporal state of a `building:Ramp` during its lifecycle." ;
    rdfs:subClassOf building:BuiltEntityState .

building:ClassOfRamp a rdfs:Class ;
    rdfs:label "Class of Ramp" ;
    rdfs:comment "A class that represents a category of `building:Ramp` based on shared characteristics." ;
    rdfs:subClassOf building:ClassOfBuiltEntity .


### Step

building:Step a rdfs:Class ;
    rdfs:label "Step" ;
    ies:powertype building:ClassOfStep ;
    rdfs:comment "A `building:BuiltEntity` that forms part of a stair or other structure, intended for ascending or descending between different elevations." ;
    rdfs:seeAlso <https://search.bsdd.buildingsmart.org/uri/buildingsmart/ifc/4.3/class/IfcStairFlight> ;
    rdfs:subClassOf building:StepState,
        building:BuiltEntity .

building:StepState a rdfs:Class ;
    rdfs:label "Step State" ;
    rdfs:comment "A temporal state of a `building:Step` during its lifecycle." ;
    rdfs:subClassOf building:BuiltEntityState .

building:ClassOfStep a rdfs:Class ;
    rdfs:label "Class of Step" ;
    rdfs:comment "A class that represents a category of `building:Step` based on shared characteristics." ;
    rdfs:subClassOf building:ClassOfBuiltEntity .

### Staircase

# Class of StairCase for the powertype pattern
building:ClassOfStairCase a rdfs:Class ;
    rdfs:label "Class of Staircase" ;
    rdfs:comment "A classifier for instances of `building:StairCase`, used to group staircases with shared characteristics (e.g., straight flight, spiral, with landings)." ;
    rdfs:subClassOf building:ClassOfBuiltEntity .

# State class for StairCase (optional, parallels StepState)
building:StairCaseState a rdfs:Class ;
    rdfs:label "Staircase State" ;
    rdfs:comment "A classification of `building:StairCase` by its condition, accessibility, or other state-related attribute." ;
    rdfs:subClassOf building:BuiltEntityState .

# StairCase definition
building:StairCase a rdfs:Class ;
    rdfs:label "Staircase" ;
    ies:powertype building:ClassOfStairCase ;
    rdfs:comment "A `building:BuiltEntity` consisting of a flight or series of flights of steps, with or without landings, designed to allow passage between different elevations within or between structures." ;
    rdfs:seeAlso <https://search.bsdd.buildingsmart.org/uri/buildingsmart/ifc/4.3/class/IfcStair> ;
    rdfs:subClassOf building:StairCaseState ,
                    building:BuiltEntity .

### Barrier
building:Barrier a rdfs:Class ;
    rdfs:label "Barrier" ;
    ies:powertype building:ClassOfBarrier ;
    rdfs:comment "A `building:BuiltEntity` that obstructs, directs, or controls movement of people, vehicles, or animals." ;
    rdfs:subClassOf building:BarrierState,
        building:BuiltEntity .

building:BarrierState a rdfs:Class ;
    rdfs:label "Barrier State" ;
    rdfs:comment "A temporal state of a `building:Barrier` during its lifecycle." ;
    rdfs:subClassOf building:BuiltEntityState .

building:ClassOfBarrier a rdfs:Class ;
    rdfs:label "Class of Barrier" ;
    rdfs:comment "A class that represents a category of `building:Barrier` based on shared characteristics." ;
    rdfs:subClassOf building:ClassOfBuiltEntity .


### Turnstile
building:Turnstile a rdfs:Class ;
    rdfs:label "Turnstile" ;
    ies:powertype building:ClassOfTurnstile ;
    rdfs:comment "A `building:BuiltEntity` that permits controlled, usually one-way, passage of individuals, typically for access control or fare collection." ;
    rdfs:subClassOf building:TurnstileState,
        building:BuiltEntity .

building:TurnstileState a rdfs:Class ;
    rdfs:label "Turnstile State" ;
    rdfs:comment "A temporal state of a `building:Turnstile` during its lifecycle." ;
    rdfs:subClassOf building:BuiltEntityState .

building:ClassOfTurnstile a rdfs:Class ;
    rdfs:label "Class of Turnstile" ;
    rdfs:comment "A class that represents a category of `building:Turnstile` based on shared characteristics." ;
    rdfs:subClassOf building:ClassOfBuiltEntity .

### Elevator
building:Elevator a rdfs:Class ;
    rdfs:label "Elevator" ;
    ies:powertype building:ClassOfElevator ;
    rdfs:comment "A `building:BuiltEntity` that vertically transports people or goods between different levels within a structure." ;
    rdfs:subClassOf building:ElevatorState,
        building:BuiltEntity .

building:ElevatorState a rdfs:Class ;
    rdfs:label "Elevator State" ;
    rdfs:comment "A temporal state of a `building:Elevator` during its lifecycle." ;
    rdfs:subClassOf building:BuiltEntityState .

building:ClassOfElevator a rdfs:Class ;
    rdfs:label "Class of Elevator" ;
    rdfs:comment "A class that represents a category of `building:Elevator` based on shared characteristics." ;
    rdfs:subClassOf building:ClassOfBuiltEntity .


### Gate
building:Gate a rdfs:Class ;
    rdfs:label "Gate" ;
    ies:powertype building:ClassOfGate ;
    rdfs:comment "A `building:BuiltEntity` that provides a hinged, sliding, or otherwise movable closure to control passage through an opening in a fence, wall, or similar boundary." ;
    rdfs:subClassOf building:GateState,
        building:BuiltEntity .

building:GateState a rdfs:Class ;
    rdfs:label "Gate State" ;
    rdfs:comment "A temporal state of a `building:Gate` during its lifecycle." ;
    rdfs:subClassOf building:BuiltEntityState .

building:ClassOfGate a rdfs:Class ;
    rdfs:label "Class of Gate" ;
    rdfs:comment "A class that represents a category of `building:Gate` based on shared characteristics." ;
    rdfs:subClassOf building:ClassOfBuiltEntity .

#####################  Obstructed Access Point An Event ########################
building:ObstructionEvent a rdfs:Class ;
    rdfs:label "Access Point Obstruction" ;
    rdfs:comment "An `ies:Event` during which some entity's normal access/function is impeded by another, potentially affecting further entities." ;
    rdfs:subClassOf ies:Event .


###########  Basement ####################

building:Basement a rdfs:Class ;
    rdfs:label "Basement"@en ;
    rdfs:comment "A `building:Storey` that is wholly or partly below the ground level of a `building:Structure`, typically used for storage, parking, or mechanical equipment."@en ;
    rdfs:subClassOf building:BasementState,
        building:Storey .

building:BasementState a rdfs:Class ;
    rdfs:label "Basement State"@en ;
    ies:powertype building:ClassOfBasementState ;
    rdfs:comment "An `ies:State` that is the temporal State of a Basement."@en ;
    rdfs:subClassOf building:StoreyState .

#########  Prepare for built environment ######################

building:ClassOfSite a rdfs:Class ;
  rdfs:label "Class of Site" ;
  rdfs:comment "An `building:ClassOfLocation` that classifies `building:Site`" ;
  rdfs:subClassOf building:ClassOfLocation .

building:Site a rdfs:Class ;
  rdfs:label "Site" ;
  ies:powertype building:ClassOfSite ;
  rdfs:comment "An `ies:Location`that is the total extent of a defined property, parcel, or facility." ;
  rdfs:subClassOf ies:Location, building:SiteState .

building:SiteState a rdfs:Class ;
  rdfs:label "Site State" ;
  ies:powertype building:ClassOfSiteState ;
  rdfs:comment "A temporal state of a Site (e.g., as‑built extent, post‑expansion extent, remediation phase)." ;
  rdfs:subClassOf ies:LocationState .

building:ClassOfSiteState a rdfs:Class ;
  rdfs:label "Class of Site State" ;
  rdfs:comment "An `building:ClassOfLocationState` that classifies `building:SiteState`" ;
  rdfs:subClassOf building:ClassOfLocationState .


###################  Minimal CRS ###########################
building:CoordinateReferenceSystem a rdfs:Class ;
    rdfs:subClassOf ies:Thing ;
    rdfs:label "Coordinate Reference System" ;
    rdfs:comment "A defined coordinate system with an associated reference frame for interpreting coordinates, e.g., EPSG:27700." .

building:epsg_27700 a building:CoordinateReferenceSystem ;
    rdfs:label "EPSG 27700" ;
    rdfs:comment "The equivalent of epsg:27700; which is known as OSGB 1936 / British National Grid" .

building:epsg_4326 a building:CoordinateReferenceSystem ;
    rdfs:label "EPSG 4326" ;
    rdfs:comment "The equivalent of epsg:4326; which is known as WGS 84" .

building:hasCoordinateReference a owl:ObjectProperty ;
    rdfs:label "has Coordinate Reference Of" ;
    rdfs:comment "A relationship that indicates how the given `ies:GeoRepresentation` should be interpreted" ;
    rdfs:domain ies:GeoRepresentation ;
    rdfs:range building:CoordinateReferenceSystem .

############## Built Environment Classifiers ######################

##############   Relationship to Surface Level ##############

building:LevelRelativeToSurface a rdfs:Class ;
    rdfs:label "Level Relative to Surface" ;
    rdfs:comment "An `ies:Characteristic` that indicates the level the element relative to the natural surface level, such as above, below, or at surface level." ;
    rdfs:subClassOf ies:Characteristic, building:ClassOfLocation .

building:AboveSurfaceLevel a building:LevelRelativeToSurface ;
    rdfs:label "Access Above Surface Level" ;
    rdfs:comment "An instance of `building:LevelRelativeToSurface` that is situated above the natural surface level, such as an elevated walkway, footbridge, or raised platform access point." ;
    rdfs:subClassOf ies:Location .

building:BelowSurfaceLevel a building:LevelRelativeToSurface ;
    rdfs:label "Access Below Surface Level" ;
    rdfs:comment "An instance of `building:LevelRelativeToSurface` that is situated below the natural surface level, such as a basement entrance, underground tunnel, or subway station access point." ;
    rdfs:subClassOf ies:Location .

building:AtSurfaceLevel a building:LevelRelativeToSurface ;
    rdfs:label "Access at Surface Level" ;
    rdfs:comment "An instance of `building:LevelRelativeToSurface` that is situated at the natural surface level, such as a standard building entrance or ground-level doorway." ;
    rdfs:subClassOf ies:Location .

###########################  Locations describing building lines ####################

########################## Physical State of Structures ##########################

### Powertype (metaclass) for physical state
building:ClassOfPhysicalState a owl:Class ;
  rdfs:subClassOf building:ClassOfBuildingState ;
  rdfs:label "Class Of Physical State" ;
  rdfs:comment "Powertype for classifying building states according to OS NGD Physical State values (Built, Derelict, Under Construction)." .

### Facet values (punned classes and instances of the powertype)
building:BuiltState a building:ClassOfPhysicalState ;
  rdfs:subClassOf building:BuildingState ;
  rdfs:label "Built" ;
  rdfs:comment "The building is fully constructed and usable (OS NGD Physical State: Built)." .

building:DerelictState a building:ClassOfPhysicalState ;
  rdfs:subClassOf building:BuildingState ;
  rdfs:label "Derelict" ;
  rdfs:comment "The building is in a derelict condition, in decay but retains roof or walls (OS NGD Physical State: Derelict)." .

building:UnderConstructionState a building:ClassOfPhysicalState ;
  rdfs:subClassOf building:BuildingState ;
  rdfs:label "Under Construction" ;
  rdfs:comment "The building is being constructed (OS NGD Physical State: Under Construction)." .

############### Roof Shape Classifiers ##################

### Powertype (metaclass) for roof section shape
building:RoofShape a owl:Class ;
  rdfs:subClassOf building:ClassOfRoofState ;
  rdfs:label "Roof Section Shape" ;
  rdfs:comment "Powertype for classifying roof section shape according to OS NGD Roof Shape values (Flat, Pitched, Mixed, Unknown)." .

### Facet values (punned classes and instances of the powertype)

# Flat (pitch <= 15°)
building:FlatRoofShape a building:RoofShape ;
  rdfs:subClassOf building:RoofState ;
  rdfs:label "Flat" ;
  rdfs:comment "The section is predominantly comprised of faces with a pitch value of ≤ 15° (OS NGD Roof Shape: Flat)." .

# Pitched (> 15°)
building:PitchedRoofShape a building:RoofShape ;
  rdfs:subClassOf building:RoofState ;
  rdfs:label "Pitched" ;
  rdfs:comment "The section is predominantly comprised of faces with a pitch value of > 15° (OS NGD Roof Shape: Pitched)." .

# Mixed (near-equal areas of flat and pitched faces and/or differing aspects)
building:MixedRoofShape a building:RoofShape ;
  rdfs:subClassOf building:RoofState ;
  rdfs:label "Mixed" ;
  rdfs:comment "The section is comprised of multiple faces with different pitch and aspect values; there is no one predominant shape due to near-equal areas of flat (≤ 15°) and pitched (> 15°) faces (OS NGD Roof Shape: Mixed)." .

# Unknown
building:UnknownRoofShape a building:RoofShape ;
  rdfs:subClassOf building:RoofState ;
  rdfs:label "Unknown" ;
  rdfs:comment "The shape could not be determined (e.g., obscured imagery or roof furniture); also used when the section was captured after imagery/height data and shape has not yet been derived (OS NGD Roof Shape: Unknown)." .

###########  Classified By Status #########################

building:StatesClassifiedByStatus a rdfs:Class ;
  rdfs:label "Classified by Status" ;
  rdfs:comment "A class that represents a category of `building:ClassifiableByStatus` based on shared characteristics." ;
  rdfs:subClassOf ies:State .
building:ClassOfStatesClassifiedByBuiltStatus a rdfs:Class ;
  rdfs:label "Class Of Classifiable by Status" ;
  rdfs:comment "A `ies:ClassOfState` whose states can be classified by status." ;
  rdfs:subClassOf ies:ClassOfState .

# Built Complete
building:BuiltComplete
  a building:ClassOfStatesClassifiedByBuiltStatus, rdfs:Class ;
  rdfs:label "Built Complete" ;
  rdfs:comment "A ClassOfStatesClassifiedByStatus that is a state in which a real-world object is physically complete and usable for the purpose by which it is classified, including completed buildings, land suitable for occupation, and structures such as advertising hoardings." ;
  rdfs:subClassOf building:StatesClassifiedByStatus .

building:Occupied
  a building:ClassOfStatesClassifiedByBuiltStatus, rdfs:Class ;
    rdfs:label "Occupied"@en-gb ;
    rdfs:comment "A ClassOfStatesClassifiedByStatus that is a state in which a `building:Structure`, `building:StructureUnit`, or `building:Space` is routinely occupied by one or more people." ;
    rdfs:subClassOf building:StatesClassifiedByStatus   .

# Built Unoccupied
building:BuiltUnoccupied
  a building:ClassOfStatesClassifiedByBuiltStatus, rdfs:Class ;
  rdfs:label "Built Unoccupied" ;
  rdfs:comment "A ClassOfStatesClassifiedByStatus that is a state in which a real-world object is not usable or not fit for the purpose by which it is classified, including buildings not suitable for occupation." ;
  rdfs:subClassOf building:StatesClassifiedByStatus .

# Historic
building:Historic
  a building:ClassOfStatesClassifiedByBuiltStatus, rdfs:Class ;
  rdfs:label "Historic" ;
  rdfs:comment "A ClassOfStatesClassifiedByStatus that is a state in which a real-world object no longer exists, including buildings demolished or subdivided, removed objects, or superseded addresses such as development sites." ;
  rdfs:subClassOf building:StatesClassifiedByStatus .

# Prebuild
building:Prebuild
  a building:ClassOfStatesClassifiedByBuiltStatus, rdfs:Class ;
  rdfs:label "Prebuild" ;
  rdfs:comment "A ClassOfStatesClassifiedByStatus that is a state in which a real-world object is under construction, reconstruction, or redevelopment." ;
  rdfs:subClassOf building:StatesClassifiedByStatus .

# Make the three states classifiable by use
building:SiteState rdfs:subClassOf building:StatesClassifiedByStatus .
building:StructureState rdfs:subClassOf building:StatesClassifiedByStatus .
building:StructureUnitState rdfs:subClassOf building:StatesClassifiedByStatus .


############### Use Classifiers ######################

### A combined class for use types

### “ClassifiedByUse” umbrella

building:StatesClassifiedByUse a rdfs:Class ;
  rdfs:label "Classified by Use" ;
  rdfs:comment "A class that represents a category of `building:ClassifiableByUse` based on shared characteristics." ;
  rdfs:subClassOf ies:State .
building:ClassOfStatesClassifiedByUse a rdfs:Class ;
  rdfs:label "Class Of Classifiable by Use" ;
  rdfs:comment "A `ies:ClassOfState` whose states can be classified by use." ;
  rdfs:subClassOf ies:ClassOfState .

# Make the three states classifiable by use
building:SiteState rdfs:subClassOf building:StatesClassifiedByUse .
building:StructureState rdfs:subClassOf building:StatesClassifiedByUse .
building:StructureUnitState rdfs:subClassOf building:StatesClassifiedByUse .

############# Commercial Use Classifiers ##############

building:CommercialUse a rdfs:Class ;
    rdfs:label "Commercial Use" ;
    rdfs:comment "A `building:ClassifiableByUse` that represents states primarily used for commercial activities, such as retail, offices, or services." ;
    rdfs:subClassOf building:StatesClassifiedByUse .

building:ClassOfCommercialUse a rdfs:Class ;
    rdfs:label "Commercial Use" ;
    rdfs:comment "A `building:ClassifiableByUse` that are classes of states primarily used for commercial activities, such as retail, offices, or services." ;
    rdfs:subClassOf building:ClassOfStatesClassifiedByUse .

building:CommercialRetailUse a rdfs:Class , building:ClassOfCommercialUse ;
  rdfs:label   "Commercial: Retail" ;
  rdfs:comment "Retail sale or serving of finished goods to the public." ;
  rdfs:subClassOf building:CommercialUse .

building:CommercialIndustrialOrManufacturingUse a rdfs:Class , building:ClassOfCommercialUse ;
  rdfs:label   "Commercial: Industrial or Manufacturing" ;
  rdfs:comment "Manufacture, processing, or extraction-based commercial activity." ;
  rdfs:subClassOf building:CommercialUse .

building:CommercialDistributionOrStorageUse a rdfs:Class , building:ClassOfCommercialUse ;
  rdfs:label   "Commercial: Distribution or Storage" ;
  rdfs:comment "Warehousing, logistics, storage, or sorting of goods/materials." ;
  rdfs:subClassOf building:CommercialUse .

building:CommercialAnimalServicesUse a rdfs:Class , building:ClassOfCommercialUse ;
  rdfs:label   "Commercial: Animal Services" ;
  rdfs:comment "Animal care, accommodation, breeding, or burial/cremation services operated commercially." ;
  rdfs:subClassOf building:CommercialUse .

building:CommercialOtherUse a rdfs:Class , building:ClassOfCommercialUse ;
  rdfs:label   "Commercial: Other" ;
  rdfs:comment "Commercial activity not covered by retail, industrial/manufacturing, distribution/storage, or animal services." ;
  rdfs:subClassOf building:CommercialUse .

########################## Building Connectivity of Structures ##########################

### Powertype (metaclass) for building state
building:BuildingConnectivity a owl:Class ;
  rdfs:subClassOf building:ClassOfBuildingState ;
  rdfs:label "Building Connectivity" ;
  rdfs:comment "Powertype for classifying building states according to OS NGD Building Connectivity values (End-Connected, Multi-Connected, Semi-Connected, Standalone)." .

### Facet values (punned classes and instances of the powertype)
building:EndConnected a building:BuildingConnectivity ;
  rdfs:subClassOf building:BuildingState ;
  rdfs:label "End-Connected" ;
  rdfs:comment "A building which is connected to one other building at the end of a connected block of buildings (e.g., terrace) (OS NGD Building Connectivity: End-Connected)." .

building:MultiConnected a building:BuildingConnectivity ;
  rdfs:subClassOf building:BuildingState ;
  rdfs:label "Multi-Connected" ;
  rdfs:comment "A building which is connected to more than one other building (OS NGD Building Connectivity: Multi-Connected)." .

building:SemiConnected a building:BuildingConnectivity ;
  rdfs:subClassOf building:BuildingState ;
  rdfs:label "Semi-Connected" ;
  rdfs:comment "A building which is connected to one other building but not at the end of a connected block of buildings (OS NGD Building Connectivity: Semi-Connected)." .

building:Standalone a building:BuildingConnectivity ;
  rdfs:subClassOf building:BuildingState ;
  rdfs:label "Standalone" ;
  rdfs:comment "A building which is not connected to another building (OS NGD Building Connectivity: Standalone)." .

##############  Community Use Classifiers ##############

building:CommunityUse a rdfs:Class ;
    rdfs:label "Community Use" ;
    rdfs:comment "A `building:ClassifiableByUse` that represents states primarily used for Community activities, such as retail, offices, or services." ;
    rdfs:subClassOf building:StatesClassifiedByUse .

building:ClassOfCommunityUse a rdfs:Class ;
    rdfs:label "Community Use" ;
    rdfs:comment "A `building:ClassifiableByUse` that are classes of states primarily used for Community activities, such as retail, offices, or services." ;
    rdfs:subClassOf building:ClassOfStatesClassifiedByUse .

building:CommunityEmergencyServicesUse a rdfs:Class , building:ClassOfCommunityUse ;
  rdfs:label   "Community: Emergency Services" ;
  rdfs:comment "Emergency services such as police, fire, ambulance, and rescue operations." ;
  rdfs:subClassOf building:CommunityUse .

building:CommunityFuneralServicesUse a rdfs:Class , building:ClassOfCommunityUse ;
  rdfs:label   "Community: Funeral Services" ;
  rdfs:comment "Funeral services, including mortuaries, crematoria, and burial grounds." ;
  rdfs:subClassOf building:CommunityUse .

building:CommunityReligiousUse a rdfs:Class , building:ClassOfCommunityUse ;
  rdfs:label   "Community: Religious Use" ;
  rdfs:comment "Places of worship, religious gatherings, and associated community services." ;
  rdfs:subClassOf building:CommunityUse .

building:CommunityOtherUse a rdfs:Class , building:ClassOfCommunityUse ;
  rdfs:label   "Community: Other" ;
  rdfs:comment "Community activities not covered by emergency services, funeral services, or religious use." ;
  rdfs:subClassOf building:CommunityUse .

############## Transport Use Classifiers ##############

building:TransportUse a rdfs:Class ;
    rdfs:label "Transport Use" ;
    rdfs:comment "A `building:ClassifiableByUse` that represents states primarily used for transport activities, such as airports, bus stations, or railways." ;
    rdfs:subClassOf building:StatesClassifiedByUse .

building:ClassOfTransportUse a rdfs:Class ;
    rdfs:label "Class Of Transport Use" ;
    rdfs:comment "A `building:ClassifiableByUse` that are classes of states primarily used for transport activities, such as airports, bus stations, or railways." ;
    rdfs:subClassOf building:ClassOfStatesClassifiedByUse .

building:AirTransportUse a rdfs:Class , building:ClassOfTransportUse ;
  rdfs:label   "Air Transport Use" ;
  rdfs:comment "Airports, heliports, and other facilities primarily used for air transport, excluding those that are for Defence purposes.." ;
  rdfs:subClassOf building:TransportUse .

building:RailTransportUse a rdfs:Class , building:ClassOfTransportUse ;
  rdfs:label   "Rail Transport Use" ;
  rdfs:comment "Railway stations, depots, and other facilities primarily used for rail transport." ;
  rdfs:subClassOf building:TransportUse .

building:RoadTrackOrPathTransportUse a rdfs:Class , building:ClassOfTransportUse ;
  rdfs:label   "Road, Track or Path Transport Use" ;
  rdfs:comment "Roads, tracks, paths, and other facilities support the movement of people and freight using roads, tracks and paths. Includes movement via motorised (for example, cars, buses) and non-motorised vehicles (for example, bicycles), on horseback and on foot." ;
  rdfs:subClassOf building:TransportUse .

building:WaterTransportUse a rdfs:Class , building:ClassOfTransportUse ;
  rdfs:label   "Water Transport Use" ;
  rdfs:comment "Ports, harbours, and other facilities primarily used for water transport, including marinas and docks." ;
  rdfs:subClassOf building:TransportUse .

##############  Residential Use Classifiers ##############

building:ResidentialUse a rdfs:Class, building:ClassOfStatesClassifiedByUse ;
    rdfs:label "Residential Use" ;
    rdfs:comment "A `building:ClassifiableByUse` that represents states primarily used for commercial activities, such as retail, offices, or services." ;
    rdfs:subClassOf building:StatesClassifiedByUse .

building:ClassOfResidentialUse a rdfs:Class ;
    rdfs:label "Residential Use" ;
    rdfs:comment "A `building:ClassifiableByUse` that are classes of states primarily used for commercial activities, such as retail, offices, or services." ;
    skos:note "Not in active use as there is only the category of Residential Use, but may be used in future to classify residential states by type of residential use." ;
    rdfs:subClassOf building:ClassOfStatesClassifiedByUse .

########## Singleton Classifiers ##########

building:GovernmentOrPublicAdministrationUse a rdfs:Class , building:ClassOfStatesClassifiedByUse ;
  rdfs:label   "Government Or Public Administration Use" ;
  rdfs:comment "Government services and administration provided or managed by central or local government." ;
  rdfs:subClassOf building:StatesClassifiedByUse .

building:MedicalOrHealthUse a rdfs:Class , building:ClassOfStatesClassifiedByUse ;
  rdfs:label   "Medical Or Health Use" ;
  rdfs:comment "Medical or health-care activities, including primary/secondary care and related health services." ;
  rdfs:subClassOf building:StatesClassifiedByUse .

building:MixedUse a rdfs:Class , building:ClassOfStatesClassifiedByUse ;
  rdfs:label   "Mixed Use" ;
  rdfs:comment "More than two defined uses." ;
  rdfs:subClassOf building:StatesClassifiedByUse .

building:EducationUse a rdfs:Class , building:ClassOfStatesClassifiedByUse ;
  rdfs:label   "Education Use" ;
  rdfs:comment "Academic or vocational teaching and learning activities and supporting premises." ;
  rdfs:subClassOf building:StatesClassifiedByUse .

building:HospitalityAndTemporaryStayUse a rdfs:Class , building:ClassOfStatesClassifiedByUse ;
  rdfs:label   "Hospitality & Temporary Stay Use" ;
  rdfs:comment "Temporary or holiday accommodation and similar short-stay premises (e.g., hotels, hostels, shelters)." ;
  rdfs:subClassOf building:StatesClassifiedByUse .

building:UtilitiesAndEnvironmentalProtectionUse a rdfs:Class , building:ClassOfStatesClassifiedByUse ;
  rdfs:label   "Utilities & Environmental Protection Use" ;
  rdfs:comment "Provision of essential services (power, water, waste, telecoms) and environmental monitoring/control." ;
  rdfs:subClassOf building:StatesClassifiedByUse .

building:DefenceUse a rdfs:Class , building:ClassOfStatesClassifiedByUse ;
  rdfs:label   "Defence Use" ;
  rdfs:comment "Military and defence-related activities and premises." ;
  rdfs:subClassOf building:StatesClassifiedByUse .

building:AgricultureAndAquacultureUse a rdfs:Class , building:ClassOfStatesClassifiedByUse ;
  rdfs:label   "Agriculture & Aquaculture Use" ;
  rdfs:comment "Agriculture, animal husbandry, and aquaculture activities and associated premises." ;
  rdfs:subClassOf building:StatesClassifiedByUse .

building:ConstructionTransitionalUse a rdfs:Class , building:ClassOfStatesClassifiedByUse ;
  rdfs:label   "Construction (Transitional) Use" ;
  rdfs:comment "On-going construction where the final end-use is not yet established (transitional site/structure state)." ;
  rdfs:subClassOf building:StatesClassifiedByUse .

building:AttractionOrActivity a rdfs:Class , building:ClassOfStatesClassifiedByUse ;
  rdfs:label   "Attraction Or Activity" ;
  rdfs:comment "Non-sporting leisure activities and related services for the public." ;
  rdfs:subClassOf building:StatesClassifiedByUse .

building:ConstructionUse a rdfs:Class , building:ClassOfStatesClassifiedByUse ;
  rdfs:label   "Construction Use" ;
  rdfs:comment "A `building:ClassifiableByUse` that represents states primarily used for construction activities." ;
  rdfs:subClassOf building:StatesClassifiedByUse .

building:HistoricOrHeritageUse a rdfs:Class , building:ClassOfStatesClassifiedByUse ;
  rdfs:label   "Historic Or Heritage Use" ;
  rdfs:comment "A `building:ClassifiableByUse` that represents states primarily used for historic or heritage activities." ;
  rdfs:subClassOf building:StatesClassifiedByUse .

building:SportsAndRecreationUse a rdfs:Class , building:ClassOfStatesClassifiedByUse ;
  rdfs:label   "Sports And Recreation Use" ;
  rdfs:comment "A `building:ClassifiableByUse` that represents states primarily used for sports and recreation activities." ;
  rdfs:subClassOf building:StatesClassifiedByUse .

building:UnknownNaturalUse a rdfs:Class , building:ClassOfStatesClassifiedByUse ;
  rdfs:label   "Unknown Natural Use" ;
  rdfs:comment "A `building:ClassifiableByUse` that represents states of natural entities whose purpose is unknown." ;
  rdfs:subClassOf building:StatesClassifiedByUse .

building:UnknownArtificialUse a rdfs:Class , building:ClassOfStatesClassifiedByUse ;
  rdfs:label   "Unknown Artificial Use" ;
  rdfs:comment "A `building:ClassifiableByUse` that represents states of artificial entities whose purpose is unknown." ;
  rdfs:subClassOf building:StatesClassifiedByUse .

#################  Entities that can be built from building:Material ###########
building:ClassOfStuffPortion a rdfs:Class ;
    rdfs:subClassOf ies:ClassOfEntity .

building:isSumOf a owl:ObjectProperty ;
    rdfs:label "is sum of" ;
    rdfs:comment "A relationship that asserts that an instance of ies:Element is the mereological sum - that is, the totality formed by combining - the members of a building:ClassOfElement" ;
    rdfs:domain ies:Element ;
    rdfs:range ies:ClassOfElement .

building:madeOf a owl:ObjectProperty ;
    rdfs:label "made of" ;
    rdfs:comment "A relationship that asserts that an instance of `building:Entity` is made (constructed) from a member of `ClassOfEntity` " ;
    rdfs:domain ies:Entity ;
    rdfs:range ies:ClassOfEntity .

building:BuildingMaterial a rdfs:Class, ies:ClassOfEntity ;
    rdfs:label "Building Material" ;
    rdfs:comment "An entity whose instances are commonly used in the construction of features of the built environment" ;
    skos:example "ConcretePortion", "Brick" ;
    rdfs:subClassOf ies:Entity .

building:eachMemberIsMadeOf a owl:ObjectProperty ;
    rdfs:label "each member is made of" ;
    rdfs:comment "A relationship that asserts that each member of an instance of `ies:ClassOfEntity` e, is made from some member(s) of `ClassOfEntity` m " ;
    rdfs:domain ies:ClassOfEntity ;
    rdfs:range ies:ClassOfEntity .

###################  The balance of the distinct building construction materials from the OSNGD data model ######################

# Countable units (unchanged pattern; broadened comments)
building:Brick a rdfs:Class, ies:ClassOfEntity ;
    rdfs:label "Brick" ;
    rdfs:comment "An `ies:Entity` that is a fired-clay (or similar) masonry unit used in walls and other constructions." ;
    rdfs:subClassOf ies:Entity .

building:Block a rdfs:Class, ies:ClassOfEntity ;
    rdfs:label "Block" ;
    rdfs:comment "An `ies:Entity` that is a masonry unit (e.g., concrete or lightweight aggregate block) used to form constructions." ;
    rdfs:subClassOf ies:Entity .

# Stuff materials (unchanged pattern; broadened comments)
### Concrete
building:concrete a ies:Stuff ;
    rdfs:label "concrete" ;
    building:isSumOf building:ConcretePortion ;
    rdfs:comment "An instance of `ies:Stuff` composed of aggregate bound with cement and water, used for structural or non-structural components." .

building:ConcretePortion a rdfs:Class, building:ClassOfStuffPortion ;
    rdfs:label "Concrete Portion" ;
    rdfs:comment "An `ies:Entity` that is a portion of `building:concrete`." ;
    rdfs:subClassOf building:StuffPortion       , building:BuildingMaterial .  ##  what does this mean

### Stone
building:stone a ies:Stuff ;
    rdfs:label "stone" ;
    building:isSumOf building:StonePortion ;
    rdfs:comment "An instance of `ies:Stuff` consisting of natural rock used as a construction material (e.g., rubble, ashlar, cladding)." .

building:StonePortion a rdfs:Class, building:ClassOfStuffPortion ;
    rdfs:label "Stone Portion" ;
    rdfs:comment "An `ies:Entity` that is a portion of `building:stone`." ;
    rdfs:subClassOf building:StuffPortion .

### Wood / Timber
building:wood a ies:Stuff ;
    rdfs:label "wood" ;
    building:isSumOf building:WoodPortion ;
    rdfs:comment "An instance of `ies:Stuff` consisting of timber/wood used as structural members, cladding, or other components." .

building:WoodPortion a rdfs:Class, building:ClassOfStuffPortion ;
    rdfs:label "Wood Portion" ;
    rdfs:comment "An `ies:Entity` that is a portion of `building:wood`." ;
    rdfs:subClassOf building:StuffPortion, building:BuildingMaterial .

### Metal
building:metal a ies:Stuff ;
    rdfs:label "metal" ;
    building:isSumOf building:MetalPortion ;
    rdfs:comment "An instance of `ies:Stuff` consisting of metallic materials (e.g., steel, aluminium) used for members, panels, or claddings." .

building:MetalPortion a rdfs:Class, building:ClassOfStuffPortion ;
    rdfs:label "Metal Portion" ;
    rdfs:comment "An `ies:Entity` that is a portion of `building:metal`." ;
    rdfs:subClassOf building:StuffPortion, building:BuildingMaterial .

### Render / Plaster
building:renderPlaster a ies:Stuff ;
    rdfs:label "render/plaster" ;
    building:isSumOf building:RenderPlasterPortion ;
    rdfs:comment "An instance of `ies:Stuff` used as a render or plaster finish applied to surfaces; underlying substrate unspecified." .

building:RenderPlasterPortion a rdfs:Class, building:ClassOfStuffPortion ;
    rdfs:label "Render/Plaster Portion" ;
    rdfs:comment "An `ies:Entity` that is a portion of `building:renderPlaster`." ;
    rdfs:subClassOf building:StuffPortion, building:BuildingMaterial .

### Artificial (non-concrete)
building:SyntheticMaterial a ies:Stuff ;
    rdfs:label "synthetic material" ;
    building:isSumOf building:SyntheticMaterialPortion ;
    rdfs:comment "An instance of `ies:Stuff` consisting of man-made non-concrete materials (e.g., plastics, composites, synthetic panels)." .

building:SyntheticMaterialPortion a rdfs:Class, building:ClassOfStuffPortion ;
    rdfs:label "Synthetic Material Portion" ;
    rdfs:comment "An `ies:Entity` that is a portion of `building:SyntheticMaterial`." ;
    rdfs:subClassOf building:StuffPortion, building:BuildingMaterial .

#####################  Inspired by roof materials ##################################

### Tile
building:tile a ies:Stuff ;
    rdfs:label "tile" ;
    building:isSumOf building:TilePortion ;
    rdfs:comment "An instance of `ies:Stuff` consisting of tile used as a construction material. Typically overlapping or interlocking units, which may be flat or curved." .

building:TilePortion a rdfs:Class, building:ClassOfStuffPortion ;
    rdfs:label "Tile Portion" ;
    rdfs:comment "An `ies:Entity` that is a portion of `building:tile`." ;
    rdfs:subClassOf building:StuffPortion, building:BuildingMaterial .


### Slate
building:slate a ies:Stuff ;
    rdfs:label "slate" ;
    building:isSumOf building:SlatePortion ;
    rdfs:comment "An instance of `ies:Stuff` consisting of slate used as a construction material. Thin, fine-grained rock typically split into flat sheets." .

building:SlatePortion a rdfs:Class, building:ClassOfStuffPortion ;
    rdfs:label "Slate Portion" ;
    rdfs:comment "An `ies:Entity` that is a portion of `building:slate`." ;
    rdfs:subClassOf building:StuffPortion, building:BuildingMaterial .


### Metal
building:metal a ies:Stuff ;
    rdfs:label "metal" ;
    building:isSumOf building:MetalPortion ;
    rdfs:comment "An instance of `ies:Stuff` consisting of metal used as a construction material. Includes materials such as steel, aluminium, copper, or zinc sheets and components." .

building:MetalPortion a rdfs:Class, building:ClassOfStuffPortion ;
    rdfs:label "Metal Portion" ;
    rdfs:comment "An `ies:Entity` that is a portion of `building:metal`." ;
    rdfs:subClassOf building:StuffPortion, building:BuildingMaterial .

### Plants
building:Plant a rdfs:Class, ies:ClassOfEntity ;
    rdfs:label "Plant" ;
    rdfs:comment "An `ies:Entity` that is a living organism belonging to the kingdom Plantae, typically characterized by the ability to perform photosynthesis." ;
    rdfs:subClassOf ies:Entity .

### Waterproof Membrane

building:WaterproofMembrane a rdfs:Class, ies:ClassOfEntity ;
    rdfs:label "Plant" ;
    rdfs:comment "An `ies:Entity` that is a thin protective layer or sheet applied to a structure to prevent the passage of water, typically used in roofs, walls, foundations, or other building components to ensure durability and moisture resistance." ;
    rdfs:subClassOf ies:Entity .

### Fabric
building:fabric a ies:Stuff ;
    rdfs:label "fabric" ;
    building:isSumOf building:FabricPortion ;
    rdfs:comment "An instance of `ies:Stuff` consisting of fabric material used in construction. Includes tensile textiles or synthetic fabrics stretched over structural frameworks." .

building:FabricPortion a rdfs:Class, building:ClassOfStuffPortion ;
    rdfs:label "Fabric Portion" ;
    rdfs:comment "An `ies:Entity` that is a portion of `building:fabric`." ;
    rdfs:subClassOf building:StuffPortion, building:BuildingMaterial .


### Glass
building:glass a ies:Stuff ;
    rdfs:label "glass" ;
    building:isSumOf building:GlassPortion ;
    rdfs:comment "An instance of `ies:Stuff` consisting of glass used as a construction material. Includes hard, transparent, or translucent sheets." .

building:GlassPortion a rdfs:Class, building:ClassOfStuffPortion ;
    rdfs:label "Glass Portion" ;
    rdfs:comment "An `ies:Entity` that is a portion of `building:glass`." ;
    rdfs:subClassOf building:StuffPortion, building:BuildingMaterial .


### Polycarbonate
building:polycarbonate a ies:Stuff ;
    rdfs:label "polycarbonate" ;
    building:isSumOf building:PolycarbonatePortion ;
    rdfs:comment "An instance of `ies:Stuff` consisting of polycarbonate used as a construction material. A strong, lightweight, transparent thermoplastic sheet." .

building:PolycarbonatePortion a rdfs:Class, building:ClassOfStuffPortion ;
    rdfs:label "Polycarbonate Portion" ;
    rdfs:comment "An `ies:Entity` that is a portion of `building:polycarbonate`." ;
    rdfs:subClassOf building:StuffPortion, building:BuildingMaterial .


### Thatch
building:thatch a ies:Stuff ;
    rdfs:label "thatch" ;
    building:isSumOf building:ThatchPortion ;
    rdfs:comment "An instance of `ies:Stuff` consisting of thatch used as a construction material. Composed of dry vegetation such as straw, reeds, or palm leaves, layered to form a covering." .

building:ThatchPortion a rdfs:Class, building:ClassOfStuffPortion ;
    rdfs:label "Thatch Portion" ;
    rdfs:comment "An `ies:Entity` that is a portion of `building:thatch`." ;
    rdfs:subClassOf building:StuffPortion, building:BuildingMaterial .

### Union helper for (Brick | Block | StonePortion)
building:Masonry a rdfs:Class, ies:ClassOfEntity ;
    rdfs:label "Masonry" ;
    rdfs:comment "Union class representing masonry made of brick, block, or stone." ;
    rdfs:subClassOf ies:Entity, building:BuildingMaterial .

# Constituents ⊑ Union (no redefinition of constituents)
building:Brick rdfs:subClassOf building:Masonry .
building:Block rdfs:subClassOf building:Masonry .
building:StonePortion rdfs:subClassOf building:Masonry .

########### Roof Inspired Unions ######################

### Glass Or Polycarbonate
building:GlassOrPolycarbonate a rdfs:Class, ies:ClassOfEntity ;
    rdfs:label "Glass Or Polycarbonate" ;
    rdfs:comment "Union class representing material entities made of glass or polycarbonate." ;
    rdfs:subClassOf ies:Entity .

# Constituents ⊑ Union
building:GlassPortion rdfs:subClassOf building:GlassOrPolycarbonate .
building:PolycarbonatePortion rdfs:subClassOf building:GlassOrPolycarbonate .


### Tile Or Stone Or Slate
building:TileOrStoneOrSlate a rdfs:Class, ies:ClassOfEntity ;
    rdfs:label "Tile Or Stone Or Slate" ;
    rdfs:comment "Union class representing material entities made of tile, stone, or slate." ;
    rdfs:subClassOf ies:Entity .

# Constituents ⊑ Union
building:TilePortion rdfs:subClassOf building:TileOrStoneOrSlate .
building:StonePortion rdfs:subClassOf building:TileOrStoneOrSlate .
building:SlatePortion rdfs:subClassOf building:TileOrStoneOrSlate .


### Waterproof Membrane Or Concrete
building:WaterproofMembraneOrConcrete a rdfs:Class, ies:ClassOfEntity ;
    rdfs:label "Waterproof Membrane Or Concrete" ;
    rdfs:comment "Union class representing material entities made of waterproof membrane or concrete." ;
    rdfs:subClassOf ies:Entity .

# Constituents ⊑ Union
building:WaterproofMembranePortion rdfs:subClassOf building:WaterproofMembraneOrConcrete .
building:ConcretePortion rdfs:subClassOf building:WaterproofMembraneOrConcrete .


##############################  Roof Section "Fusions" ##########################

building:hasCombinedSurfaceArea a owl:ObjectProperty ;
    rdfs:label "has combined surface area" ;
    rdfs:comment "A relationship that asserts the arithmetic sum of the surface areas of the members of a class" ;
    rdfs:domain ies:ClassOfEntity ;
    rdfs:range building:SurfaceArea ;
    rdfs:subPropertyOf ies:relationship .

building:ClassOfClassOfRoofSection a rdfs:Class ;
    rdfs:label "Class of Class of Roof Section" ;
    rdfs:comment "A class that represents a category of `building:ClassOfRoofSection` based on shared characteristics." ;
    rdfs:subClassOf building:ClassOfRoofSection .

building:ClassOfClassOfRoofSection a rdfs:Class ;
    rdfs:label "Class of Class of Roof Section" ;
    rdfs:comment "A class that represents a category of `building:ClassOfRoofSection` based on shared characteristics." ;
    rdfs:subClassOf building:ClassOfBuiltEntity .

building:RoofSectionsByCompassOrientation a rdfs:Class, building:ClassOfClassOfRoofSection ;
    rdfs:label "Roof Sections By Aspect" ;
    rdfs:comment "A `ies:ClassOfClassOfRoofSection` that classifies roof sections by their  compass orientation" ;
    rdfs:subClassOf building:ClassOfRoofSection .

# 8-point compass classes for roof sections

building:NorthFacingRoofSectionSum a rdfs:Class, building:RoofSectionsByCompassOrientation ;
    rdfs:label "North Facing Roof Sections" ;
    rdfs:comment "An instance of `ies:RoofSectionsByCompassOrientation` that represents the sum of roof sections that face north.  They need not be contiguous.  Instances are `rdfs:subClassOf building:RoofSection`." ;
    rdfs:subClassOf building:ClassOfRoofSection ;
    ies:eachMemberIsPartOfSomeMemberOf building:Roof .

building:EastFacingRoofSectionSum a rdfs:Class, building:RoofSectionsByCompassOrientation ;
    rdfs:label "East Facing Roof Sections" ;
    rdfs:comment "An instance of `ies:RoofSectionsByCompassOrientation` that represents the sum of roof sections that face east.  They need not be contiguous.  Instances are `rdfs:subClassOf building:RoofSection`." ;
    rdfs:subClassOf building:ClassOfRoofSection ;
    ies:eachMemberIsPartOfSomeMemberOf building:Roof .

building:SouthFacingRoofSectionSum a rdfs:Class, building:RoofSectionsByCompassOrientation ;
    rdfs:label "South Facing Roof Sections" ;
    rdfs:comment "An instance of `ies:RoofSectionsByCompassOrientation` that represents the sum of roof sections that face south.  They need not be contiguous.  Instances are `rdfs:subClassOf building:RoofSection`." ;
    rdfs:subClassOf building:ClassOfRoofSection ;
    ies:eachMemberIsPartOfSomeMemberOf building:Roof .

building:WestFacingRoofSectionSum a rdfs:Class, building:RoofSectionsByCompassOrientation ;
    rdfs:label "West Facing Roof Sections" ;
    rdfs:comment "An instance of `ies:RoofSectionsByCompassOrientation` that represents the sum of roof sections that face west.  They need not be contiguous.  Instances are `rdfs:subClassOf building:RoofSection`." ;
    rdfs:subClassOf building:ClassOfRoofSection ;
    ies:eachMemberIsPartOfSomeMemberOf building:Roof .

building:NorthEastFacingRoofSectionSum a rdfs:Class, building:RoofSectionsByCompassOrientation ;
    rdfs:label "North East Facing Roof Sections" ;
    rdfs:comment "An instance of `ies:RoofSectionsByCompassOrientation` that represents the sum of roof sections that face north east.  They need not be contiguous.  Instances are `rdfs:subClassOf building:RoofSection`." ;
    rdfs:subClassOf building:ClassOfRoofSection ;
    ies:eachMemberIsPartOfSomeMemberOf building:Roof .

building:SouthEastFacingRoofSectionSum a rdfs:Class, building:RoofSectionsByCompassOrientation ;
    rdfs:label "South East Facing Roof Sections" ;
    rdfs:comment "An instance of `ies:RoofSectionsByCompassOrientation` that represents the sum of roof sections that face south east.  They need not be contiguous.  Instances are `rdfs:subClassOf building:RoofSection`." ;
    rdfs:subClassOf building:ClassOfRoofSection ;
    ies:eachMemberIsPartOfSomeMemberOf building:Roof .

building:SouthWestFacingRoofSectionSum a rdfs:Class, building:RoofSectionsByCompassOrientation ;
    rdfs:label "South West Facing Roof Sections" ;
    rdfs:comment "An instance of `ies:RoofSectionsByCompassOrientation` that represents the sum of roof sections that face south west.  They need not be contiguous.  Instances are `rdfs:subClassOf building:RoofSection`." ;
    rdfs:subClassOf building:ClassOfRoofSection ;
    ies:eachMemberIsPartOfSomeMemberOf building:Roof .

building:NorthWestFacingRoofSectionSum a rdfs:Class, building:RoofSectionsByCompassOrientation ;
    rdfs:label "North West Facing Roof Sections" ;
    rdfs:comment "An instance of `ies:RoofSectionsByCompassOrientation` that represents the sum of roof sections that face north west.  They need not be contiguous.  Instances are `rdfs:subClassOf building:RoofSection`." ;
    rdfs:subClassOf building:ClassOfRoofSection ;
    ies:eachMemberIsPartOfSomeMemberOf building:Roof .

############################  Building parts code set analysis ################################
building:Tower a rdfs:Class ;
    rdfs:label "Tower" ;
    rdfs:comment "A building that is tall and vertically oriented, typically rising significantly above its surroundings, often serving purposes such as observation, defence, habitation, or communication." ;
    rdfs:subClassOf building:Structure .


building:AirTrafficControlTower a rdfs:Class ;
  rdfs:label "Air Traffic Control Tower" ;
  rdfs:comment "A tower from which aircraft movements are monitored and directed." ;
  rdfs:subClassOf building:Tower .

building:BoatHouse a rdfs:Class ;
  rdfs:label "Boat House" ;
  rdfs:comment "A Building that is positioned by water and designed for the shelter and storage of boats, often with direct water access." ;
  rdfs:subClassOf building:Building .

building:Building a rdfs:Class ;
  rdfs:label "Building" ;
  rdfs:comment "A Building that includes a roof and walls forming enclosed space suitable for occupation or use." ;
  rdfs:subClassOf building:Building .

building:Castle a rdfs:Class ;
  rdfs:label "Castle" ;
  rdfs:comment "A building that is a medieval or early-modern fortification or a pseudo-fortified stately house." ;
  rdfs:subClassOf building:Building .

building:Columbarium a rdfs:Class ;
  rdfs:label "Columbarium" ;
  rdfs:comment "A Building that houses niches for urns containing human remains and provides access to those niches." ;
  rdfs:subClassOf building:Building .

building:Kiln a rdfs:Class ;
  rdfs:label "Kiln" ;
  rdfs:comment "A Building that contains a furnace or oven for burning, baking, or drying materials." ;
  rdfs:subClassOf building:Building .

building:Lighthouse a rdfs:Class ;
  rdfs:label "Lighthouse" ;
  rdfs:comment "A Building that is a tower containing a navigational light to aid maritime or aerial traffic." ;
  rdfs:subClassOf building:Building .

building:MartelloTower a rdfs:Class ;
  rdfs:label "Martello Tower" ;
  rdfs:comment "A low, round coastal defence tower historically designed to carry artillery." ;
  rdfs:subClassOf building:Tower .

building:MultistoreyCarPark a rdfs:Class ;
  rdfs:label "Multistorey Car Park" ;
  rdfs:comment "A Building that comprises multiple levels dedicated to the parking or storage of vehicles." ;
  rdfs:subClassOf building:Building .

building:Pagoda a rdfs:Class ;
  rdfs:label "Pagoda" ;
  rdfs:comment "A Building that is a multi‑storey structure with ornamental roofs at each level, stylistically derived from from East and South East Asia temple forms." ;
  rdfs:subClassOf building:Building .

building:PoliceCallBox a rdfs:Class ;
  rdfs:label "Police Call Box" ;
  rdfs:comment "A Building that is a small kiosk designed to house a telephone for contacting the police." ;
  rdfs:subClassOf building:Building .

building:RoofedBandstand a rdfs:Class ;
  rdfs:label "Roofed Bandstand" ;
  rdfs:comment "A Building that is a roofed performance platform, typically open at the sides, for public musical events." ;
  rdfs:subClassOf building:Building .

building:Shelter a rdfs:Class ;
  rdfs:label "Shelter" ;
  rdfs:comment "A structure that provides cover for people against weather or adverse conditions." ;
  rdfs:subClassOf building:Structure .

building:SignalBox a rdfs:Class ;
  rdfs:label "Signal Box" ;
  rdfs:comment "A Building that is a distinctive railway‑side structure historically housing the mechanisms for points and signals." ;
  rdfs:subClassOf building:Building .

building:StaticCaravanOrMobileHome a rdfs:Class ;
  rdfs:label "Static Caravan Or Mobile Home" ;
  rdfs:comment "A Building that is a relocatable dwelling originally designed for movement but positioned for residential or holiday use." ;
  rdfs:subClassOf building:Building .

building:Tomb a rdfs:Class ;
  rdfs:label "Tomb" ;
  rdfs:comment "A Sepulchre a roofed edifice used for the interment of human remains." ;
  rdfs:subClassOf building:Sepulchre .

building:WheelHouse a rdfs:Class ;
  rdfs:label "Wheel House" ;
  rdfs:comment "A Building that houses the lifting gear associated with mining operations." ;
  rdfs:subClassOf building:Building .

building:Windmill a rdfs:Class ;
  rdfs:label "Windmill" ;
  rdfs:comment "A Building that is designed to be wind‑driven for milling or pumping and typically comprises an occupiable tower with sails." ;
  rdfs:subClassOf building:Building .

building:BellTower a rdfs:Class ;
  rdfs:label "Bell Tower" ;
  rdfs:comment "A free-standing tower designed primarily to house and sound suspended bells." ;
  rdfs:subClassOf building:Tower .

building:BoreHole a rdfs:Class ;
  rdfs:label "Bore Hole" ;
  rdfs:comment "A Structure that encloses a drilled hole used to extract substances such as water, oil, or gas." ;
  rdfs:subClassOf building:Structure .

building:Bridge a rdfs:Class ;
    rdfs:label "Bridge" ;
    rdfs:comment "A structure that is built to span a physical obstacle, such as a river, valley, or road, providing a passage for pedestrians, vehicles, or utilities." ;
    rdfs:subClassOf building:Structure .

building:CableBridge a rdfs:Class ;
  rdfs:label "Cable Bridge" ;
  rdfs:comment "A bridge built to carry cables over an obstacle such as a river or road." ;
  rdfs:subClassOf building:Bridge .

building:CastleWall a rdfs:Class ;
  rdfs:label "Castle Wall" ;
  rdfs:comment "A defensive wall forming part of a castle or fortified complex." ;
  rdfs:subClassOf building:Wall .

building:ClockTower a rdfs:Class ;
  rdfs:label "Clock Tower" ;
  rdfs:comment "A tall tower incorporating one or more clock faces positioned near its summit." ;
  rdfs:subClassOf building:Tower .

building:Sepulchre a rdfs:Class ;
    rdfs:label "Sepulchre" ;
    rdfs:comment "A structure that is built to receive and enclose the body of the dead, serving as a place of burial and remembrance." ;
    rdfs:subClassOf building:Structure .

building:Crypt a rdfs:Class ;
  rdfs:label "Crypt" ;
  rdfs:comment "A Sepulchre that is an underground or partly underground chamber used to inter the dead." ;
  rdfs:subClassOf building:Sepulchre .

building:FogHorn a rdfs:Class ;
  rdfs:label "Fog Horn" ;
  rdfs:comment "A Structure that contains apparatus to emit loud warning sounds in conditions of reduced visibility near navigable waters." ;
  rdfs:subClassOf building:Structure .

building:Gantry a rdfs:Class ;
  rdfs:label "Gantry" ;
  rdfs:comment "A Structure that is an elevated framework supported on legs designed to carry loads or equipment such as signals, pipes or tackle." ;
  rdfs:subClassOf building:Structure .

building:Hide a rdfs:Class ;
  rdfs:label "Hide" ;
  rdfs:comment "A camouflaged shelter permitting observation of wildlife without disturbance." ;
  rdfs:subClassOf building:Shelter .

building:LychGate a rdfs:Class ;
  rdfs:label "Lych Gate" ;
  rdfs:comment "A Structure that is a roofed gateway typically at the entrance to a churchyard." ;
  rdfs:subClassOf building:Structure .

building:MotorVehicleWeighbridge a rdfs:Class ;
  rdfs:label "Motor Vehicle Weighbridge" ;
  rdfs:comment "A Structure that houses apparatus for weighing road vehicles and their loads." ;
  rdfs:subClassOf building:Structure .

building:RailVehicleWeighbridge a rdfs:Class ;
  rdfs:label "Rail Vehicle Weighbridge" ;
  rdfs:comment "A Structure that houses apparatus for weighing rail vehicles and their loads." ;
  rdfs:subClassOf building:Structure .

building:RoofedClockTower a rdfs:Class ;
  rdfs:label "Roofed Clock Tower" ;
  rdfs:comment "A tower incorporating a clock and covered by a roofed superstructure." ;
  rdfs:subClassOf building:Tower .

building:RoofedShaft a rdfs:Class ;
  rdfs:label "Roofed Shaft" ;
  rdfs:comment "A Structure that encloses the vertical or near‑vertical entrance to a mine." ;
  rdfs:subClassOf building:Structure .

building:RoofedTower a rdfs:Class ;
  rdfs:label "Roofed Tower" ;
  rdfs:comment "A tall, isolated tower covered by a roof and lacking an explicit functional specification." ;
  rdfs:subClassOf building:Tower .

building:RoofedWell a rdfs:Class ;
  rdfs:label "Roofed Well" ;
  rdfs:comment "A Structure that is a water‑extraction well provided with a protective roof." ;
  rdfs:subClassOf building:Structure .

building:Stand a rdfs:Class ;
  rdfs:label "Stand" ;
  rdfs:comment "A Structure that provides tiered seating and/or standing accommodation for spectators, with at least one open side." ;
  rdfs:subClassOf building:Structure .

building:TelecommunicationsMast a rdfs:Class ;
  rdfs:label "Telecommunications Mast" ;
  rdfs:comment "A Structure that is a tall mast supporting equipment for transmitting or receiving electronic signals." ;
  rdfs:subClassOf building:Structure .

building:Terraces a rdfs:Class ;
  rdfs:label "Terraces" ;
  rdfs:comment "A Structure that comprises banked, wide steps forming spectator accommodation with at least one open side." ;
  rdfs:subClassOf building:Structure .

building:TravellingCrane a rdfs:Class ;
  rdfs:label "Travelling Crane" ;
  rdfs:comment "A Structure that houses rail‑mounted lifting machinery capable of moving loads along a track." ;
  rdfs:subClassOf building:Structure .

building:VehicleDip a rdfs:Class ;
  rdfs:label "Vehicle Dip" ;
  rdfs:comment "A Structure that contains a sunken basin used for immersing vehicles in disinfectant solution." ;
  rdfs:subClassOf building:Structure .

building:WaterPumpingChamber a rdfs:Class ;
  rdfs:label "Water Pumping Chamber" ;
  rdfs:comment "A Structure that contains a void or chamber from which fresh water is pumped to regulate supply." ;
  rdfs:subClassOf building:Structure .

building:WaterTower a rdfs:Class ;
  rdfs:label "Water Tower" ;
  rdfs:comment "A tall tower supporting a water tank to provide pressure and regulate supply." ;
  rdfs:subClassOf building:Tower .

building:Weir a rdfs:Class ;
  rdfs:label "Weir" ;
  rdfs:comment "A Structure that is a barrier built across a watercourse to control or divert flow." ;
  rdfs:subClassOf building:Structure .

building:Well a rdfs:Class ;
  rdfs:label "Well" ;
  rdfs:comment "A Structure that is a constructed shaft or hole for extracting water from the ground." ;
  rdfs:subClassOf building:Structure .

building:WindPump a rdfs:Class ;
  rdfs:label "Wind Pump" ;
  rdfs:comment "A Structure that is a tower or mast supporting wind‑driven blades used to pump water." ;
  rdfs:subClassOf building:Structure .

building:Arch a rdfs:Class ;
  rdfs:label "Arch" ;
  rdfs:comment "A BuiltEntity that is a curved structural element spanning an opening and bearing load from above." ;
  rdfs:subClassOf building:BuiltEntity .

building:Archway a rdfs:Class ;
  rdfs:label "Archway" ;
  rdfs:comment "A BuiltEntity that is a roofed passage opening formed within a Structure allowing vehicular passage." ;
  rdfs:subClassOf building:BuiltEntity .

building:Pergola a rdfs:Class ;
  rdfs:label "Pergola" ;
  rdfs:comment "A BuiltEntity that is a colonnaded passage supporting a trellised roof intended for planting." ;
  rdfs:subClassOf building:BuiltEntity .

building:RoofedChimney a rdfs:Class ;
  rdfs:label "Roofed Chimney" ;
  rdfs:comment "A BuiltEntity that is a flue or chimney provided with a protective roof or capping." ;
  rdfs:subClassOf building:BuiltEntity .

building:RoofedLeat a rdfs:Class ;
  rdfs:label "Roofed Leat" ;
  rdfs:comment "A BuiltEntity that is a watercourse enclosed by a conventional roof, conveying water for processes." ;
  rdfs:subClassOf building:BuiltEntity .

building:RoofedOutfall a rdfs:Class ;
  rdfs:label "Roofed Outfall" ;
  rdfs:comment "A BuiltEntity that is a roofed channel or structure used to discharge liquids to a receiving water body." ;
  rdfs:subClassOf building:BuiltEntity .

building:SupportedRoofedConveyor a rdfs:Class ;
  rdfs:label "Supported Roofed Conveyor" ;
  rdfs:comment "A BuiltEntity that is an elevated, roofed conveyor installation for transporting materials." ;
  rdfs:subClassOf building:BuiltEntity .

building:VentilationShaft a rdfs:Class ;
  rdfs:label "Ventilation Shaft" ;
  rdfs:comment "A BuiltEntity that is a vertical passage constructed to allow air flow to or from tunnels or underground spaces." ;
  rdfs:subClassOf building:BuiltEntity .

building:Waterwheel a rdfs:Class ;
  rdfs:label "Waterwheel" ;
  rdfs:comment "A BuiltEntity that is a large wheel driven by flowing water to transmit mechanical power." ;
  rdfs:subClassOf building:BuiltEntity .

building:BuildingWithMadeSurface a rdfs:Class ;
  rdfs:label "Building And Made Surface" ;
  rdfs:comment "A BuiltEntity that is a man‑made surface which simultaneously serves as the roof to a Building below." ;
  rdfs:subClassOf building:BuiltEntity .

building:BuildingUnderConstruction a rdfs:Class ;
  rdfs:label "Building Under Construction" ;
  rdfs:comment "A StructureState that is the temporal condition of a Building while construction is in progress and completion has not yet occurred." ;
  rdfs:subClassOf building:StructureState .

building:RuinedBuilding a rdfs:Class ;
  rdfs:label "Ruined Building" ;
  rdfs:comment "A StructureState that is the temporal condition of a Building when much of its fabric has decayed or collapsed so it is no longer fully functional." ;
  rdfs:subClassOf building:StructureState .

building:BuildingWithCarParkOnRoof a rdfs:Class ;
  rdfs:label "Building With Car Park On Roof" ;
  rdfs:comment "A StructureState that is the temporal condition of a Building whose roof is used as a car‑parking surface." ;
  rdfs:subClassOf building:StructureState .

building:BuildingWithPathOnRoof a rdfs:Class ;
  rdfs:label "Building With Path On Roof" ;
  rdfs:comment "A StructureState that is the temporal condition of a Building whose roof provides a pedestrian pathway." ;
  rdfs:subClassOf building:StructureState .

building:BuildingWithDovecot a rdfs:Class ;
  rdfs:label "Building And Dovecot" ;
  rdfs:comment "A StructureState that is the temporal condition of a Building equipped with internal provision for dovecote roosting." ;
  rdfs:subClassOf building:StructureState .

building:BuildingWithLight a rdfs:Class ;
  rdfs:label "Building And Light" ;
  rdfs:comment "A StructureState that is the temporal condition of a Building equipped with a light for illuminating surrounding areas." ;
  rdfs:subClassOf building:StructureState .

building:FloatingStructure a rdfs:Class ;
  rdfs:label "Floating Structure" ;
  rdfs:comment "A StructureState that is the temporal condition of a Structure situated afloat upon the surface of water." ;
  rdfs:subClassOf building:StructureState .

###################### Named Location Classes #######################

building:LocationAsBuildingLine a rdfs:Class ;
    rdfs:label "Location As Building line" ;
    rdfs:comment "An `building:ClassOfLocation`" ;
    rdfs:subClassOf building:ClassOfLocationState .  # class of state


### Building Internal Division
building:BuildingInternalDivision
  a rdfs:Class, building:LocationAsBuildingLine ;
  rdfs:subClassOf ies:Location ; # State ;
  rdfs:label "Building Internal Division"@en ;
  rdfs:comment "An ies:Location that denotes the alignment of a division internal to a building complex—either between two buildings with the same occupier, between individual garages within a block, or between buildings that have an overhanging outline or a shared occupation."@en ;
  dct:source <https://docs.os.uk/osngd/code-lists/code-lists-overview/buildinglinedescriptionvalue> .

### Building Occupier Division
building:BuildingOccupierDivision
  a rdfs:Class, building:LocationAsBuildingLine ;
  rdfs:subClassOf ies:Location ;
  rdfs:label "Building Occupier Division"@en ;
  rdfs:comment "An ies:Location that denotes the alignment of the division between two buildings that have different occupiers."@en ;
  dct:source <https://docs.os.uk/osngd/code-lists/code-lists-overview/buildinglinedescriptionvalue> .

### Overhanging Building Edge
building:OverhangingBuildingEdge
  a rdfs:Class, building:LocationAsBuildingLine ;
  rdfs:subClassOf ies:Location ;
  rdfs:label "Overhanging Building Edge"@en ;
  rdfs:comment "An ies:Location that denotes the edge delimiting the limit of a building element that overhangs and allows passage underneath."@en ;
  dct:source <https://docs.os.uk/osngd/code-lists/code-lists-overview/buildinglinedescriptionvalue> .


##############################
# OS Geographic concepts     #
##############################

building:SovereignCountry a rdfs:Class ;
    rdfs:label "Sovereign Country" ;
    rdfs:comment "A country that is the whole region ruled by a sovereign state, and is not a region of another country; a few examples include the United Kingdom, Italy, Japan, Kenya, and the USA; England, Scotland, Wales, and Northern Ireland are not sovereign countries, but rather constituent countries" ;
    rdfs:subClassOf ies:Country .

building:ConstituentCountry a rdfs:Class ;
    rdfs:label "Constituent Country" ;
    rdfs:comment "A country that is a region of another country; constituent countries have typically been devolved a high degree of autonomy because of its distinctive historical and cultural identity; England, Scotland, Wales, and Northern Ireland are the four constituent countries of the United Kingdom of Great Britain and Northern Ireland; other examples of constituent countries include Denmark, Greenland, and the Faroe Islands, which are the three constituent countries of the Kingdom of Denmark" ;
    rdfs:subClassOf ies:Country, ies:RegionOfCountry .

building:UKLocalAdministrativeRegion a rdfs:Class ;
   rdfs:label "UK Local Administrative Region" ;
   rdfs:comment "A region of the UK that is an administrative division of one of its four constituent countries; local administrative regions have different names depending on the constituent countries in which they are located" ;
   rdfs:subClassOf ies:RegionOfCountry .

building:UpperTierLocalAdministrativeRegion a rdfs:Class ;
   rdfs:label "Upper-Tier Local Administrative Region" ;
   rdfs:comment "A UK local administrative region that is a direct administrative division of one of the constituent countries of the United Kingdom; the councils of upper-tier local administrative regions are responsible for strategic, high cost services in the related region; some - which are called 'unitary authorities' -  are also responsible for more localized services, hence serving all government functions in the region" ;
   rdfs:subClassOf building:UKLocalAdministrativeRegion .

building:LowerTierLocalAdministrativeRegion a rdfs:Class ;
   rdfs:label "Lower-Tier Local Administrative Region" ;
   rdfs:comment "A UK local administrative region that is not a direct administrative division of one of the constituent countries of the United Kingdom; the councils of lower-tier local administrative regions are only responsible for localized services like housing, waste collection, and leisure" ;
   rdfs:subClassOf building:UKLocalAdministrativeRegion .

building:UnitaryAuthorityRegion a rdfs:Class ;
   rdfs:label "Unitary Authority Region" ;
   rdfs:comment "An upper-tier local administrative region whose administration is responsible for all government functions and services in a given area; informally, a unitary authority can be said to combine the functions of a county council and those of a district council" ;
   rdfs:subClassOf building:UpperTierLocalAdministrativeRegion .

building:EnglishAdministrativeCounty a rdfs:Class ;
   rdfs:label "English Administrative County" ;
   rdfs:comment "An upper-tier local administrative region that (i) is a direct administrative division of England, and (ii) is further divided into districts; county councils are responsible for strategic, higher cost services like education, social services, and transport, whereas more localized services are responsibility of district councils" ;
   rdfs:subClassOf building:UpperTierLocalAdministrativeRegion .

building:MetropolitanCounty a rdfs:Class ;
   rdfs:label "Metropolitan County" ;
   rdfs:comment "An English administrative county that approximately corresponds to one large town or city" ;
   rdfs:subClassOf building:EnglishAdministrativeCounty .

building:NonMetropolitanCounty a rdfs:Class ;
   rdfs:label "Non-Metropolitan County" ;
   rdfs:comment "An English administrative county that does not correspond to one large town or city, and typically encompasses various settlements and rural areas" ;
   rdfs:subClassOf building:EnglishAdministrativeCounty .

building:ScottishCouncilArea a rdfs:Class ;
   rdfs:label "Scottish Council Area" ;
   rdfs:comment "An upper-tier local administrative region that is a direct administrative division of Scotland; all Scottish council areas are unitary authority regions" ;
   rdfs:subClassOf building:UpperTierLocalAdministrativeRegion, building:UnitaryAuthorityRegion .

building:WelshPrincipalArea a rdfs:Class ;
   rdfs:label "Welsh Principal Area" ;
   rdfs:comment "An upper-tier local administrative region that is a direct administrative division of Wales; all Welsh principal areas are unitary authority regions" ;
   rdfs:subClassOf building:UpperTierLocalAdministrativeRegion, building:UnitaryAuthorityRegion .

building:NorthernIrelandDistrict a rdfs:Class ;
   rdfs:label "Northern Ireland District" ;
   rdfs:comment "An upper-tier local administrative region that is a direct administrative division of Northern Ireland; all Northern Ireland Districts are unitary authority regions" ;
   rdfs:subClassOf building:UpperTierLocalAdministrativeRegion, building:UnitaryAuthorityRegion .

building:EnglishDistrict a rdfs:Class ;
   rdfs:label "English District" ;
   rdfs:comment "A lower-tier local administrative region that is a direct administrative division of an English administrative county" ;
   rdfs:subClassOf building:LowerTierLocalAdministrativeRegion .

building:CivilParish a rdfs:Class ;
   rdfs:label "Civil Parish" ;
   rdfs:comment "A lower-tier local administrative region that is a direct administrative division of either a unitary authority or an English district; civil parishes are the lowest-level administrative divisions of England, since they have no smaller administrative divisions; civil parishes are typically - but not exclusively - found in rural areas" ;
   rdfs:subClassOf building:LowerTierLocalAdministrativeRegion, building:CivilParishOrCommunityArea .

building:WelshCommunityArea a rdfs:Class ;
   rdfs:label "Welsh Community Area" ;
   rdfs:comment "A lower-tier local administrative region that is a direct administrative division of a Welsh principal area; community areas can be viewed as the Welsh analog of English civil parishes and have similarly localized responsibilities" ;
   rdfs:subClassOf building:LowerTierLocalAdministrativeRegion, building:CivilParishOrCommunityArea .

building:CivilParishOrCommunityArea a rdfs:Class ;
   rdfs:label "Civil Parish Or Community Area" ;
   rdfs:comment "A lower-tier local administrative region that is either an English civil parish or a Welsh community area" ;
   rdfs:subClassOf building:LowerTierLocalAdministrativeRegion .

building:ConstituencyRegion a rdfs:Class ;
   rdfs:label "Constituency Region" ;
   rdfs:comment "A region of a country that is instituted for enabling the residing voters to elect their representatives in either the central government of the country or in some local administration" ;
   rdfs:subClassOf ies:RegionOfCountry .

building:UKParliamentConstituencyRegion a rdfs:Class ;
   rdfs:label "UK Parliamentary Constituency Region" ;
   rdfs:comment "A constituency that is instituted for electing one member of the House of Commons in each UK general election" ;
   rdfs:subClassOf building:ConstituencyRegion .

building:DevolvedParliamentConstituencyRegion a rdfs:Class ;
   rdfs:label "Devolved Parliament Constituency Region" ;
   rdfs:comment "A constituency that is instituted for electing members of one of the three devolved parliaments of the United Kingdom; the devolved parliaments of the United Kingdom are the Scottish Parliament, the Welsh Parliament (aka Senedd Cymru), and the Northern Ireland Assembly" ;
   rdfs:subClassOf building:ConstituencyRegion .

building:ScottishParliamentConstituencyRegion a rdfs:Class ;
   rdfs:label "Scottish Parliament Constituency Region" ;
   rdfs:comment "A constituency that is instituting for electing one member of the Scottish Parliament in each Scottish Parliament election" ;
   rdfs:subClassOf building:DevolvedParliamentConstituencyRegion .

building:SeneddConstituencyRegion a rdfs:Class ;
   rdfs:label "Senedd Constituency Region" ;
   rdfs:comment "A constituency that is instituted for electing one member of the Welsh Parliament (aka Senedd Cymru) in each Senedd election" ;
   rdfs:subClassOf building:DevolvedParliamentConstituencyRegion .

building:AssemblyConstituencyRegion a rdfs:Class ;
   rdfs:label "Assembly Constituency Region" ;
   rdfs:comment "A constituency that is instituted for electing one member of the Northern Ireland Assembly in each Northern Ireland Assembly election" ;
   rdfs:subClassOf building:DevolvedParliamentConstituencyRegion .

building:Ward a rdfs:Class ;
   rdfs:label "Ward" ;
   rdfs:comment "A constituency that is instituted for electing one or more representatives in local elections" ;
   rdfs:subClassOf building:ConstituencyRegion .

building:CeremonialCounty a rdfs:Class ;
   rdfs:label "Ceremonial County" ;
   rdfs:comment "A region of a the UK that is instituted for appointing a Lord Lieutenant and possibly one or two High Sheriffs, who serve respectively as personal and judicial representative of the regnant king or queen; many ceremonial counties approximately correspond or are even identical to administrative regions of the UK" ;
   rdfs:subClassOf ies:RegionOfCountry .

building:EnglishCeremonialCounty a rdfs:Class ;
   rdfs:label "English Ceremonial County" ;
   rdfs:comment "A ceremonial county that is part of England; each English ceremonial county has one Lord Lieutenant and one or two High Sheriffs" ;
   rdfs:subClassOf building:CeremonialCounty .

building:ScottishLieutenancyArea a rdfs:Class ;
   rdfs:label "Scottish Lieutenancy Area" ;
   rdfs:comment "A ceremonial county that is part of Scotland; each Scottish Lieutenancy Area has one Lord Lieutenant, but no High Sheriff" ;
   rdfs:subClassOf building:CeremonialCounty .

building:WelshPreservedCounty a rdfs:Class ;
   rdfs:label "Welsh Preserved County" ;
   rdfs:comment "A ceremonial county that is part of Wales; each Welsh Preserved County has one Lord Lieutenant and one High Sheriff" ;
   rdfs:subClassOf building:CeremonialCounty .

building:NorthernIrelandLieutenancyArea a rdfs:Class ;
   rdfs:label "Northern Ireland Lieutenancy Area" ;
   rdfs:comment "A ceremonial county that is part of Northern Ireland; each Northern Ireland Lieutenancy Area has one Lord Lieutenant, but no High Sheriff" ;
   rdfs:subClassOf building:CeremonialCounty .

building:HistoricCounty a rdfs:Class ;
   rdfs:label "Historic County" ;
   rdfs:comment "A region of the UK that was initially instituted as a feudal or administrative division in a time span that goes from the Early Middle Ages to the Tudor period; historic counties are linked to cultural and local identities, and are still referred to for certain purposes, like sport initiatives or even judicial purposes" ;
   rdfs:subClassOf ies:RegionOfCountry .

building:GeopoliticalDependency a rdfs:Class ;
   rdfs:label "Geopolitical Dependency" ;
   rdfs:comment "A location that (i) is not part of a sovereign country, and (ii) is in some respects under the jurisdiction of the institutions of a sovereign country; examples include Puerto Rico (which is a dependency of the USA), the Cook Islands (which are a dependency of New Zealand), and the British Overseas Territories - and the Falklands - which are dependencies of the United Kingdom" ;
   rdfs:subClassOf ies:Location .

building:isGeopoliticalDependencyOf a owl:ObjectProperty ;
   rdfs:label "is Geopolitical Dependency Of" ;
   rdfs:comment "The relation that obtains between a geopolitical dependency d and a sovereign country c if and only if the government of d is in some respects under the jurisdiction of the institutions of c" ;
   rdfs:domain building:GeopoliticalDependency ;
   rdfs:range building:SovereignCountry ;
   rdfs:subPropertyOf ies:relationship .

building:CrownDependency a rdfs:Class ;
   rdfs:label "Crown Dependency" ;
   rdfs:comment "A geopolitical dependency that (i) is a dependency of the United Kingdom, (ii) is part of the British Isles, and (iii) is under the sovereignty of the British Crown; there are three Crown dependencies: the Isle of Man, the Bailiwick of Jersey, and the Bailiwick of Guernsey" ;
   rdfs:subClassOf building:GeopoliticalDependency .

building:BritishOverseasTerritory a rdfs:Class ;
   rdfs:label "British Overseas Territory" ;
   rdfs:comment "A geopolitical dependency that (i) is a dependency of the United Kingdom, (ii) is located outside of the British Isles, and (iii) is under the rule of the United Kingdom's government; most British overseas territories are former colonies of the British Empire, but some are not: for example, the British Antarctic Territory and South Georgia and the South Sandwich Islands, both of which are mainly used for research purposes" ;
   rdfs:subClassOf building:GeopoliticalDependency .

building:isInstitutionalSuccessorOf a owl:ObjectProperty ;
   rdfs:label "is Institutional Successor Of" ;
   rdfs:comment "The sub-relation of ies:successorTo that obtains between two regions of a country (ies:RegionOfCountry) if and only if the former has replaced the latter within the administrative hierarchy of a country" ;
   rdfs:domain ies:RegionOfCountry ;
   rdfs:range ies:RegionOfCountry ;
   rdfs:subPropertyOf ies:successorTo .

building:Waterbody a rdfs:Class ;
   rdfs:label "Waterbody" ;
   rdfs:comment "A geographic feature that is a large water mass; for example, a sea or a stream - conceived as a mass of water, rather than the channel conveying it" ;
   rdfs:subClassOf ies:GeographicFeature .

building:TidalWaterbody a rdfs:Class ;
   rdfs:label "Tidal Water Body" ;
   rdfs:comment "A waterbody that is affected by tides - that is, cyclical changes in the water level due to the gravitational pull of the Moon and the Sun; besides seas, oceans, and their parts, other types of waterbody can also be tidal, including rivers and lakes that are connected to the sea" ;
   rdfs:subClassOf building:Waterbody .

building:NonTidalWaterbody a rdfs:Class ;
   rdfs:label "Non-Tidal Water Body" ;
   rdfs:comment "A waterbody that is not affected by tides" ;
   rdfs:subClassOf building:Waterbody .
